---
tags:
  - chapter
  - cmplxanal
date: 2025-02-03
completed: true
---
[[Directory]], [[Complex Analysis 1|Subject Directory]]
[[University/Undergraduate/Second Year/Complex Analysis/Lectures/1. |ðŸž€ðŸž€]] [[University/Undergraduate/Second Year/Complex Analysis/Lectures/6. |â—€]] [[University/Undergraduate/Second Year/Complex Analysis/Lectures/8. |â–¶]] [[University/Undergraduate/Second Year/Complex Analysis/Lectures/22. |ðŸž‚ðŸž‚]]
# 
## 
### Definition 1.1: Power Series
A power series is a series of the form
$$
f(z)=\sum_{n=0}^{\infty} a_{n}(z-z_{0})^{n}
$$
where ${} z_{0} \in \mathbb{C} {}$ and ${} \{ a_{n} \}_{n=0}^{\infty} \subseteq \mathbb{C} {}$ are called the coefficients
### Theorem 1.2: 
For any power series ${} \sum_{n=0}^{\infty} a_{n}(z-z_{0})^{n} {}$ there is a value ${} 0\leq \hat{R}\leq \infty  {}$ such that
- if ${} 0<\hat{R}<\infty  {}$, then the series converges absolutely for those $z$ with ${} |z-z_{0}|<\hat{R} {}$, that is, for all ${} z \in D(z_{0},\, \hat{R}) {}$ and diverges with ${} |z-z_{0}|>\hat{R} {}$
- If ${} \hat{R}=\infty  {}$, then the series converges absolutely for all ${} z \in \mathbb{C} {}$
- If ${} \hat{R}=0 {}$, then the series diverges for $z\neq z_{0}$.

In fact, we have that
$$
\hat{R}=\left( \limsup_{n\tto \infty}  |a_{n}|^{1/n} \right)^{-1}
$$
#### Proof:
Using the nth root test, set ${} w_{n}=a_{n}(z-z_{0})^{n} {}$. Then 
$$
\begin{align}
L & =\limsup_{n\tto \infty} |w_{n}|^{1/n} \\
 & =\limsup_{n\tto \infty} |a_{n}(z-z_{0})|^{1/n} \\
 & =\limsup_{n\tto \infty} |a_{n}|^{1/n} |z-z_{0}| \\
 & =|z-z_{0}|\limsup_{n\tto \infty}|a_{n}|^{1/n} \\ 
 & =\frac{|z-z_{0} |}{\hat{R}} 
\end{align}
$$
and the rest follows trivially from the conditions of the rational root test
#### Remark:
Note that the radius of convergence does not say anything about points on the boundary of the disk
### Corollary 1.3:
Let ${} \hat{R} {}$ be the radius of convergence of ${} \sum_{n=0}^{\infty} a_{n}(z-z_{0})^{n} {}$. Then this series converges uniformly in the closed disk ${} \conj{D(z_{0},\, r)} {}$ for any positive ${} r<\hat{R} {}$.
#### Proof:
#todo find this
### Theorem 1.4:
Assume that ${} a_{n}\neq 0 {}$. If the sequence ${} |a_{n}| / |a_{n+1}| {}$ converges, then ${} \hat{R}=\lim_{n\tto \infty} |a_{n}| / |a_{n+1}| {}$. 
#### Proof:
Let 
$$
C=\lim_{n\tto \infty} \frac{|a_{n}|}{|a_{n+1}|} 
$$
and set
$$
\begin{align}
 w_{ n} & =a_{n}(z-z_{0})^{n}  \\
 L&  =\lim_{n\tto \infty} \frac{|w_{n+1}|}{|w_{n}|}  \\
 & =\lim_{n\tto \infty}  \frac{ |a_{n+1}||z-z_{0}|^{n+1}}{|a_{n}||z-z_{0}|^{n}}  \\
 & =|z-z_{0}| \lim_{n\tto \infty} \frac{|a_{n+1}|}{|a_{n}|} \\
 & =\frac{|z-z_{0}|}{C} 
 \end{align}
$$
As before, for absolute convergence, we need ${} L<1 {}$, that is, ${} |z-z_{0}|<C {}$, and for divergence we need $L>1 {}$, that is, ${} |z-z_{0}|>C {}$.
### Lemma 1.5:
For any ${} k \in \mathbb{N} {}$, the power series ${} \sum_{n=0}^{\infty} a_{n+k}(z-z_{0})^{n} {}$ has the same radius of convergence as ${} \sum_{n=0}^{\infty} a_{n}(z-z_{0})^{n} {}$. 
#### Proof:
Clearly, both series converge for ${} z=z_{0} {}$. Now if $z\neq z_{0}$, then 
$$
\begin{align}
\sum_{n=0}^{\infty} a_{n}(z-z_{0})^{n} & =\sum_{n=0}^{k-1} a_{n}(z-z_{0})+\sum_{n=k}^{\infty} a_{n}(z-z_{0})^{n} \\
 & =\sum_{n=0}^{k-1} a_{n}(z-z_{0})^{n}+(z-z_{0})^{k} \sum_{n=k}^{\infty} a_{n}(z-z_{0})^{n-k} \\
 & =\sum_{n=0}^{k-1} a_{n}(z-z_{0})^{n}+(z-z_{0})^{k} \sum_{n=0}^{\infty} a_{n+k}(z-z_{0})^{k}
\end{align}
$$
and so since the LHS converges, then the RHS converges.
### Lemma 1.6:
Suppose that ${} \{ b_{n} \}_{n=0}^{\infty} \subseteq \mathbb{C} {}$ is a sequence of complex numbers for which there exist ${} C_{1},\, C_{2}>0 {}$ and ${} m_{1},\, m_{2} \in \mathbb{N} {}$, ${} n_{0} \in \mathbb{Z}^{+} {}$ such that
$$
\frac{C_{1}}{n^{m_{1}}} \leq  |b_{n}|\leq C_{2}n^{m_{2}}
$$
for all $n\geq n_{0} {}$. Then the power series ${} \sum_{n=0}^{\infty} b_{n}a_{n}(z-z_{0})^{n} {}$ has the same radius of convergence as ${} \sum_{n=0}^{\infty} a_{n}(z-z_{0})^{n} {}$.
#### Proof:
Note that ${} \lim_{n\tto \infty} n^{1/n}=1 {}$. The conditions of the lemma imply the existence of some $n_{1}>n_{0} {}$ such that
$$
\frac{1}{n^{m_{1}+1}}\leq |b_{n}|\leq  n^{m_{2}+1}
$$
for all $n\geq n_{1}$, and so
$$
\frac{1}{n^{(m_{1}+1)/n}}\leq |b_{n}|^{1/n}\leq n^{(m_{2}-1)/n}
$$
We know that the left and right hand sides converge to $1$ as ${} n\to{}\infty  {}$. Hence, for every $\varepsilon>0 {}$, there exist $n_{\varepsilon}>n_{1} {}$ such that
#todo finish this.
