---
tags:
  - chapter
  - fouranal
date: 2025-01-17
completed: false
---
[[Directory]], [[Fourier Analysis 1|Subject Directory]]
[[1. Introduction and Preliminaries from Real Analysis|ðŸž€ðŸž€]] [[1. Introduction and Preliminaries from Real Analysis|â—€]] [[University/Undergraduate/Second Year/Fourier Analysis/Lectures/3. |â–¶]] [[University/Undergraduate/Second Year/Fourier Analysis/Lectures/22. |ðŸž‚ðŸž‚]]
# 
## Classes of Functions
### Functions on $\mathbb{R} {}$ or on an Interval
The functions we shall be working with will take values in $\mathbb{C} {}$. We shall be working with:
- Continuous functions
- Piecewise continuous functions
- Riemann integrable functions
### Functions on the circle
We denote the unit circle in the complex plane by ${} \mathbb{T} {}$, that is, 
$$
\mathbb{T}=\{ z \in \mathbb{C} \mid  |z|=1 \}=\{ e^{i\theta} \mid  \theta \in  [0,\, 2\pi) \}
$$
Let ${} F: \mathbb{T}\to{}\mathbb{R}  {}$. Then ${} F(e^{i\theta}) {}$ is a $2\pi {}$-periodic function on $\mathbb{R}$, as 
$$
F(e^{i(\theta+2\pi)})=F(e^{i\theta}\cdot e^{i 2\pi})=F(e^{i\theta})
$$
In fact, there is an equivalence between functions on ${} \mathbb{T}$, $2\pi {}$-periodic functions on $\mathbb{R} {}$, and functions on ${} [0,\, 2\pi) {}$.
## Fourier Series
Let $f:\mathbb{R}\to{}\mathbb{C} {}$ which is $L$-periodic, where ${} \mathbb{R}\ni L>0 {}$. We want to represent $f$ as a sum:
$$
f(x)=\sum_{n=-\infty }^{\infty} c_{n} e^{2\pi i \frac{ n x }{ L }}
$$
recall that
$$
e^{2\pi i \frac{nx}{L} }=\cos \left( 2\pi \frac{ nx }{ L } \right)+i \sin \left( 2\pi \frac{ nx }{ L } \right)
$$
but it is more convenient to use the exponential form. We refer to the numbers ${} \frac{2\pi}{L}n {}$ as "frequencies". 

Now, what are ${} c_{n}$? We may find that
$$
c_{n}= \frac{1}{L} \int_{0}^{L} f(x)e^{-i \frac{ 2\pi }{ L }nx} \ud x 
$$
These are the $n^{\text{th}} {}$ Fourier coefficient. We will also need to prove that 
$$
\sum_{n=-N}^{N} c_{n} e^{i \frac{ 2\pi }{ L }nx} \longrightarrow f(x)
$$
as ${} N\to{}\infty  {}$. Also note that ${} f(x)e^{-i \frac{ 2\pi }{ L }nx} {}$ is $L$ periodic, so the Fourier coefficients may be integrated over any interval of length $L$. Therefore, it is simpler to integrate from $0$. 

From now on, ${} L=2\pi {}$. Now write
$$
\begin{align}
f(x) & =\sum_{n=-\infty }^{\infty} \hat{f_{n}} e^{inx} \\
\hat{f_{n}}  & =\frac{1}{2\pi} \int_{-\pi}^{\pi} f(x)e^{-inx} \ud x 
\end{align}
$$
Why do we use this formula to generate these coefficients? Let us do a simple calculation:
$$
I(n)=\frac{1}{2\pi} \int_{-\pi}^{\pi} e^{inx} \ud x 
$$If ${} n=0 {}$, then ${} I(n)=1 {}$. Otherwise, if $n\neq 0$, then ${} I(n)=0 {}$. 
### Trigonometric Polynomials
Trigonometric polynomials are finite sums of the form:
$$
\sum_{m=a}^{b} a_{m} e^{imx}
$$
Suppose that $f$ is a trigonometric polynomial. Let us compute ${} \hat{f_{n}} {}$; we want to show that ${} \hat{f_{n}}=a_{n} {}$ for $a\leq n\leq b {}$, and $0$ otherwise. Now
$$
 \begin{align}
 \hat{f_{n}} & =\frac{1}{2\pi} \int_{-\pi}^{\pi } \left( \sum_{m=a}^{b} a_{m} e^{imx} \right) \cdot e^{-inx} \ud x    \\
 & = \sum_{m=a}^{b} \frac{1}{2\pi}\int_{-\pi}^{\pi} a_{m} e^{im x} \cdot e^{-inx} \ud x  \\
 & =\sum_{m=a}^{b} a_{m} \frac{1}{2\pi} \int_{-\pi}^{\pi} e^{i(n-m)x} \ud x  \\
 & =\begin{cases}
a_{m}  & ,a\leq n\leq b \\
0 & ,\text{ otherwise}
\end{cases}
 \end{align}
$$
#### Example:
Consider $f(\theta)=\theta {}$ for ${} \theta \in [-\pi,\, \pi) {}$. We compute the Fourier coefficients:
$$
\hat{f_{n}}=\frac{1}{2\pi} \int_{-\pi}^{\pi} x e^{-inx} \ud x 
$$
We have 2 cases: ${} n=0 {}$
$$
\hat{f_{0}}=\int_{-\pi}^{\pi} x \ud x =0
$$
and $n\neq 0$. Then
$$
\begin{align}
2\pi \hat{f_{0}} & =\int_{-\pi}^{\pi} xe^{-inx} \ud x    \\
 & =\left.-\frac{x}{in}e^{-inx}\right|_{x=-\pi}^{\pi}+\frac{1}{in} \int_{-\pi}^{\pi} e^{-inx} \ud x  \\
 & =-\frac{\pi}{in}e^{-i\pi x}+\frac{\pi}{in}e^{i\pi x} \\
 & =-\frac{2\pi}{in}(-1)^{n} \\
 & =\frac{i}{n}2\pi (-1)^{n}
 \end{align}
$$
and so
$$
\begin{align}
 f(\theta) & =\sum_{n=-\infty }^{\infty} \frac{i}{n}(-1)^{n} e^{in\theta}   \\
 & =\sum_{n=1}^{\infty} \frac{i}{n}(-1)^{n} e^{in\theta}-\frac{i}{n}(-1)^{-n}e^{in\theta} \\
 & =\sum_{n=1}^{\infty} \frac{i}{n}(-1)^{n} e^{in\theta}-e^{-in\theta} \\
 & =\sum_{n=1}^{\infty} \frac{2}{n}(-1)^{n+1}\sin (n\theta)
 \end{align}
$$
#### Example:
Consider ${} f(\theta)=\frac{(\theta-\pi)^{2}}{4} {}$ for ${} 0\leq \theta<2\pi {}$. Exercise: #todo show that
$$
f(\theta)=\frac{\pi^{2}}{12}+\sum_{n=1}^{\infty} \frac{ \cos n\theta }{ n^{2} }
$$
#### Example: The Dirichlet Kernel
Define
$$
D_{N}(\theta) =\sum_{n=-N}^{N}  e^{in\theta}
$$
This is a simple Fourier series where
$$
\hat{f_{n}}=\begin{cases}
1, & |n|\leq N \\
0, & |n|>N
\end{cases}
$$
We may express ${} D_{N} {}$ as 
$$
D_{N}(x)=\frac{\sin \left( \left( N+\frac{1}{2} \right)x \right)}{\sin \left( \frac{x}{2} \right)} 
$$
as we will now show. Let ${} \omega=e^{i\theta} {}$. Then 
$$
\sum_{n=0}^{N} e^{in\theta}=\sum_{n=0}^{N} \omega^{n}=\frac{ 1-\omega^{N+1} }{ 1-\omega }
$$
and 
$$
\sum_{n=-N}^{0} e^{in\theta}=\sum_{n=0}^{N} e^{-in\theta}=\frac{ 1-\conj{\omega}^{N+1} }{ 1-\conj{\omega} }
$$
so
$$
\begin{align}
 D_{N}(\theta) & =\frac{ 1-\omega^{N+1} }{ 1-\omega }+\frac{ 1-\conj{\omega}^{N+1} }{ 1-\conj{\omega} }-1   \\
 & =\frac{1-e^{i(N+1)\theta}}{1-e^{i\theta}} +\frac{1-e^{-i(N+1)\theta}}{1-e^{-i\theta}}-1 \\
 & =\frac{1-e^{i(N+1)\theta}}{1-e^{i\theta}}-\frac{e^{i\theta}-e^{-iN\theta}}{1-e^{i\theta}}-1 \\
 & =\frac{1-e^{i(N+1)\theta}-e^{i\theta}+e^{-iN\theta}-1+e^{i\theta}}{1-e^{i\theta}}  \\
 & =\frac{e^{-iN\theta}-e^{i(N+1)\theta}}{1-e^{i\theta}}  \\
 & =\frac{e^{-i(N+1/2)\theta}-e^{-i(N+1/2)\theta}}{e^{i\theta/2}-e^{-i\theta/2}}  \\
 & =\frac{\sin \left( \left( N+\frac{1}{2} \right)\theta \right)}{\sin \left( \frac{\theta}{2} \right)} 
 \end{align}
$$
as required. (Phew)