---
tags:
  - chapter
  - fouranal
date: 2025-01-24
completed: true
---
[[Directory]], [[Fourier Analysis 1|Subject Directory]]
[[1. Introduction and Preliminaries from Real Analysis|ðŸž€ðŸž€]] [[University/Undergraduate/Second Year/Fourier Analysis/Lectures/3. |â—€]] [[University/Undergraduate/Second Year/Fourier Analysis/Lectures/5. |â–¶]] [[University/Undergraduate/Second Year/Fourier Analysis/Lectures/22. |ðŸž‚ðŸž‚]]
# Convergence
Let $f {}$ be Riemann integrable on ${} [-\pi,\, \pi] {}$. Define
$$
\hat{f_{n}}=\frac{1}{2\pi} \int_{-\pi}^{\pi} f(\theta) e^{-in\theta}\ud \theta
$$
for ${} n \in \mathbb{Z} {}$. Then is it true that
$$
f(\theta)=\sum_{n=-\infty }^{\infty} \hat{f_{n}}e^{in\theta}
$$
in other words, if 
$$
S_{N}=\sum_{n=-N}^{N} \hat{f_{n}} e^{in\theta}
$$
then does
$$
S_{N}(\theta)\to{}f(\theta)
$$
as ${} N\to{}\infty  {}$. 
#### Example:
${} f(0)=1 {}$ and ${} f(x)=0 {}$ for $x\neq 0 {}$. Then the Fourier coefficients are all $0 {}$, and so $f {}$ cannot be reconstructed from it's Fourier coefficients

Suppose that $f {}$ is continuous at $0 {}$. Is ${} f(0) {}$ uniquely defined by ${} \{\hat{f_{n}}\}_{n=-\infty }^{\infty } {}$. The answer is yes, as will be shown. 
### Theorem 1.1: Uniqueness of Fourier Series
If $f {}$ is continuous at ${} \bar{\theta} {}$, and ${} \hat{f_{n}}=0 {}$ for all ${} n \in \mathbb{Z} {}$, then ${} f(\bar{\theta})=0 {}$.
#### Remark:
Suppose we have ${} f,\, g {}$ are both continuous at $\theta {}$, and ${} \hat{f_{n}}=\hat{g_{n}} {}$. Then define ${} h=f-g {}$, and so ${} \hat{h_{n}}=0 {}$. Then the above theorem implies that ${} f=g {}$ at $\theta {}$. 
#### Proof:
#todo read full proof in lecture notes. Later in the course, we will have a more general theorem from which this will follow. 

We know that
$$
\hat{f_{n}}=\int_{-\pi}^{\pi} f(\theta)e^{-in\theta} \ud \theta=0 
$$
In particular, 
$$
\int_{-\pi}^{\pi} f(\theta)\cos (n\theta) \ud \theta=0 
$$
Idea: Assume that ${} f(\bar{\theta})\neq 0 {}$, and bring this to a contradiction. For now, assume that $f {}$ is real, as we can always break into real and imaginary parts. 

WLOG, assume that ${} f(\bar{\theta })>0 {}$. By multiplying $f {}$ by a suitable factor, we may assume that ${} f(\bar{\theta })=2 {}$. Then there exists some interval, say ${} [-\eta,\, \eta] {}$ such that $f>1 {}$ on ${} [-\eta,\, \eta] {}$. 

Take some small $\varepsilon>0 {}$ and a large ${} k \in \mathbb{N} {}$. Consider 
$$
\int_{-\pi}^{\pi} f(\theta) (\varepsilon+\cos \theta)^{k} \ud \theta 
$$
By assumption, this integral must be zero, as otherwise the ${} \hat{f_{n}} {}$ would be positive. O the other hand, estimates show that (by choosing a sufficiently large $k {}$ and sufficiently small $\varepsilon {}$), then the integral can be made positive. Therefore, this is a contradiction. 

Now if $f {}$ is complex valued, then we split it into real and imaginary parts. 
### Corollary 1.2:
Let ${} f {}$ be continuous such that 
$$
 \sum_{n=-\infty }^{\infty} |\hat{f_{n}}|<\infty 
$$
Then $f {}$ is uniquely defined by it's Fourier coefficients. 

Alternatively, let $f {}$ be a continuous $2\pi {}$-periodic function such that 
$$
\sum_{n=-\infty }^{\infty } |\hat{f_{n}}|<\infty 
$$
then 
$$
S_{N}(\theta)\to{}f(\theta)
$$
as ${} N\to{}\infty  {}$ uniformly in $\theta {}$.
#### Proof:
Consider
$$
\sum_{n=-\infty }^{\infty} \hat{f_{n}} e^{i\theta}
$$
Then notice that
$$
|\hat{f_{n}}e^{i\theta}|=|\hat{f_{n}}|
$$
This is the condition of the Weierstrass ${} M {}$-test, and by it, ${} S_{N}(\theta)\to{}g(\theta) {}$ uniformly in $\theta {}$. Moreover, $g {}$ is continuous. Now let
$$
\begin{align}
 \hat{g_{m}} & =\frac{1}{2\pi} \int_{-\pi}^{\pi} g(\theta)e^{-im\theta} \ud \theta \\
 & =\lim_{N\tto \infty} \frac{1}{2\pi} \int_{-\pi}^{\pi} S_{N}(\theta)e^{-im\theta} \ud \theta   \\
 & =\lim_{N\tto \infty} \frac{1}{2\pi}\int_{-\pi}^{\pi} \left( \sum_{n=-N}^{N} \hat{f_{n}} e^{in\theta} \right) e^{-im\theta} \ud \theta \\
 & =\hat{f_{m}}
 \end{align}
$$
and so by the above theorem, then ${} f=g$.
### Theorem 1.3:
Let $f$ be a $2\pi {}$-periodic function which is twice continuously differentiable. Then ${} \hat{f_{n}}=O\left( \frac{1}{n^{2}} \right) {}$ as ${} |n|\to{}\infty  {}$ and in particular ${} \sum_{n=-\infty }^{\infty} |\hat{f_{n}}|< \infty  {}$
#### Proof:
We have that
$$
\begin{align}
 \hat{f_{n}} & =\frac{1}{2\pi} \int_{-\pi}^{\pi} f(\theta) e^{-in\theta} \ud \theta  \\
 & = -\frac{1}{2\pi} \frac{1}{in}\int_{-\pi}^{\pi} f(\theta)(e^{in\theta})' \ud \theta  \\
 & =-\frac{1}{2\pi} \frac{1}{in}\left.f(\theta)e^{-in\theta}\right|_{-\pi}^{\pi}+\frac{1}{2\pi} \frac{1}{in} \int_{-\pi}^{\pi} f'(\theta)e^{-in\theta} \ud \theta \\

 \end{align}
$$
and we have that
$$
\begin{align}
\left.f(\theta)e^{-in\theta}\right|_{-\pi}^{\pi} & =f(\pi)e^{-in\pi}-f(-\pi)e^{in\pi} \\
 & =(-1)^{n}(f(\pi)-f(-\pi)) \\
 & =0
\end{align}
$$
so now
$$
\hat{f_{n}}=\frac{1}{2\pi} \frac{1}{in} \int_{-\pi}^{\pi} f'(\theta)e^{-in\theta} \ud \theta =\frac{1}{in} \hat{f_{n}'}
$$
and likewise ${} \hat{f_{n}'}=\frac{1}{in} \hat{f_{n}''} {}$. Therefore, ${} \hat{f_{n}}=\frac{1}{n^{2}}\hat{f''_{n}} {}$. Now we have that ${} \hat{f_{n}''} {}$ is bounded, as 
$$
\hat{f_{n}''}=\frac{1}{2\pi} \int_{-\pi}^{\pi} f''(\theta)e^{-in\theta} \ud \theta \Rightarrow |\hat{f_{n}''}|\leq \frac{1}{2\pi} \int_{-\pi}^{\pi} |f''(\theta)| \ud \theta=C
$$
and so ${} \hat{f_{n}}\leq  \frac{1}{n^{2}}C {}$.
### Remark:
For uniform convergence of a Fourier series, it suffices to assume that $f$ is once continuously differentiable. Even better, it suffices to assume Lipschitz continuity of $f {}$.
# Convolutions
## Introduction
### Definition 2.1: Convolutions
Let ${} f$ and $g$ be $2\pi {}$-periodic Riemann Integrable functions. Their *convolution*, ${} f *g {}$ is defined as
$$
(f*g)(x)=\frac{1}{2\pi} \int_{-\pi}^{\pi} f(y)g(x-y) \ud y 
$$

Why do we care? Given a $2\pi {}$-periodic function $f$, we define as usual
$$
f \to{} \hat{f_{n}}= \frac{1}{2\pi} \int_{-\pi}^{\pi} f(y)e^{-iny} \ud y 
$$
and
$$
S_{n}(x)=\sum_{n=-N}^{N} \hat{f_{n}} e^{inx}
$$
so
$$
\begin{align}
 S_{N}(x) & =\sum_{n=-N}^{N} \frac{1}{2\pi} \int_{-\pi}^{\pi} f(y) e^{-iny} e^{inx}\ud y    \\
 & =\frac{1}{2\pi} \int_{-\pi}^{\pi} f(y)  \sum_{n=-N}^{N} e^{in(x-y)}\ud x  \\
 & =(f *D_{N} )(x)
 \end{align}
$$
where ${} D_{N}$ is the ${} N^{\text{th}} {}$ Dirichlet kernel.
### Remark
Let $F$ be $2\pi {}$-periodic. Then 
$$
\int_{-\pi}^{\pi} F(x) \ud x =\int_{-\pi}^{\pi} F(x-a) \ud x  \qquad \forall a \in \mathbb{R}
$$
