---
tags:
  - chapter
  - fouranal
date: 2025-02-03
completed: false
---
[[Directory]], [[Fourier Analysis 1|Subject Directory]]
[[1. Introduction and Preliminaries from Real Analysis|ðŸž€ðŸž€]] [[University/Undergraduate/Second Year/Fourier Analysis/Lectures/6. |â—€]] [[University/Undergraduate/Second Year/Fourier Analysis/Lectures/8. |â–¶]] [[University/Undergraduate/Second Year/Fourier Analysis/Lectures/22. |ðŸž‚ðŸž‚]]
# Summation
## Methods
### Cesaro Average 
Let ${} \{ x_{k} \}_{k=0}^{\infty }  {}$ be a sequence of numbers, and let ${} S_{n}=\sum_{k=0}^{n-1} x_{k} {}$. Then ${} \sigma_{N}=\frac{1}{N} \left( \sum_{N=0}^{N-1} S_{n} \right) {}$, and so
$$
\begin{align}
 \sigma_{N} & =\frac{1}{N}(x_{0}+(x_{0}+x_{1})+(x_{0}+x_{1}+x_{2})+\dots+(x_{0}+\dots+x_{N-1}))   \\
 & =x_{0}+\frac{N-1}{N} x_{1}+\dots+\frac{1}{N}x_{N-1}
 \end{align}
$$
This gives "weights" in front of each term. 
### Abel Average
Let ${} A(r)=\sum_{k=0}^{\infty }r^{k} x_{k}  {}$ with ${} 0<r<1 {}$. This again gives weights in front of the ${} x_{k}$. Now to find the sum, let ${} r \to{}1 {}$. 

Now we get that 
$$
 \left\{  \text{summable}  \right\} \subset \{ \text{Cesaro summable} \} \subset  \{ \text{Abel summable} \}
$$
#### Example:
There are series that are Abel summable that are not Cesaro summable. First, we get that
$$
\frac{1}{1+r}=\sum_{k=0}^{\infty} (-1)^{k} r^{k}=1-r+r^{2}-r^{3}+\dots{}
$$
Then 
$$
\frac{d}{dr} \frac{1}{1+r}=-\frac{1}{(1+r^{2})}=\sum_{k=0}^{\infty} (-1)^{k}kr^{k-1}=\sum_{k=0}^{\infty} (-1)^{k+1} (k+1) r^{k}
$$
or
$$
\frac{1}{1+r^{2}}=\sum_{k=0}^{\infty} (-1)^{k}(k+1)r^{k}
$$
Consider the Abel summation of
$$
\sum_{k=0}^{\infty} (-1)^{k} (k+1)=1-2+3-4+5-6+\dots \phantom{+}
$$
You can check that the Cesaro average also diverges.( #todo)
However, the Abel average converges; in particular, ${} A(r)=\frac{1}{(1+r)^{2}}\to{}\frac{ 1 }{  4} {}$ as ${} r\to{}1 {}$. 
### Abel Summation of Fourier Series
We may write
$$
\sum_{n=-\infty }^{\infty } \hat{f_{n}} e^{in\theta}=\hat{f_{0}}+(\hat{f_{1}}e^{i\theta}+\hat{f_{-1}}e^{-i\theta })+(\hat{f_{2}}e^{2i\theta}+\hat{f_{-2}}e^{-2i\theta})+\dots \phantom{+}
$$
And so
$$
A(r)=\sum_{n=-\infty }^{\infty} \hat{f_{n}}r^{|n|} e^{in\theta}
$$
Why does this converge?
Recall that $f$ is Riemann integrable. Therefore, 
$$
f\to{}\hat{f_{n}}=\frac{1}{2\pi} \int_{-\pi}^{\pi} f(\theta)e^{-in\theta} \ud x 
$$
and so
$$
|\hat{f_{n}}|\leq  \frac{1}{2\pi} \int_{-\pi}^{\pi} |f(\theta)| \ud x  
$$
and so 