---
tags:
  - classical_dynamics
  - chapter
date: 2024-01-16
---
[[Directory]], [[Intro to Dynamical Systems 1|Subject Directory]]
# First order ODEs
## Homogenous
### Definition 1.1: Homogenous Functions
What is a homogeneous function? If we have a multivariable function ${} F:\mathbb{R}^{n}\to{}\mathbb{R} {}$ with
$$
F(\lambda x_{1},\, \lambda x_{2},\,\dots,\,\lambda x_{n})=\lambda^{d} F(x_{1},\, x_{2},\,\dots,\,x_{n})
$$
We say that the function is homogenous of degree ${} d$.
#### Example: 
$$
f(x,\, y,\, z)=x+y+2z
$$
is a homogenous function, as
$$
f(\lambda x,\, \lambda y,\, \lambda z)=\lambda x+\lambda y+2\lambda z = \lambda(x+y+2z )=\lambda  f(x,\, y,\, z)
$$
and it is of degree 1
#### Example:
$$
f(x,\, y,\, z)=x^{2}+yz
$$
is a homogenous function as
$$
\begin{align}
f(\lambda x,\, \lambda y,\, \lambda z) & =\lambda^{2}x^{2}+\lambda \lambda yz \\
 & =\lambda^{2}(x^{2}+yz) \\
 & =\lambda^{2} f(x,\, y,\, z)
\end{align}
$$
and it is of degree 2
#### Non-Example:
$$
f(x,\, y,\, z)=x+y+1
$$
is *not* homogenous as, 
$$
\begin{align}
f(\lambda x,\, \lambda y,\, \lambda z)=\lambda x+\lambda y+1 \neq \lambda x+\lambda y+\lambda=\lambda(x+y+1)=\lambda f(x,\, y,\, z)
\end{align}
$$
### Definition 1.2
An ODE is homogenous if
$$
\frac{dx}{dt} =f(x,\, t)
$$
where ${} f {}$ is homogenous in degree 0, that is, 
$$
f(\lambda x,\, \lambda t)=f(x,\, t)
$$
we can write it as a function of ${} x/t {}$ and
$$
\frac{dx}{dt} =G\left( \frac{x}{t} \right)
$$
We can solve these with substitution
### How to solve an equation of the above form
We write 
$$
\frac{x}{t}=v,\, \qquad x=vt
$$
so
$$
\frac{dx}{dt}=G(v)\Rightarrow \frac{d(vt)}{dt} =G(v)
$$
and we have
$$
\frac{d(vt)}{dt} =v+t\frac{dv}{dt} 
$$
so
$$
v+t \frac{dv}{dt}=G(v)
$$
and finally
$$
\frac{dv}{dt}=\frac{ G(v)-v }{ t }
$$
and this is separable. Finally, we solve this separable equation
$$
\int \frac{1}{G(v)-v} \ud v=\int \frac{1}{t} \ud v  
$$
Once solved, this will give a function in terms of $v {}$ that is a solution, in particular, $v(t) {}$. However, we want ${} x(t) {}$, not ${} v(t) {}$, so we must solve 
$$
x(t)=tv(t)
$$
#### Example:
$$
\frac{dx}{dt} =\frac{x^{2}-t^{2}}{2xt} 
$$
This is not direct or separable, so we check if it is homogenous of degree 0. Note that 
$$
\frac{\lambda^{2} x^{2}-\lambda^{2} t^{2}}{\lambda^{2}2xy} =\frac{x^{2}-t^{2}}{2xy} 
$$
so it is homogenous of degree 0. Now we want to find ${} G(v) {}$. In particular, we want to write it in terms of ${} x/t {}$, as follows:
$$
\frac{ x^{2}-t^{2} }{ 2xt }=\frac{ \left( \frac{x}{t} \right)^{2}-1 }{ 2\frac{x}{t} }=\frac{v^{2}-1}{2v} =G(v)
$$
Now
$$
\frac{dx}{dt} =\frac{d(vt)}{dt}=v+t\frac{dv}{dt}  
$$
so
$$
v+t \frac{dv}{dt} = \frac{v^{2}-1}{2v} 
$$
We now separate the variables:
$$
t\frac{dv}{dt}= \frac{ v^{2}-1 }{ 2v }-v
$$
$$
\left( \frac{v^{2}-1}{2v} -v \right)^{-1} \frac{dv}{dt} =\frac{1}{t}
$$
$$
 \int  \left( \frac{v^{2}-1}{2v} -v \right)^{-1} \ud v =\int\frac{1}{t} \ud t
$$
if we solve this integral, we find that
$$
\begin{align}
 \ln(v^{2}+1) & =-\ln |t|+C   \\
 \ln(|t|(v^{2}+1)) & =C \\
|t|(v^{2}+1) & =e^{C}=A,\, \qquad A>0 \\
 \end{align}
$$
Resubstituting we get. Since $A>0 {}$, we can move the $\pm {}$ from the absolute value from the ${} t$ to the ${} A {}$, so now $A\neq 0 {}$.
$$
\begin{align}
 t\left( \frac{x^{2}}{t^{2}}+1 \right) & =A   \\
x^{2}+t^{2} & =At \\
x & =\pm\sqrt{At-t^{2}}
 \end{align}
$$
Now if we fiddle with the equation, we can get a circle. In particular
$$
\begin{align}
x^{2}+t^{2}-At+\left( \frac{A}{2} \right)^{2} &  =\left( \frac{A}{2} \right)^{2} \\
x^{2}+\left( t-\frac{A}{2} \right)^{2} & =\left( \frac{A}{2} \right)^{2}
\end{align}
$$
## Linear
(these are still first order)
### Definition 1.3: Linear ODE
A linear ODE is an ODE of the form
$$
\frac{dx}{dt} =f(t)x+g(t)
$$
### Linear Map
If a map ${} L(x)$ is linear, then 
$$
L(\alpha x_{1}+\beta x_{2})=\alpha L(x_{1})+\beta L(x_{2})
$$
Note that ${} \frac{dx}{dt} -f(t)x {}$ is a linear map in $x$. In particular, 
$$
\begin{align}
 L(\alpha x_{1}+\beta x_{2}) & =\frac{d}{dt} (\alpha x_{1}+\beta x_{2})-f(t)(\alpha x_{1}+\beta x_{2})  \\
 & = \alpha  \frac{dx_{1}}{dt} +\beta  \frac{dx_{2}}{dt}-\alpha f(t)x_{1} - \beta f(t)x_{2} \\
 & =\alpha\left(  \frac{dx_{1}}{dt} -f(t)x_{1} \right)+\beta\left(  \frac{dx_{2}}{dt}-f(t)x_{2} \right) \\
 & =\alpha L(x_{1})+\beta L(x_{2})
 \end{align}
$$