---
tags:
  - dynamical_systems1
  - chapter
date: 2024-01-19
---
[[Directory]], [[Intro to Dynamical Systems 1|Subject Directory]]
[[2. Homogenous and First Order ODEs|Last]] ;; [[ |Next]]
# ODEs
## Linear ODES
### General form
We have ${} f,\, g,\, x {}$ as functions of $t$. A linear ODE is of the form
$$
\frac{dx}{dt} -fx=g
$$
If we multiply by a function ${} \mu=\mu(t) {}$, we get
$$
\mu \frac{dx}{dt} -\mu fx=\mu g
$$
Now note that 
$$
\frac{d(\mu x)}{dt} =\mu \frac{dx}{dt}  + x \frac{d\mu}{dt}
$$
So we can add $0$  on our original equation like so
$$
\mu \frac{dx}{dt} +x \frac{d\mu}{dt} - x \frac{d\mu}{dt}-\mu fx=\mu g
$$
and we get
$$
\frac{d(\mu x)}{dt}-x\left( \frac{d\mu}{dt}-\mu f \right)=\mu g
$$
We can pick $\mu$ (as will be shown later) such that
$$
\frac{d\mu}{dt}+\mu f=0
$$
and so we simply get
$$
\frac{d(\mu x)}{dt}=\mu g
$$
This is an *explicit* equation, as $\mu g$ only depends on $t$. Therefore
$$
\begin{align}
 \mu x & =\int \mu g \ud t   \\
 & =\Gamma(t)+C \\
x & =\frac{\Gamma+C}{\mu}
 \end{align} 
$$
Now we find $\mu$. Recall that we pick $\mu$ such that
$$
\frac{d\mu}{dt}+\mu f=0
$$
so
$$
\begin{align}
 \frac{d\mu}{dt} & =-\mu f \\
\frac{1}{\mu} \frac{d\mu}{dt} & =-f  \\
\int \frac{1}{\mu} \ud \mu & =-\int f \ud t   \\
\ln |\mu|+C & =-\int f(t) \ud t 
 \end{align}
$$
so
$$
\mu(t)=\exp\left( -\int f(t) \ud t  +C\right)
$$
(don't ask me where the absolute values went). We generally pick $C$ to be $0$, as we just need *a* $\mu$ that satisfies the equation, and ${} C=0 {}$ is (usually) simpler
#### Example:
$$
t(t+1) \frac{dx}{dt} -(t+2)x=t^{3}(2x-3)
$$
We *bring it to the linear form*, that is, 
$$
\frac{dx}{dt} -\frac{t+2}{t(t+1)}x=\frac{t^{3}(2t-3)}{t(t+1)}=\frac{t^{2}(2t-3)}{t+1}
$$
Note that
$$
f(t)=\frac{ t+2 }{ t(t+1) }\qquad g(t)=\frac{ t^{2}(2t-3) }{ t+1 }
$$
We now find $\mu$. We have
$$
\begin{align}
 \mu(t) & =\exp\left( -\int \frac{ t+2 }{ t(t+1) } \ud t  \right)  \\
 & = \exp\left( -\left( \int \frac{2(t+1)}{t(t+1)}dt-\int  \frac{t}{t(t+1)} \ud t  \right) \right) \\
 & =\exp\left( -\left( \int \frac{2}{t} \ud t -\int \frac{1}{t+1} \ud t  \right) \right) \\
 & =\exp(-(2\ln(t)-\ln(t+1))) \\
 & =\exp(\ln(t+1)+\ln(t^{-2})) \\
 & =\exp\left( \ln\left( \frac{ t+1 }{ t^{2} } \right) \right) \\
 & =\frac{ t+1 }{ t^{2} }
 \end{align}
$$
Finally, we find $x$. Recall that
$$
\begin{align}
 x(t) & =\frac{1}{\mu(t)} \int \mu(t)g(t) \ud t  \\ \\
 & =\frac{t^{2}}{t+1} \int \frac{t+1}{t^{2}} \cdot  \frac{t^{2}(2t-3)}{t+1}  \ud t  \\
 & = \frac{t^{2}}{t+1} \int 2t-3 \ud t \\
 & =\frac{t^{2}}{t+2}(t^{2}-3t+C)
 \end{align}
$$

