# II. Formulas
1. 
$$
\Int(X\cap Y)=\Int(X) \cap \Int(Y)
$$
##### Proof:
$$
\begin{align}
\Int(X \cap Y) & =1-\conj{1-X\cap Y} \\
  & =1-\conj{(1-X)\cup (1-Y)} \\
 & =1-\conj{1-X} \cup \conj{1-Y} \\
	 & =(1-\conj{1-X}) \cap (1-\conj{1-Y}) \\
 & =\Int(X) \cap \Int(Y)
\end{align}
$$
2. 
$$
\bigcup_{\iota}\Int(X_{\iota})\subseteq \Int\left( \bigcup_{\iota} X_{\iota} \right)
$$
##### Proof:
$$
\begin{align}
\bigcup_{\iota}\Int(X_{i}) & =\bigcup_{\iota}1-\conj{1-X_{\iota}}  \\
 & =1-\bigcap_{\iota} \conj{1-X_{\iota}} \\
 & \subseteq 1-\conj{\bigcap_{\iota} 1-X_{\iota}} \\
 & =1-\conj{1-\bigcup_{\iota}X_{\iota}} \\
 & =\Int\left( \bigcup_{\iota} X_{\iota} \right)
\end{align}
$$
3. 
$$
\Int(X)=X-\conj{1-X}=X-\Fr(X)\subseteq X
$$
##### Proof:
$$
\begin{align}
\Int(X) & =1-\conj{1-X} \\
1-\conj{1-X}\subseteq 1-1-X=X\Rightarrow \qquad  & =X \cap(1-\conj{1-X}) \\
 & =X-\conj{1-X} \\
 & =X-(X \cap \conj{1-X}) \\
 & =X-(\conj{X} \cap X \cap  \conj{1-X}) \\
 & =X-(\Fr(X) \cap X) \\
 & =(X-\Fr(X)) \cup(X-X) \\
 & =X-\Fr(X)
\end{align}
$$
4. 
$$
\Fr(1-X)=\Fr(X)
$$
##### Proof:
$$
\begin{align}
 \Fr(1-X)  & = \conj{1-X} \cap\conj{(1-(1-X))} \\
	 & =\conj{X} \cap  \conj{1-X} \\
	 & =\Fr(X)
 \end{align}
$$
5. 
$$
\Fr(\conj{X}) \subseteq  \Fr(X)
$$
##### Proof:
$$
\begin{align}
\Fr(\conj{X}) & =\conj{1-\conj{X}} \cap \conj{\conj{X}} \\
 & =\conj{\conj{1}-\conj{X}} \cap \conj{X} \\
 & \subseteq \conj{1-X} \cap \conj{X} \\
 & = \Fr(X)
\end{align}
$$
Counterexample against equality: ${} \conj{\mathbb{Q}}=\mathbb{R} {}$, and ${} \Fr(\mathbb{Q})=\mathbb{R} {}$, but ${} \Fr(\conj{\mathbb{Q}})=0 {}$
6. 
$$
\Fr(X)=(X \cap \conj{1-X}) \cup(\conj{X}-X)
$$
##### Proof:
$$
\begin{align}
	\Fr(X) & =\conj{X} \cap \conj{1-X} \\
 & =((\conj{X} -X )\cup X)\cap \conj{1-X} \\
	 & =(X \cap \conj{1-X}) \cup((\conj{X}-X)\cap \conj{1-X}) \\
\conj{X}-X\subseteq 1-X\subseteq \conj{1-X}\Rightarrow \qquad  & =(X \cap \conj{1-X}) \cup(\conj{X}-X)
\end{align}
$$
7. 
$$
X \cup \Fr(X)=\conj{X}
$$
##### Proof:
$$
\begin{align}
X \cup \Fr(X) & =X \cup(X \cap \conj{1-X})\cup(\conj{X}-X) \\
 & =\conj{X} \cup(X \cap \conj{1-X}) \\
X \subseteq \conj{X}\Rightarrow X \cap \conj{1-X} \subseteq \conj{X} \Rightarrow \qquad  & =\conj{X}
\end{align}
$$
8. 
$$
\Fr(X) \cup \Fr(Y)=\Fr(X \cup Y) \cup \Fr(X \cap Y) \cup (\Fr(X ) \cap \Fr(Y))
$$
##### Proof:
$$
\begin{align}
\Fr(X \cup Y)  & =\conj{X \cup Y} \cap \conj{1-X \cup Y} \\
 & =(\conj{X}\cup \conj{Y}) \cap \conj{(1-X) \cap (1-Y)} \\
 & \subseteq (\conj{X} \cup \conj{Y}) \cap (\conj{1-X} \cap \conj{1-Y}) \\
 & =(\conj{X} \cap(\conj{1-X}) \cap\conj{(1-Y)})\cup (\conj{Y} \cap(\conj{1-X}) \cap\conj{(1-Y)}) \\
 & \subseteq (\conj{X} \cap \conj{1-X}) \cup(\conj{Y} \cap \conj{1-Y}) \\
 & =\Fr(X) \cup \Fr(Y)
\end{align}
$$
and
$$
\begin{align}
 \Fr(X \cap Y) & =  \conj{X \cap Y} \cap \conj{1-X \cap Y} \\
 & =\conj{X \cap Y} \cap \conj{(1-X) \cup (1-Y)} \\
 & \subseteq \conj{X} \cap \conj{Y} \cap(\conj{1-X} \cup \conj{1-Y}) \\
 & = (\conj{X} \cap \conj{Y} \cap \conj{1-X}) \cup(\conj{X} \cap \conj{Y} \cap \conj{1-Y}) \\
 & \subseteq (\conj{X} \cap \conj{1-X}) \cup(\conj{Y} \cap \conj{1-Y}) \\
 & =\Fr(X) \cup \Fr(Y) 
 \end{align}
$$
so
$$
\Fr(X \cup Y) \cup \Fr( X \cap Y) \cup(\Fr(X) \cap \Fr(Y)) \subseteq  \Fr(X) \cup \Fr(Y)
$$
I'm not doing the other side fuck that shit
9. 
$$
\Int(\Int(X))=\Int(X)
$$
##### Proof:
$$
\begin{align}
\Int(\Int(X)) & =1-\conj{1-(1-\conj{1-X})} \\
 & =1- \conj{\conj{1-X}} \\
 & =1-\conj{1-X} \\
	 & =\Int(X)
\end{align}
$$
10. 
$$
\Fr(\Fr(\Fr(X)))=\Fr(\Fr(X))
$$
##### Proof:
$$
\begin{align}
\Fr(\Fr(\Fr(X)))
\end{align}
$$