---
tags:
  - chapter
  - alggeo
date: 2025-02-07
completed: false
---
[[Directory]], [[Algebraic Geometry 1|Subject Directory]]
[[University/Undergraduate/Second Year/Algebraic Geometry/Lectures/1. |ðŸž€ðŸž€]] [[University/Undergraduate/Second Year/Algebraic Geometry/Lectures/3. |â—€]] [[University/Undergraduate/Second Year/Algebraic Geometry/Lectures/5. |â–¶]] [[University/Undergraduate/Second Year/Algebraic Geometry/Lectures/11. |ðŸž‚ðŸž‚]]
# 
## 
### Lemma 1.1:
Let $K$ be an algebraically closed field of characteristic $p>3 {}$, and let ${} \lambda \in K -\{ 0,\, 1 \} {}$. Let ${} \phi(t),\, \psi(t) \in K(t) {}$, and suppose that ${} \psi(t)^{2}=\phi(t)(\phi(t)-1)(\phi(t)-\lambda) {}$, then ${} \varphi(t),\, \psi(t) \in K {}$ (i.e. are constant)
#### Proof:
If ${} \phi(t) \in K {}$, then ${} \psi(t) \in K {}$. We may write
$$
\phi(t)=\frac{r(t)}{s(t)} \qquad \psi(t)=\frac{p(t)}{q(t)}
$$
where ${} r,\, s,\, p,\, q \in K[t] {}$, and we may assume that ${} r,\, s {}$ and ${} p,\, q {}$ have no common factors. Now we clear denominators in our starting equation:
$$
s(t)^{3}p(t)^{2}=q(t)^{2}r(t)(r(t)-s(t))(r(t)-\lambda s(t)) \tag{*}
$$
#todo find the notes missing

Similarly, ${} q(t)^{2} \mid  s(t)^{3} {}$. This tells us that ${} as(t)^{3}=q(t)^{2} {}$, for some ${} a \in K {}$. This gives us
$$
as(t)= \left( \frac{q(t)}{s(t)} \right) ^{2}\tag{**}
$$
This tells us that ${} s(t)$ is a square in ${} K[t]$ and ${} s(t) \mid q(t) {}$. Now substitute ${} (**) {}$ into ${} (*) {}$:
$$
p^{2}(t)=ar(t)(r(t)-s(t))(r(t)-\lambda s(t))
$$
In fact, ${} r(t),\, r(t)-s(t),\, r(t)-\lambda s(t) {}$ are also squares in ${} K[t] {}$. 

We shall now construct an infinite sequence of polynomials. Set ${} r_{0}(t)=r(t) {}$ and ${} s_{0}(t)=s(t) {}$. We proceed by way of induction.

We claim that, with the supposition that there exist ${} r_{i}(t) {}$ and ${} s_{i}(t) \in K[t] {}$ with no common factors, and ${} \lambda_{i},\, \mu_{i} \in K -\{ 0 \} {}$ with ${} \lambda_{i}\neq \mu_{i} {}$ such that 
$$
r_{i}(t),\, s_{i}(t),\, r_{i}(t)-\lambda_{i} s_{i}(t),\, r_{i}(t)-\mu_{i} s_{i}(t)
$$
are all squares in ${} K[t] {}$, then there exist ${} r_{i+1}(t) {}$ and ${} s_{i+1}(t) \in K[t] {}$ with no common factors and ${} \lambda_{i+1},\, \mu_{i+1} \in K-\{ 0 \} {}$ with ${} \lambda_{i+1}\neq \mu_{i+1} {}$ such that
$$
r_{i+1}(t),\, s_{i+1}(t),\, r_{i+1}(t)-\lambda_{i+1} s_{i+1}(t),\, r_{i+1}(t)-\mu_{i+1} s_{i+1}(t)
$$
are all squares, and ${} \deg r_{i+1}=\frac{ \deg r_{i} }{ 2 } {}$ and ${} \deg s_{i+1} = \frac{ \deg s_{i} }{ 2 } {}$. Note that since ${} r_{i},\, s_{i} {}$ are both squares they must have even degree. 
##### Proof:
We have that ${} r_{i}(t)=u(t)^{2} {}$ and ${} s_{i}(t)=v(t)^{2} {}$. Then
$$
r_{i}(t)-\lambda_{i} s_{i}(t)=(u(t)-\lambda'v(t))(u(t)+\lambda'v(t))
$$
where ${} (\lambda')^{2}=\lambda_{i} {}$, and 
$$
r_{i}(t)-\mu_{i} s_{i}(t)=(u(t)-\mu'v(t))(u(t)+\mu'v(t))
$$
where ${} (\mu')^{2}=\mu_{i} {}$. Note that ${} u(t),\, v(t) {}$ have no common factors, so
$$
u(t)-\lambda'v(t) \qquad \text{ and }\qquad u(t)+\lambda'v(t)
$$
have no common factors, and 
$$
u(t)-\mu'v(t) \qquad \text{ and }\qquad u(t)+\mu'v(t)
$$
have no common factors. In particular, all of these polynomials are squares. Therefore, take
$$
r_{i+1}(t)=u(t)-\lambda' v(t) \qquad \text{and} \qquad s_{i+1}(t)=u(t)+\lambda'v(t)
$$
and one may find ${} \lambda_{i+1},\, \mu_{i+1} \in K-\{ 0 \} {}$ such that 
$$
u(t)-\mu'v(t)=r_{i+1}(t)+\lambda_{i+1}s_{i+1}(t)\qquad \text{and}\qquad 
u(t)+\mu'v(t)=r_{i+1}(t)+\mu_{i+1}s_{i+1}(t)
$$

(follows from linear algebra, check #todo). Furthermore, ${} \deg r_{i+1}=\deg r_{i} / 2 {}$ and ${} \deg s_{i+1}=\deg  s_{i} / 2 {}$. 


Now apply the claim with ${} r_{0}(t)=r(t) {}$ and ${} s_{0}(t)=s(t) {}$ and $\lambda_{0}=\lambda {}$ and ${} \mu_{0}=1 {}$. 