---
tags:
  - chapter
  - alggeo
date: 2025-02-28
completed: false
---
[[Directory]], [[Algebraic Geometry 1|Subject Directory]]
[[University/Undergraduate/Second Year/Algebraic Geometry/Lectures/1. |ðŸž€ðŸž€]] [[University/Undergraduate/Second Year/Algebraic Geometry/Lectures/6. |â—€]] [[University/Undergraduate/Second Year/Algebraic Geometry/Lectures/8. |â–¶]] [[University/Undergraduate/Second Year/Algebraic Geometry/Lectures/11. |ðŸž‚ðŸž‚]]
# Morphisms
## Functions on Algebraic sets
Let ${} X \subseteq  K^{n} {}$ be an algebraic set, and let ${} I=I(X) {}$. We define ${} K[X]=K[x_{1},\,\dots,\,x_{n}] / I {}$. We call this the ring of polynomial (or regular) functions on $X$. Let ${} f \in K[X] {}$. 
### Claim
We claim that ${} f {}$ defines a function ${} X \to{}K {}$,
#### Proof:
Let ${} F \in K[x_{1},\,\dots,\,x_{n}] {}$ such that ${} f=F \:(\mathrm{mod}\  I)  {}$, and define ${} f(a_{1},\,\dots,\,a_{n})=F(a_{1},\,\dots,\,a_{n}) {}$ for a point ${} \mathbf{a} = (a_{1},\,\dots,\,a_{n}) \in X {}$. We must check that this is well defined.  Let ${} \tilde{F} \in K[x_{1},\,\dots,\,x_{n}] {}$ such that ${} f=\tilde{F} \:(\mathrm{mod}\  I)  {}$. Since ${} F-\tilde{F} \in I {}$, then ${} (F-\tilde{F})(a_{1},\,\dots,\,a_{n})=0 {}$. Therefore, 
$$
\tilde{F}(a_{1},\,\dots,\,a_{n})=F(a_{1},\,\dots,\,a_{n})
$$
as required. 
### Remark
$K$ is an algebraic set. One should think of $f {}$ as a morphism of algebraic sets ${} f:X \to{}K {}$. 
## Polynomial mappings (or morphisms) between algebraic sets
Let ${} X \subseteq K^{n} {}$ and ${} Y \subseteq K^{m} {}$ be two algebraic sets. A polynomial map, or morphism, $f:X\to{}Y {}$ is a function of the form
$$
f(a_{1},\,\dots,\,a_{n})=(F_{1}(a_{1},\,\dots,\,a_{n}),\,\dots,\,F_{m}(a_{1},\,\dots,\,a_{n}))
$$
where ${} (a_{1},\,\dots,\,a_{n}) \in X {}$ and ${} F_{i} \in K[x_{1},\,\dots,\,x_{n}] {}$. 
### Remark
1) The identity map ${} 1_{X}:X\to{}X {}$ is a morphism.
2) If $f:X\to{}Y {}$ and $g:Y\to{}Z {}$ are morphisms, then ${} (g \circ  f):X\to{}Z {}$ is a morphism. 

We say that a morphism is an isomorphism if it has an inverse which is a morphism, i.e.
$$
f:X\to{}Y \Rightarrow \exists g:Y\to{}X\quad :\quad g \circ  f = f \circ  g = \id 
$$
Note that bijective morphisms are not always isomorphisms.
#### Example:
1) ${} f:K \to{}K^{3} {}$ mapping ${} t\mapsto (t,\, t^{2},\, t^{3}) {}$. This is a morphism, but not an isomorphism. We showed that $f(K)=X {}$ is an algebraic set, and that ${} f:K\to{}X {}$ is an isomorphism, with inverse ${} g:X\to{}K {}$ given by ${} (x,\, y,\, z)\mapsto x {}$. 
2) isomorphisms are always bijective (exercise)
3) ${} C=\{ x^{2}-y^{3}=0 \} \subseteq \mathbb{C}^{3} {}$. Let ${} r(t):\mathbb{C} \to{}C {}$ mapping ${} t \mapsto (t^{3},\, t^{2}) {}$. This is bijective (easy) but not an isomorphism (not so easy).
## Morphisms of rings
Let $f:X\to{}Y {}$ be a morphism of algebraic sets. We define a $K$-algebra morphism $f^{*}:K[Y]\to{}K[X] {}$ as follows: 

Let ${} g \in K[Y] {}$. Then $g$ gives a polynomial function $g:Y\to{}K {}$. Then ${} g \circ  f:X\to{}K {}$ is again polynomial function, and ${} g \circ  f \in K[X] {}$. We define
$$
f^{*}(g)=g \circ f
$$
#todo exercise: verify this is a $K$-algebra morphism, e.g. ${} f^{*}(g+h)=(g+h)\circ f=g \circ  f + h \circ  f = f^{*}(g)+f^{*}(h) {}$. 

More concretely, ${} X \subseteq K^{n} {}$, ${} Y \subseteq K^{m} {}$, and $f:X\to{}Y {}$ is given by ${} f(x_{1},\,\dots,\,x_{n})=(F_{1}(x_{1},\,\dots,\,x_{n}),\,\dots,\,F_{m}(x_{1},\,\dots,\,x_{n})) {}$, and ${} g \in K[Y] {}$ is represented by a polynomial ${} g(y_{1},\,\dots,\,y_{m}) {}$, then ${} f^{*}(g)=g(F_{1}(x_{1},\,\dots,\,x_{n}),\,\dots,\,F_{m}(x_{1},\,\dots,\,x_{n})) {}$.

In fact, every $K$-algebra morphism $\Phi:K[Y]\to{}K[X] {}$ arises this way. Suppose there exists some $f:X\to{}Y {}$ such that $f^{*}=\Phi {}$. To prove this, let ${} K[Y]=K[y_{1},\,\dots,\,y_{m}] / I(Y) {}$. We define ${} f_{i}=\Phi(\conj{y_{i}}) {}$, where ${} \conj{y_{i}}=y_{i} \:(\mathrm{mod}\   I(Y))  {}$.  Now ${} f_{i} \in K[X] {}$ gives a function ${} f_{i}:X \to{}K {}$. Thus, 
$$
f= (f_{1},\,\dots,\,f_{m})
$$
gives ${} f:X\to{}K^{m} {}$. Now we need to show that ${} f(X) \subseteq Y {}$. To show this, we need to show that if ${} g \in I(Y) {}$, then ${} g(f_{1},\,\dots,\,f_{m})=0 {}$. This holds, since
$$
\begin{align}
g(f_{1},\,\dots,\,f_{m}=g(\phi))
\end{align}
$$