---
tags:
  - chapter
  - calculus1
date: 2023-11-30
---
[[Directory]], [[Calculus 1|Subject Directory]]
# 
## 
### 
The fundamental theorem of calculus has ${} 2 {}$ important uses:
1. It guarantees that all continuous functions on ${} [a,\, b] {}$ have an antiderivative
2. It allows us to differentiate functions defined by integrals

Now we wonder if anti derivatives are unique. The answer is very quickly no, as if $F$ is a function, then 
$$
F'(x)=f(x)=(F(x)+c)'
$$

### Theorem 1.1: The Fundamental Theorem of Calculus part 2
Let ${} f:[a,\, b]\to{}\mathbb{R} {}$ be a function (not necessarily continuous) which is Riemann integrable. Suppose also that ${} F:[a,\, b]\to{}\mathbb{R} {}$ is continuous such that ${} F'(x)=f(x) {}$ for all ${} x \in (a,\, b) {}$. Then
$$
\int_{a}^{b} f(x) \ud x =F(b)-F(a)=\left[ F(x) \right] _{a}^{b} \quad \text{    (notation)}
$$
#### Remark:
$F$ may be *any* antiderivative of $f$, not necessarily the one defined in FTC part 1.
#### Corollary:
If ${} f:[a,\, b]\to{}R {}$ is Riemann integrable, and ${} F,\, G:[a,\, b]\to{}\mathbb{R} {}$ are antiderivatives for $f$, then there is some ${} c \in \mathbb{R} {}$ such that for all ${} x \in [a,\, b] {}$
$$
F(x)=G(x)+c
$$
#### Proof:
Since ${} F,\, G {}$ are antiderivatives, by FTC part 2, 
$$
\int_{a}^{x} f(t) \ud t =F(x)-F(a)
$$
and
$$
\int_{a}^{x} f(t) \ud t=G(x)-G(a) 
$$
Therefore, ${} F(x)-F(a)=G(x)-G(a) {}$, so ${} F(x)=G(x)+(\underbrace{ F(a)-G(a) }_{ c \in \mathbb{R} }) {}$
In this way, FTC part 2 has 2 important uses:
1. Guarantees antiderivatives are unique up to an additive constant
2. Gives us a practical way to compute integrals
### Example:
Compute
$$
\frac{d}{dx} \int_{0}^{\tan (x)} \frac{1}{\sqrt{1+t^{2}}} \ud t 
$$
Let ${} u(x)=\tan(x) {}$, then
$$
\begin{align}
 \frac{d}{dx} \int_{0}^{\tan(x)} \frac{1}{\sqrt{1+t^{2}}} \ud t & =\frac{du}{dx} \frac{d}{dx} \int_{0}^{u} \frac{1}{\sqrt{1+t^{2}}} \ud t \\
 & =\sec ^{2}(x) \frac{1}{\sqrt{1+u^{2}}} \\
 & =\sec ^{2}(x) \frac{1}{\sqrt{1+\tan ^{2}(x)}} \\
 & =\frac{\sec ^{2}(x)}{\sec(x)} \\
 & =\sec (x) 
 \end{align}
$$
### Example:
Compute 
$$
\int_{0}^{\pi/4} \frac{\tan(\theta)}{\cos(\theta)} \ud \theta 
$$
Note that $$
\frac{ \tan\theta }{ \cos\theta }=\sec\theta \tan\theta=\frac{d}{d\theta}\sec\theta
$$
so
$$
\int_{0}^{\pi/4} \frac{d}{d\theta}\sec\theta \ud \theta =[\sec\theta]_{0}^{\pi/4}=\sec\left( \frac{\pi}{4} \right)-\sec(0)=\sqrt{2}-1
$$
By FTC part 2.
### Definition 1.2:
Let ${} f:[a,\, b]\to{}\mathbb{R} {}$ be integrable. Then 
$$
\int_{a}^{b} f(x) \ud x 
$$is called the *definite integral* of ${} f(x)$. 
### Definition 1.3:
Suppose that $f$ has an antiderivative $F$. The *indefinite integral* of $f$ is another name for ${} F(x)+c {}$, for some ${} c \in \mathbb{R} {}$, written as
$$
\int f(x) \ud x 
$$
without limits
### Definition 1.4:
Given a definite or indefinite integral
$$
\int_{a}^{b} f(x) \ud x \text{ or } \int f(x) \ud x
$$
The expression ${} f(x) {}$ is called the *integrand*.
# Integration Techniques
## Integration by Substitution
### Proposition 2.1
Suppose ${} x=x(t) {}$ is a continuous function of ${} t {}$ on the interval ${} [t_{1},\, t_{2}] {}$, and differentiable on ${} (t_{1},\, t_{2}) {}$. Let ${} a=x(t_{1}) {}$ and ${} b=x(t_{2}) {}$, then
$$
\int_{a}^{b} f(x) \ud x =\int_{t_{1}}^{t_{2}} f(x(t))\frac{dx}{dt}  \ud t
$$
#### Example:
Find the indefinite integral 
$$
\int \frac{1}{\sqrt{1-x^{2}}} \ud x 
$$
using substitution.
Set ${} x(t)=\sin(t) {}$, ${} \frac{dx}{dt} =\cos(t) {}$, so
$$
\int \frac{1}{\sqrt{1-x^{2}}} \ud x =\int \frac{1}{\sqrt{1-\sin ^{2}t}}\cos t \ud t =\int  \ud t =t+c=\arcsin(x)+c
$$
#### Example:
Compute the definite integral 
$$
\int_{0}^{\pi/2} \sin^{m}(\theta)\cos(\theta) \ud \theta 
$$
let ${} u=\sin\theta {}$. Then, 
$$
\frac{du}{d\theta}=\cos(\theta)\Rightarrow \frac{d\theta}{du}=\frac{1}{\cos(\theta)} 
$$
Then
$$
\int_{0}^{\pi/2} \sin^{m}(\theta)\cos(\theta) \ud \theta =\int_{0}^{1} u^{m}\cos\theta \frac{ 1 }{ \cos\theta }\ud u =\left[ \frac{1}{m+1}u^{m+1} \right]_{0}^{1}=\frac{1}{m+1}
$$
## Integration by Parts
The Leibniz rule was useful for differentiation, and we can "reverse it" to help with integration.

Suppose ${} f,\, g {}$ are differentiable such that ${} f'(x) {}$ and ${} g'(x) {}$ are continuous. If we wanted to integrate ${} f'(x)g(x) {}$, then recall that
$$
\frac{d}{dx} [f(x)g(x)]=f'(x)g(x)+f(x)g'(x)
$$
or in other words
$$
f'(x)g(x)=\frac{d}{dx} (f(x)g(x))-f(x)g'(x)
$$
Therefore, 
$$
\begin{align}
 \int_{a}^{b} f'(x)g(x) \ud x  & =\int_{a}^{b} \frac{d}{dx} (f(x)g(x))-f(x)g'(x) \ud x    \\
 & =\int_{a}^{b} \frac{d}{dx} (f(x)g(x)) \ud x -\int_{a}^{b} f(x)g'(x) \ud x  \\
 & = [f(x)g(x)]_{a}^{b}-\int_{a}^{b} f(x)g'(x) \ud x 
 \end{align}
$$
(similarly for indefinite integrals)
#### Example:
Compute the indefinite integral
$$
\int \arcsin(x) \ud x 
$$
First, lets use the substitution ${} x(\theta)=\sin(\theta) {}$, then 
$$
\begin{align}
 \int \arcsin(x) \ud x  & =\int \arcsin(\sin(\theta))\cos(\theta) \ud \theta    \\
 & =\int \theta \cos\theta \ud \theta 
 \end{align}
$$
Note that
$$
\frac{d}{d\theta}=\sin\theta+\theta \cos\theta
$$
So
$$
I=\int \frac{d}{d\theta}(\theta \sin\theta)-\sin\theta \ud x= \theta \sin\theta+\cos\theta+c
$$
Now we have
$$
\sqrt{1-x^{2}}=\sqrt{1-\sin ^{2}\theta}=\sqrt{\cos ^{2}\theta}=\cos\theta
$$
So
$$
I=x\arcsin x+\sqrt{1-x^{2}}+c
$$
#### Example:
Compute 
$$
I=\int_{1}^{2} \ln(x) \ud x
$$
So
$$
\frac{d}{dx} (x\ln x)=\ln x+x\cdot \frac{1}{x}=\ln(x)+1
$$
So
$$
\begin{align}
 \int_{1}^{2} \ln(x) \ud x  & =\int_{1}^{2} \frac{d}{dx} (x\ln (x))-1 \ud x    \\
 & ={[x\ln(x)]_{1}^{2}}-\int_{1}^{2}  \ud x  \\
 & =[x\ln(x)]_{1}^{2}-[x]_{1}^{2} \\
 & =2\ln(x)-1\ln(1)-(2-1) \\

 \end{align}
$$