---
tags:
  - chapter
  - calculus1
date: 2023-10-13
---
[[Directory]], [[Calculus 1|Subject Directory]]
# Further Trigonometry
## Identities
### Euler's Formula
For all $\theta \in\mathbb{R}$
$$
e^{i\theta}=\cos\theta+i\sin\theta
$$
(where $i^{2}=-1$)

What does $e^{z}$ even mean when $z\in\mathbb{C}$??
### ...using power series
If we define that the power series that works in the reals, also works for complex numbers, then we can define
$$
\begin{align}
 e^{ix}: & =\sum_{n=0}^{\infty} \frac{(ix)^{n}}{n!}  \\
 & = 1+\frac{ix}{1!}-\frac{x^{2}}{2!}+\frac{ix^{3}}{3!}+\frac{x^{4}}{4!}+\dots
 \end{align}
$$
By this definition, we get
$$
e^{-ix}=e^{i(-x)}=\sum_{n=0}^{\infty} \frac{(-ix)^{n}}{n!}=1-\frac{ix}{1!}-\frac{x^{2}}{2!}+\frac{ix^{3}}{3!}+\frac{x^{4}}{4!}
$$
Note that the terms with an even powers have the same sign, but the odd terms have an opposite sign

Therefore
$$
\begin{align}
 \frac{1}{2}(e^{ix}+e^{-ix})&=1-\frac{x^{2}}{2!}+\frac{x^{4}}{4!}-\frac{x^{6}}{6!}+\dots   \\
 & =\cos x
 \end{align}
$$
and
$$
\begin{align}
 \frac{1}{2i}\left( e^{ix}-e^{-ix}\right)&=x-\frac{x^{3}}{3!}+\frac{x^{5}}{5!}-\frac{x^{7}}{7!}+\dots \\
 & =\sin x  
 \end{align}
$$
Rearranging these equations, we directly get
$$
e^{ix}=\cos x+i\sin x
$$
### Compound Angle Formulae
These do *not* need to be learned by rote
By multiplying power series, we have that 
$$
e^{i(\theta+\varphi)}=e^{i\theta}e^{i\varphi}, \qquad\forall \theta,\, \varphi \in  \mathbb{R}
$$
Note: $\theta,\,\varphi$ are thought of as angles

So, 
$$
\begin{align}
 \cos(\theta+\varphi)+i\sin(\theta+\varphi)&=e^{i(\theta+\varphi)}   \\
 & =e^{i\theta}e^{i\varphi} \\
 & =(\cos\theta+i\sin\theta)(\cos\varphi+i\sin\varphi) \\
 & =\cos\theta \cos\varphi+i\cos\theta \sin\varphi+i\sin\theta \cos\varphi-\sin\theta \sin\varphi \\
 & =\cos\theta \cos\varphi-\sin\theta \sin\varphi \\
 & \phantom{={}}i(\cos\theta \sin\varphi+\sin\theta \cos\varphi)
 \end{align}
$$
Specifically, we have
$$
\cos(\theta+\varphi)=\cos\theta \cos\varphi-\sin\theta \sin\varphi
$$
and
$$
\sin(\theta+\varphi)=\sin\theta \cos\varphi+\cos\theta \sin\varphi
$$
### Many Identities
$$
\tan(\theta+\varphi)=\frac{\tan\theta+\tan\varphi}{1-\tan\theta \tan\varphi}
$$
By setting $\varphi=\theta$, we have
$$
\begin{align}
\cos2\theta & =\cos ^{2}\theta-\sin ^{2}\theta \\
\sin 2\theta & =2\sin\theta \cos\theta  \\
\tan 2\theta & =\frac{2\tan\theta}{1-\tan ^{2}\theta}
\end{align}
$$
By adding $\sin ^{2}\theta+\cos ^{2}\theta=1$ and $\cos ^{2}\theta-\sin ^{2}\theta=\cos 2\theta$, we get
$$
\cos ^{2}\theta=\frac{1}{2}(1+\cos 2\theta)
$$
and by taking the difference
$$
\sin ^{2}\theta=\frac{1}{2}(1-\cos 2\theta)
$$
We also get difference formula
$$
\begin{align}
\sin(\theta-\varphi) & =\sin\theta cos\varphi-\cos\theta \sin\varphi \\
\cos(\theta-\varphi) & =\cos\theta \cos\varphi+\sin\theta \sin\varphi \\
\tan(\theta-\varphi) & =\frac{\tan\theta-\tan\varphi}{1+\tan\theta \tan\varphi}
\end{align}
$$
### Relation to Hyperbolic Trigonometry
We know that $\cosh x=\frac{1}{2}e^{x}+e^{-x}$ for $x \in\mathbb{R}$
we extend the definition to $x \in\mathbb{C}$
$$
\begin{align}
\cos\theta & =\frac{1}{2}(e^{i\theta}+e^{-i\theta})=\cosh i\theta \\
\sin\theta & =\frac{1}{2i}(e^{i\theta}-e^{-i\theta})=-i\sinh i\theta \\
\tan\theta & =\frac{-i\sinh i\theta}{\cosh i\theta}=-i\tanh i\theta
\end{align}
$$

