---
tags:
  - exercises
  - grillet_abstract_alg
date:
count: 21
---
[[Directory]], [[Grillet Abstract Algebra]]
[[/Textbooks/Undergraduate/First Year/Grillet Abstract Algebra/Exercises/2.12. Group Extensions Exercises.md|ðŸž€ðŸž€]] [[/Textbooks/Undergraduate/First Year/Grillet Abstract Algebra/Exercises/2.12. Group Extensions Exercises.md|â—€]] [[/Textbooks/Undergraduate/First Year/Grillet Abstract Algebra/Exercises/3.2. Subrings and Ideals Exercises.md|â–¶]] [[/Textbooks/Undergraduate/First Year/Grillet Abstract Algebra/Exercises/3.12. GrÃ¶bner Bases Exercises.md|ðŸž‚ðŸž‚]]
1. skip
2. skip
3. skip
4. skip
5. skip
6. 
Let ${} x,\, n \in \mathbb{Z} {}$ with ${} \gcd(x,\, n)=1 {}$. Now ${} x {}$ induces an element ${} \conj{x} \in \mathbb{Z}_{n} {}$ with ${} \conj{x}\equiv x \:(\mathrm{mod}\  n)  {}$. Since ${} x,\, n {}$ are relatively prime, then ${} \conj{x} {}$ has (additive) order $n {}$, and is a unit. Now take the multiplicative group of units of ${} \mathbb{Z}_{n}$. This has order ${} \phi(n) {}$, and so every element in the group has order which divides ${} \phi(n)$. Therefore, ${} \conj{x}^{\phi(n)}=1 {}$, and so
$$
x^{\phi(n)}\equiv 1 \:(\mathrm{mod}\  n) 
$$
7. skip
8. skip
9. skip
10. skip
11. 
${} R^{1}$ is clearly an abelian group under addition. Now if ${} (x,\, a),\, (y,\, b),\, (z,\, c) \in R^{1} {}$, then 
$$
\begin{align}
 ((x,\, a)(y,\, b))(z,\, c) & = (xy+bx+ay,\, ab)(z,\, c) \\
 & =(xyz+bxz+ayz+cxy+bcx+acy+abz,\, abc) \\
	 & =(x,\, a)(yz+cy+bz,\, bc) \\
 & =(x,\, a)((y,\, b)(z,\, c)) 
 \end{align}
$$
and 
$$
(0, 1)(x,\, y)=(0x+0y+1x,\, 1y)=(x,\, y)=(x 0+x 1 + y0,\, y 1)=(x,\, y)(0,\, 1)
$$
so ${} R^{1}$ is a ring with identity
12. 
Suppose that
$$
(0,\, 2)(x,\, y)(0,\, 2)=(0,\, 2)
$$
then 
$$
(4x,\, 4y)=(0,\, 2)
$$
and so ${} x=0 {}$ and ${} 4y=2 {}$, or ${} y=\frac{1}{2} {}$, which is not an element of $\mathbb{Z}$. Therefore, ${} R^{1}$ is not regular.
13. 
Let $R {}$ be a ring with identity. Now if ${} x \in R {}$, then set ${} \zeta_{x}:R\to{}R {}$ be defined by ${} \zeta_{x}(r)=xr {}$. Now if ${} \zeta_{x}=\zeta_{y} {}$, then ${} \zeta_{x}(1)=x=y=\zeta_{y}(1) {}$, and so the mapping ${} x \mapsto \zeta_{x} {}$ is injective. Furthermore, if ${} x,\, y {}$ in $R$, then
$$
\zeta_{x+y}(r)=(x+y)(r)=xr+yr=\zeta_{x}(r)+\zeta_{y}(r)
$$
and
$$
\zeta_{xy}(r)=(xy)(r)=x(yr)=\zeta_{x}(\zeta_{y}(r))
$$
and so ${} \zeta_{x}$ is a homomorphism, and $R$ is embedded in ${} \operatorname{End}(R,\, +) {}$.