---
tags:
  - exercises
  - grillet_abstract_alg
date:
count: 42
---
[[Directory]], [[Grillet Abstract Algebra]]
[[/Textbooks/Undergraduate/First Year/Grillet Abstract Algebra/Exercises/4.9. Separability Exercises.md|ðŸž€ðŸž€]] [[/Textbooks/Undergraduate/First Year/Grillet Abstract Algebra/Exercises/4.9. Separability Exercises.md|â—€]] [[/Textbooks/Undergraduate/First Year/Grillet Abstract Algebra/Exercises/5.2. Normal Extensions Exercises.md|â–¶]] [[/Textbooks/Undergraduate/First Year/Grillet Abstract Algebra/Exercises/5.9. Geometric Constructions Exercises.md|ðŸž‚ðŸž‚]]
1. 
We have that the roots of ${} X^{3}-2 {}$ are ${} \sqrt[3]{2},\, \sqrt[3]{2}e^{2\pi i/3},\, \sqrt[3]{2}e^{4\pi i/3} {}$. Then ${} \mathbb{Q}(\sqrt[3]{2},\, e^{2\pi i/3}) {}$ is the splitting field of ${} X^{3}-2 {}$
2. 
The roots of ${} X^{4}+5X^{2}+6 {}$ are ${} -i\sqrt{2},\, i\sqrt{2},\, -i\sqrt{3},\, i\sqrt{3} {}$. Therefore, ${} \mathbb{Q}(i,\, \sqrt{2},\, \sqrt{3}) {}$ is the splitting field of 
3. skip
4. skip
5. 
Let $K$ be a field that contains a subfield of order ${} p^{n}$. Then that field is isomorphic to ${} GF(p^{n}) {}$, and so every element is a root of ${} X^{p^{n}}-X {}$. Since that is ${} p^{n}$ elements, then ${} X^{p^{n}}-X {}$ splits in $K$. Conversely, if ${} X^{p^{n}}-X {}$ splits in $K$, then its roots must form a subfield, and since there are ${} p^{n}$ distinct roots, then $K$ has a subfield of order ${} p^{n}$. 

Now let ${} E,\, F \subseteq K {}$ be subfields of order ${} p^{n}$. Then ${} E \cup F {}$ contains roots of ${} X^{p^{n}}-X {}$, and so ${} |E \cup F|\leq p^{n} {}$, so ${} E\cup F=E=F {}$.
1. 
Suppose that a field $K {}$ of order ${} p^{n} {}$ contains a subfield $E {}$ of order ${} p^{m}$. Then $K$ is the splitting field of ${} X^{p^{n}}-X {}$, and $E$ is the splitting field of ${} X^{p^{m}}-X {}$. Let ${} x \in E {}$. Then ${} x^{p^{n}}=x^{p^{m}}=x {}$. Therefore, ${} x^{p^{n}-1}=x^{p^{m}-1}=1 {}$, and so ${} p^{m}-1 \mid  p^{n}-1 {}$, or ${} a(p^{m}-1)=p^{n}-1 {}$ for some ${} a \in \mathbb{Z} {}$.

Now suppose that ${} m \nmid n {}$. Then 
$$
\mathbb{Z}\ni a=\frac{p^{n}-1}{p^{m}-1} =\frac{\sum_{k=0}^{n-1} p^{k}}{\sum_{k=0}^{m-1} p^{k}} 
$$
and so if ${} \ell=\floor*{n / m}  {}$, then 
$$
a=\left( \sum _{k=0}^{\ell-1}p^{mk} \right)\left( \sum_{k=0}^{m-1} p^{k} \right)+p^{\ell m+1} \frac{\sum_{k=0}^{n-\ell m-1} p^{k}}{\sum_{k=0}^{m-1} p^{k}} 
$$
and since ${} p \nmid \sum_{k=0}^{m-1} p^{k} {}$, then ${} \sum_{k=0}^{m-1} p^{k} \nmid p^{\ell m+1} {}$, and since ${} n-\ell m - 1 < m-1 {}$, then the ${} 2nd {}$ term is not an element $\mathbb{N}$, and since the first term is, then this is a contradiction, as $a {}$ is an element of $\mathbb{Z}$. Therefore, ${} m \mid n {}$.

Conversely, suppose that ${} m \mid  n {}$. Then 
$$
\sum_{k=0}^{n /m} p^{k}=\frac{p^{n}-1}{p^{m}-1} \in \mathbb{Z}
$$
so ${} p^{m}-1 \mid  p^{n}-1 {}$. Therefore there exists a subgroup ${} E^{\times } \leq K^{\times } {}$ of order ${} p^{m}-1 {}$. Then if ${} x \in E=E^{\times } \cup  \{ 0 \} {}$, then ${} x^{p^{m}-1}=1 {}$, so ${} x^{p^{m}}-x=0 {}$, and ${} E\cong GF(p^{m}) {}$, so ${} E \subseteq K {}$ is a subfield of order ${} p^{m}$.
7. skip
