---
tags:
  - exercises
  - grillet_abstract_alg
date: 2025-02-28
count: 45
---
[[Directory]], [[Grillet Abstract Algebra]]
[[/Textbooks/Undergraduate/First Year/Grillet Abstract Algebra/Exercises/5.1. Splitting Fields Exercises.md|ðŸž€ðŸž€]] [[/Textbooks/Undergraduate/First Year/Grillet Abstract Algebra/Exercises/5.3. Galois Extensions Exercises.md|â—€]] [[/Textbooks/Undergraduate/First Year/Grillet Abstract Algebra/Exercises/5.5. Polynomials Exercises.md|â–¶]] [[/Textbooks/Undergraduate/First Year/Grillet Abstract Algebra/Exercises/5.9. Geometric Constructions Exercises.md|ðŸž‚ðŸž‚]]
1. 
Suppose that ${} \Gal(E : F) {}$ is normal in ${} \Gal(E : K) {}$. Let $\sigma$ be a $K$-automorphism of ${} \bar{K} {}$. Then since $E$ is normal over $K$, then ${} \alpha=\sigma_{|E} \in \Gal(E : K) {}$. By normality, ${} \alpha\Gal(E : F)\alpha ^{-1}=\Gal(E : F) {}$. Therefore, ${} \alpha\gamma=\delta\alpha {}$ for ${} \gamma,\, \delta \in \Gal(E : F) {}$. Now if ${} x \in F {}$, then ${} \alpha x=\alpha\gamma x=\delta\alpha x {}$, so ${} \alpha x \in \Fix_{E}(\Gal(E : F))=F {}$. Therefore, $\alpha F=F {}$, and so $\sigma F=F {}$, and $F$ is normal over $K$.

Now suppose that $F$ is normal over $K {}$. Let $\alpha \in \Gal(E : K) {}$.  Then $\alpha {}$ may be extended to an automorphism $\sigma {}$ of ${} \bar{K} {}$, so $\alpha F=F {}$. Therefore, if ${} \gamma \in \Gal(E : F) {}$ and ${} x \in F {}$, then ${} \alpha ^{-1}x \in F {}$, so ${} \gamma\alpha ^{-1}x=\alpha ^{-1}x {}$, and ${} \alpha\gamma\alpha ^{-1}x=\alpha\alpha ^{-1}x=x {}$, so ${} \alpha\gamma\alpha ^{-1} \in \Gal(E : F) {}$. Therefore, $\Gal(E : F) {}$ is normal in $\Gal(E : K) {}$. 

Now let ${} F {}$ be normal over ${} K {}$. Then consider ${} \Phi:\Gal(E : K)\to{}\Gal(F : K) {}$ defined by ${} \alpha\mapsto \alpha_{|F}$. If ${} \alpha,\, \beta \in \Gal(E : K) {}$, then ${} (\alpha\beta)_{|F}=\alpha_{|F}\beta_{|F} {}$, clearly, so $\Phi$ is a homomorphism of groups. Now ${} \ker \Phi=\Gal(E : F) {}$. Therefore, 
$$
\Gal(F : K)=\Gal(E : K) / \Gal(E : F)
$$
by the first isomorphism theorem.
2. 
Let ${} G$ be a group, and let ${} H,\, K \leq G {}$ be subgroups of finite index. Now if ${} g \in G {}$, then
$$
g(H \cap  K)=gH \cap  gK
$$
and since there are finitely many distinct cosets of ${} H$ and $K$, then there are finitely many intersections between them. Therefore, ${} [G:H \cap K] {}$ is finite.
3. 
Let $G$ be a group, and let $H \leq G {}$ have finite index. Therefore, ${} S={} \{ gHg^{-1} \mid g \in G \} {}$ is finite. If ${} K \in S {}$, and ${} a,\, b \in K {}$, then ${} ab^{-1}=gxg^{-1}gy^{-1}g^{-1}=gxy^{-1}g^{-1} {}$ for some ${} x,\, y \in H {}$ and ${} g \in G {}$. Since ${} xy^{-1} \in H {}$, then ${} gxy^{-1}g^{-1} \in K {}$. Therefore, $K$ is a subgroup of $G$. Furthermore, if ${} K \in S {}$, then ${} K=gHg^{-1} {}$, and if ${} x \in G {}$, then ${} x=gyg^{-1} {}$ for some ${} y \in G {}$, such that 
$$
xK=xgHg^{-1}=gyg^{-1}gHg^{-1}=gyHg^{-1}
$$
and so there is a bijection between cosets of $H$ and $K$. Therefore, $H$ is of finite index (in fact, the same index). Now ${} N=\bigcap S {}$ is a subgroup of finite index. If ${} g \in G {}$, then
$$
gNg^{-1}=g\left( \bigcap S \right)g^{-1}=\bigcap _{K \in S}gKg^{-1}=\bigcap _{\substack{K \in S\\K=fHf^{-1}\\f \in G} }gfH(gf)^{-1}=\bigcap S=N
$$
and so $H {}$ contains a normal subgroup of finite index. 
4.  
First, given a set of normal subgroups ${} A {}$ of $G {}$, then ${} g\left( \bigcap A \right)=\bigcap_{N \in A} gN {}$. Consider the map ${} \phi:G / \bigcap A \to{} \prod_{N \in A} G / N  {}$ mapping
$$
\bigcap _{N \in A} gN \mapsto \prod_{N \in A} gN
$$
Suppose that ${} g\left( \bigcap A \right)=h\left( \bigcap A \right) {}$. Then ${} gh^{-1} \in \bigcap A {}$, and so ${} gh^{-1} \in N {}$ for all ${} N \in A {}$. Therefore, ${} gN=hN {}$, and so $\phi$ is well defined. Now let ${} g,\, h \in G {}$ such that ${} \phi\left( g\left( \bigcap A \right) \right)=\phi\left( h\left( \bigcap A \right) \right) {}$. Then for all ${} N \in A {}$, then ${} gN=hN {}$, and so ${} gh^{-1} \in \bigcap A {}$. Therefore, $\phi {}$ is injective, and ${} G / \bigcap A {}$ is isomorphic to a subgroup of ${} \prod _{N \in A} G /N {}$.

Now if ${} A$ is the set of normal subgroups of finite index of $G$, then ${} \bigcap A=1 {}$, and so ${} G / \bigcap A\cong G {}$. Furthermore, each ${} G /N {}$ is finite, where ${} N \in A {}$. Therefore, ${} \prod _{N \in A} G /N {}$ is a direct product of finite groups. Now ${} \phi:G\to{}\prod _{N \in A} G /N {}$ is an embedding of $G$ into a direct product of finite groups. 

Conversely, suppose that $G$ may be embedded into a direct product of finite groups. Consider ${} G\leq \prod _{H \in B}H=A {}$, where $H$ are finite. Now given ${} K \in B {}$, then define 
$$
C_{K}=\prod _{\substack{H \in B\\H\neq K} }H
$$
and so ${} A=C_{K} \times K {}$. Now $C_{K} {}$ is normal in $A {}$, and ${} C_{K} \cap G \trianglelefteq  G {}$, and
$$
\begin{align}
G / (G \cap  C_{K}) \cong  GC_{K} / C_{K} \leq  A /C_{K} \cong K
\end{align}
$$
and so ${} G / (G \cap C_{K}) {}$ is finite. Therefore, ${} G \cap C_{K} {}$ is a normal subgroup of finite index. Now given ${} H,\, K \in B {}$ considered as subgroups of $A {}$ then ${} H \cap  K=\varnothing  {}$, as they form a direct product. Now 
$$
\bigcap _{K \in B} G \cap C_{K}= G \cap  \bigcap _{K \in B} C_{K}=1
$$
as required. 
5. Skip
6. Skip
7. 
First, let $H {}$ be open on ${} G=\Gal(E : K) {}$. Then 
$$
H=\bigcup _{\substack{\sigma \in S_{1} \subseteq G\\K\trianglelefteq G\\K \in S_{2}} }\sigma K
$$
(this is imprecise but you know what I mean) (I'm tired it's like 2am right now) (don't judge me future me)
where the ${} K$ are of finite index. Now ${} H^{-1}=\bigcup \sigma ^{-1}K^{-1}=\bigcup \sigma ^{-1}K {}$ which is still a union of cosets of normal subgroups of finite index. Therefore, ${} H^{-1} {}$ is open, and ${} (-)^{-1} {}$ is continuous. 

Now let ${} H$ be open on $G$. Then ${} S=(-\cdot -)^{-1}(H) {}$ is the set of all pairs of elements ${} a,\, b \in G {}$ such that ${} ab \in H {}$. We wish to show that $S {}$ is open in ${} G \times G {}$. Let ${} (a,\, b) \in S {}$. Then ${}  {}$