---
tags:
  - greub_linalg
  - exercises
date: 2023-12-21
---
[[Directory]], [[Greub Linear Algebra 1|Subject Directory]]
[[Linear Algebra - Werner Greub.pdf#page=39|Exercise Sheet]]
5. 
i)
Let $X$ be a set, and let $C(X)$ be the free vector space on $X {}$ over ${} \Gamma {}$. Let $F {}$ be another vector space over $\Gamma {}$, and let ${} f:X\to{}F {}$.

Let ${} \iota:X\to{}C(X) {}$ be defined by ${} x\mapsto f_{x} {}$ is the inclusion map. Then ${} \iota(X) {}$ is a basis of $C(X)$. Then ${} \iota^{0}:X\to{}\iota(X) {}$ is a bijection. Let ${} \varphi^{0}:\iota(X)\to{}F {}$ be defined by ${} \varphi^{0}(x)=f((\iota^{0})^{-1}(x)) {}$. Now ${} \varphi^{0} {}$ is a map of a basis of ${} C(X)$ into $F {}$. Therefore, there exists a unique linear extension of ${} \varphi^{0}$, ${} \varphi:C(X)\to{}F {}$. Now given ${} x \in X {}$, 
$$
(\varphi \circ \iota)(x)=\varphi(\iota(x))=\varphi(\iota^{0}(x))=\varphi^{0}(\iota^{0}(x))=f((\iota^{0})^{-1}(\iota^{0}(x))) =f(x)
$$
so ${} \varphi \circ \iota=f {}$. 

Now let ${} \psi:C(X)\to{}F {}$ be a linear map such that ${} \psi \circ \iota=f {}$. Then given ${} x \in X {}$,  ${} \psi(\iota(x))=f(x)=\varphi(\iota(x)) {}$. Since $\iota(X)$ is a basis of $C(X)$. Therefore, $\psi {}$ is an extension of ${} \varphi^{0} {}$, so ${} \psi=\varphi {}$, and $\varphi$ is unique.
ii)
Let ${} \alpha:X \to{}Y {}$ be a function. Now we have $\iota_{X}:X\to{}C(X) {}$ and ${} \iota_{Y}:Y\to{}C(Y) {}$ as the inclusion maps. We then restrict and ${} \iota_{X}^{0}:X\to{}\iota_{X}(X) {}$ and ${} \iota_{Y}^{0}:Y\to{}\iota_{Y}(Y) {}$, and we have ${} \iota_{X}(X) {}$ as a basis of ${} C(X) {}$ and ${} \iota_{Y}(Y) {}$ as a basis of $Y {}$. 

Now let ${} \alpha_{*}^{0}:\iota_{X}(X)\to{}\iota_{Y}(Y) {}$ be equal to ${} \iota_{Y}^{0} \circ \alpha \circ (\iota_{X}^{0})^{-1} {}$. This maps a basis of $C(X) {}$ to a basis of $C(Y)$. Therefore, there exists a unique extension ${} \alpha_{*}:C(X)\to{}C(Y) {}$. Since ${} \iota_{X}^{0}$ and ${} \iota_{Y}^{0}$ are bijections, then if $\alpha$ is injective, then ${} \alpha_{*}^{0}$ is injective, so ${} \iota_{X}(X) {}$ is linearly independent in ${} C(Y) {}$, and if $\alpha$ is surjective, then ${} \alpha_{*}^{0}$ is injective, so $\iota_{X}(X)$ is a spanning set of $C(Y)$. Finally, if $\alpha$ is bijective, then $\alpha_{*} {}$ is a linear isomorphism.

This linear map clearly commutes the diagram by construction. 

Now let ${} \beta:Y \to{}Z {}$. Then there exists a unique linear map $\beta_{*}$ from $C(Y)$ to $C(Z) {}$, and a unique linear map ${} (\beta \circ  \alpha)_{*} {}$ from $C(X)$ to $C(Z)$. Now 
$$
\begin{align}
 \beta_{*}^{0} \circ  \alpha_{*}^{0}  & =\iota_{Z}^{0} \circ  \beta \circ (\iota_{Y}^{0})^{-1} \circ \iota_{Y}^{0} \circ  \alpha \circ  (\iota_{X}^{0})^{-1}   \\
 & = \iota^{0}_{Z} \circ (\beta \circ \alpha) \circ  (\iota_{X}^{0})^{-1} \\
 & = (\beta \circ \alpha)_{*}^{0}
 \end{align}
$$
Therefore, ${} \beta_{*} \circ  \alpha_{*}=(\beta \circ  \alpha)_{*} {}$.
iii)
Let $E$ be a vector space. We have the identity map $\iota:E\to{}E {}$. Therefore, there exists a unique linear map $\pi_{E}:C(E)\to{}E {}$ with ${} \pi_{E} \circ  \iota_{E} {}=\iota$.
iv)
Let $E$ and $F$ be vector spaces with a map ${} \varphi:E\to{}F {}$. Now suppose that $\varphi {}$ is linear. Therefore, there exists a unique linear map ${} \varphi_{*} :E\to{}F {}$ with ${} \varphi_{*} \circ \iota_{E}=\iota_{F} \circ  \varphi {}$. Note that if ${} e \in E {}$, then ${} f_{e} \in C(E) {}$, and ${} \pi_{E}(f_{e})=(\iota_{E}^{0})^{-1}(f_{e}) {}$, so $\pi_{E} {}$ is the unique linear extension of ${} (\iota_{E}^{0})^{-1} {}$.

Then let ${} \mathbf{x}  \in C(E) {}$. Since ${} \iota_{X}(E) {}$ is a basis, then ${} \mathbf{x}=\sum_{e\in E} \lambda_{e}f_{e} {}$. Now we have
$$
\begin{align}
(\pi_{F} \circ  \varphi_{*})(\mathbf{x}) & =\pi_{F}\left( \varphi_{*}\left( \sum_{e\in E} \lambda_{e} f_{e} \right) \right) \\
 & =\sum_{e\in E} \lambda_{e} \pi_{F}(\varphi_{*}(f_{e})) \\
 & =\sum_{e\in E} \lambda_{e} (\pi_{F}\circ \iota^{0}_{F} \circ  \varphi \circ  (\iota_{E}^{0})^{-1})(f_{e}) \\
 & =\sum_{e\in E} \lambda_{e}(\varphi \circ  \pi_{E})(f_{e}) \\
 & =(\varphi \circ  \pi_{E})(\mathbf{x})
\end{align}
$$
so 
$$
\pi_{F} \circ  \varphi_{*} = \varphi \circ  \pi_{E}
$$
Conversely, suppose 
$$
\pi_{F} \circ  \varphi_{*}=\varphi \circ  \pi_{E}
$$
Then since ${} \pi_{F} \circ  \varphi_{*} {}$ is linear, and $\pi_{E}$ is linear, then $\varphi {}$ is linear. In particular, we have ${} \varphi = \pi_{F} \circ  \varphi_{*} \circ \iota_{E} {}$. Now if ${} \mathbf{x}_{\alpha} \in E {}$, then 
$$
\begin{align}
\sum_{\alpha} \lambda_{\alpha} \varphi(\mathbf{x}_{\alpha}) & =\pi_{F}\left( \varphi_{*}\left( \sum_{\alpha} \lambda_{\alpha} \iota_{E}(\mathbf{x}_{\alpha})\right) \right) \\
 & = \pi_{F}\left( \varphi_{*}\left( \sum_{\alpha}\lambda_{\alpha} f_{\mathbf{x}_{\alpha}} \right) \right) \\
 & =\pi_{F}\left( \iota_{F}\left( \varphi\left( \pi_{E}\left( \sum_{\alpha}\lambda_{\alpha}f_{\mathbf{x}_{\alpha}} \right) \right) \right) \right) \\
 & =\varphi\left( \sum_{\alpha}\lambda_{\alpha} \  \pi_{E}(f_{\mathbf{x}_{\alpha}}) \right) \\
 & =\varphi\left( \sum_{\alpha}\lambda_{\alpha} \mathbf{x}_\alpha \right)
\end{align}
$$
Therefore, $\varphi$ is linear.
v)
Let ${} N(E)=\{ f_{\lambda \mathbf{a}+\mu \mathbf{b}} - \lambda f_{\mathbf{a}}-\mu f_{\mathbf{b}}\mid \mathbf{a},\, \mathbf{b} \in E,\, \lambda ,\, \mu \in \Gamma \} \subseteq C(E) {}$. Now let ${} \mathbf{X} \in \ker  \pi_{E} {}$. Then ${} \pi_{E}(\mathbf{X} {})=0 {}$. We have ${} \mathbf{X}=\sum_{\alpha} \lambda_{\alpha} f_{\mathbf{x}_{\alpha}} {}$, so ${} \pi_{E}(\mathbf{X})=0 {}$ means that
$$
\begin{align}
 \pi_{E}\left( \sum_{\alpha} \lambda_{\alpha} f_{\mathbf{x}_{\alpha}} \right)  & =\sum_{\alpha} \lambda_{\alpha} \pi_{E}(f_{\mathbf{x}_{\alpha}}) \\
 & =\sum_{\alpha} \lambda_{\alpha} \mathbf{x}_{\alpha} =0 
 \end{align}
$$
Suppose