---
tags:
  - exercises
  - grillet_abstract_alg
date:
count: 31
---
[[Directory]], [[Grillet Abstract Algebra]]
[[/3.1. Rings Exercises.md|ðŸž€ðŸž€]] [[/3.10. Unique Factorization Domains Exercises.md|â—€]] [[/3.12. GrÃ¶bner Bases Exercises.md|â–¶]] [[/3.12. GrÃ¶bner Bases Exercises.md|ðŸž‚ðŸž‚]]
1. skip
2. 
Let ${} R$ be a domain. Then given an infinite family of indeterminants ${} ( X_{i} )_{i=1}^{\infty}  {}$, the family of ideals
$$
I=\{ (X_{ 1}),\, (X_{1})+(X_{2}),\,  (X_{1})+(X_{2})+(X_{3}),\,\dots \}
$$
is contained in the commutative ring ${} R[( X_{i} )_{i=1}^{\infty} ] {}$, and forms a chain. However, since there are infinite distinct indeterminants, the chain never terminates.
3. 
Let ${} R\subseteq S {}$ be commutative rings, and suppose that ${} R$ is Noetherian, and $S$ is generated by $R {}$ and finitely many elements of $S$, say, ${} (s_{i})_{i =1}^{n} {}$ for some finite $I$. Let $\varphi:R\to{}S {}$ be inclusion map. Then there is a homomorphism from ${} \psi:R[X_{1},\,\dots,\,X_{n}]\to{}S {}$ mapping ${} A\mapsto{}^{\varphi}A(s_{1},\,\dots,\,s_{n})=A(s_{1},\,\dots,\,s_{ n}) {}$. Since $R$ is Noetherian, then ${} R[X_{1},\,\dots,\,X_{n}] {}$ is Noetherian. Furthermore, ${} \im \psi \subseteq S {}$ contains $R {}$ and the ${} s_{i} {}$, and so therefore contains $S$, and $\psi$ is surjective. 

Now let $I$ be an ideal in $S {}$. Then there exists an ideal $J {}$ of ${} R[X_{1},\,\dots,\,X_{ n}]$ such that ${} \psi(J)=I {}$. Therefore, since $J$ is finitely generated as an ideal, then $I$ is finitely generated as an ideal, and $S$ is Noetherian.
4. 
Let $M$ be the free commutative monoid on ${} \{ X_{1},\,\dots,\,X_{ n} \} {}$, and let $\mathcal{C}$ be a congruence on $M$. Now let
$$
S=\{ X^{a}-X^{b} \mid X^{a},\, X^{b} \in M,\, X^{a} \mathbin{\mathcal{C}}X^{b} \}
$$
and let ${} \mathscr{I}({\mathcal{C}}) {}$ be the ideal generated by ${} S$ in ${} \mathbb{Z}[X_{1},\,\dots,\,X_{n}] {}$. We call ${} \mathscr{I}({\mathcal{C}}) {}$ the *congruent ideal corresponding to $\mathcal{C} {}$*.

Conversely, let $I$ be an ideal in ${} \mathbb{Z}[X_{1},\,\dots,\,X_{n}] {}$. Now given ${} X^{a},\, X^{b} \in M {}$, set ${} X^{a} \mathbin{\mathscr{C}(I)} X^{b} {}$ if ${} X^{a}-X^{b} \in I {}$. First note that ${} 0=X^{a}-X^{a} \in I {}$, so $\mathscr{C}(I)$ is reflexive. Now if ${} X^{a}-X^{b} \in I {}$, then ${} -1 \in \mathbb{Z} {}$, so ${} X^{b}-X^{a} \in I {}$, and so ${} \mathscr{C}(I) {}$ is symmetric. Finally, if ${} X^{a}-X^{b} \in I {}$ and ${} X^{b}-X^{c} \in I {}$, then ${} X^{a}-X^{c}=X^{a}-X^{b}+X^{b}-X^{c} \in I {}$, and ${} \mathscr{C}(I) {}$ is transitive and is therefore a equivalence relation. Furthermore, if ${} X^{a}-X^{b} \in I {}$ and ${} X^{c} \in M {}$, then ${} X^{c} \in \mathbb{Z}[X_{1},\,\dots,\,X_{n}] {}$, and so ${} X^{c}(X^{a}-X^{b})=X^{a}X^{c}-X^{b}X^{c} \in I {}$, and ${} \mathscr{C}(I) {}$ is a congruence. 

Now let $\mathcal{C}$ be a congruence, and let ${} \mathcal{D}=\mathscr{C}(\mathscr{I}(\mathcal{C})) {}$. Then if ${} X^{a}\mathbin{\mathcal{C}} X^{b} {}$, then ${} X^{a}-X^{b} \in I_{\mathcal{C}} {}$. Therefore, ${} X^{a} \mathbin{\mathcal{D}}X^{b} {}$. Conversely, if ${} X^{a} \mathbin{\mathcal{D}} X^{b} {}$, then ${} X^{a}-X^{b} \in I_{\mathcal{C}} {}$, and 
$$
X^{a}-X^{b}=p_{1}(X^{a_{1}}-X^{b_{1}})+\dots+p_{n}(X^{a_{n}}-X^{b_{n}})
$$
for some polynomials ${} p_{i} \in \mathbb{Z}[{X_{1},\,\dots,\,X_{n}}] {}$ and monomials ${} X^{a_{i}},\, X^{b_{i}} \in M {}$. We may assume that the coefficients of the ${} p_{i} {}$ are units or zero, as, otherwise, if ${} q {}$ is a non-unit coefficient of the term ${} X^{r} {}$ of ${} p_{i} {}$, then we may write, if ${} q'=\operatorname{sgn}(q) {}$,
$$
\begin{align}
 p_{i}(X^{a_{i}}-X^{b_{i}})  & =\left( p_{i}-qX^{r}+q'\sum _{j=1}^{|q|}  X^{r} \right) (X^{a_{i}}-X^{b_{i}}) \\
 & =(p_{i}-qX^{r})(X^{a_{i}}-X^{b_{i}})+\sum _{j=1}^{|q|}(q'X^{r}(X^{a_{i}}-X^{b_{i}}))
 \end{align}
$$
and now we may assign ${} p'_{j}=p_{j} {}$ if $j\neq i {}$, ${} p'_{i}=p_{i} {}$, and ${} p_{k}'=q'X^{r} {}$ for ${} n+1\leq k\leq |q| {}$. Then this is another valid representation as given above, but without the non-unit coefficient given above.

Now expand out each ${} p_{i}$. If we write
$$
p_{i}=\sum_{j} u_{i,j}X^{p_{i, j}}
$$
for (nonzero) units ${} u_{i,\, j} {}$, then we get
$$
X^{a}-X^{b}=\sum _{i=1}^{n}\sum _{j}u_{i,j}(X^{p_{i,j}+a_{i}}-X^{p_{i,j}+b_{i}})
$$
Then each ${} X^{p_{i,j}+a_{i}}\mathbin{\mathcal{C}}X^{p_{i,j}+b_{i}} {}$, as ${} X^{a_{i}} \mathbin{\mathcal{C}} X^{B_{i}} {}$. We write ${} c_{i,j}=p_{i,j}+a_{i} {}$ and ${} d_{i,j}=p_{i,j}+b_{i} {}$ if ${} u_{i,j}=1, {}$ otherwise we write $c_{i,j}=p_{i,j}+b_{i} {}$ and ${} d_{i,j}=p_{i,j}+a_{i} {}$. Again we have. Finally, since the range of both $i$ and $j$ are finite, then we may reindex such that we have an index $k {}$ running from $1$ to $\ell$ with ${} r_{k}=c_{i,j} {}$ and ${} s_{k}=d_{i,j} {}$. Then finally we may write
$$
X^{a}-X^{b}=\sum _{k=1}^{\ell}(X^{r_{k}}-X^{s_{k}})
$$
Then there exists a finite list ${} (m_{i})_{i=1}^{j} {}$ such that ${} r_{m_{1}}=a {}$ and ${} s_{m_{j}}=b {}$, and ${} r_{m_{i}}=s_{m_{i-1}} {}$ for ${} j\geq i>1 {}$, and so by transitivity, ${} X^{a} \mathbin{\mathcal{C}} X^{b} {}$. Therefore, $\mathcal{C}=\mathcal{D} {}$, and $\mathscr{I}$ is injective. 

Now let ${} \mathcal{C}_{1} \subseteq  \mathcal{C}_{2} \subseteq \dots  {}$ is an infinite chain of congruences. Then ${} \mathscr{I}(\mathcal{C}_{1}) \subseteq \mathscr{I}(\mathcal{C}_{2})\subseteq \dots  {}$ is an infinite chain of ideals. Since ${} \mathbb{Z}[X_{1},\,\dots,\,X_{n}] {}$ is Noetherian, then there exists some $k$ such that ${} \mathscr{I}(\mathcal{C}_{k})=\mathscr{I}(\mathcal{C}_{\ell}) {}$ for all ${} \ell \geq k {}$. Since $\mathscr{I}$ is injective, then ${} \mathcal{C}_{k}=\mathcal{C}_{\ell} {}$ for all $\ell\geq k$, and so the congruences on $M$ satisfy the a.c.c.