---
tags:
  - chapter
  - intro_algebra1
date: 2023-11-06
---
[[Directory]], [[Intro to Algebra 1|Subject Directory]]
# 
## 
### Lemma 1.1
Let $G {}$ be a group
1. There is a *unique* identity element ${} e \in G {}$ such that
$$
eg=ge=g\quad\forall g \in G
$$
2. For all ${} g \in  G {}$ there is a *unique* inverse element ${} h \in G {}$ such that
$$
gh=hg=e\phantom{\quad\forall g \in G}
$$
#### Proof:
1. 
Assume there exist ${} e_{1},\, e_2 \in G$ such that for all ${} g\in G {}$, we have
$$
\begin{align}
e_{1}g=ge_{1}=g \tag{1} \\
e_{2}g=ge_{2}=g \tag{2}
\end{align}
$$
By ${} (1)$, we have
$$
e_{1}e_{2}=e_{2}
$$
By ${} (2)$, we have
$$
e_{1}e_{2}=e_{1}
$$
So we have
$${} e_{1}=e_{1}e_{2}=e_{2} {}$$
So ${} e_{1}=e_{2} {}$, so the identity is unique.
2. 
Assume that given ${} g \in G {}$, there exist ${} h_{1},\, h_{2}\in G$ such that
$$
\begin{align}
gh_{1}=h_{1}g=e \\
gh_{2}=h_{2}g=e
\end{align}
$$
So we have
$$
\begin{align}
gh_{1} & =e &  &  \Rightarrow  \\
h_{2}(gh_{1}) & =h_{2}e &  & \Rightarrow  \\
(h_{2}g)h_{1} & =h_{2}e
\end{align}
$$
We have ${} h_{2}g=e {}$, so
$$
\begin{align}
(h_{2}g)h_{1} =eh_{1} & =h_{2}e \\
 h_{1} & =h_{2}
\end{align}
$$
#### Notation:
By the lemma, given ${} g\in G,\, \exists !h \in G {}$ such that ${} gh=hg=e$. This $h$ is called *the* inverse of $g$ and is written as $g^{-1}$.
#### Note:
If $G$ is a group under addition, we write $-g {}$ instead of $g^{-1}$.
### Proposition 1.2: The Cancellation Law
Let $G$ be a group, and let ${} g,\, h,\, k \in  G {}$. 
1. If ${} gh=gk {}$, then ${} h=k {}$
2. If ${} hg=kg {}$, then ${} h=k {}$
#### Proof:
#todo proof is an exercise on sheet 6.
### Proposition 1.3: Properties of Inverses
Let $G {}$ be a group. Let $g,\, h \in G {}$, with ${} e\in G {}$ being the identity
1. If ${} gh=e {}$, then ${} h=g^{-1} {}$, and $g=h^{-1}$. (Note that this is different from the definition, because it only requires multiplication on one side)
2. $(gh)^{-1}=h^{-1}g^{-1}$. This is sometimes called the "socks and shoes lemma"
3. ${} (g^{-1})^{-1}=g {}$
#### Proof:
1. 
Suppose that $gh=e$. Then we have
$$
\begin{align}
g^{-1}(gh) & =g^{-1}e \\
(g^{-1}g)h & =g^{-1}e \\
eh & =g^{-1}e  \\
h & =g^{-1}
\end{align}
$$
(The proof that $g=h^{-1}$ is similar)
2. 
By part $1.$, we just need to show that 
$$
\begin{align}
(gh)(h^{-1}g^{-1})=e
\end{align}
$$
We have
$$
\begin{align}
(gh)(h^{-1}g^{-1}) & =g((hh^{-1})g^{-1}) \\
 & =g(eg^{-1}) \\
 & =gg^{-1} \\
 & =e
\end{align}
$$
As required, so $(gh)^{-1}=h^{-1}g^{-1} {}$
3. 
This follows immediately from ${} 1. {}$, as ${} g^{-1}g=e {}$. Then $g=(g^{-1})^{-1} {}$
### Definition 1.4
A group ${} (G,\, *) {}$ is called "abelian" if $*$ is commutative. (Also sometimes called commutative, but that is non-standard)
#### Example:
| Abelian                                                 | Nonabelian                  |
| ------------------------------------------------------- | --------------------------- |
| $\mathbb{Z}$                                            | ${} S_{n}\quad(n\geq 3) {}$ |
| ${} \mathbb{Z}_{n} {}$                                  | ${} D_{n}\quad(n\geq 3) {}$ |
| ${} \mathbb{Z}_{n}^{\times} {}$                         | ${} GL_{2}(\mathbb{R})$     |
| ${} \mathbb{Q}^{\times}=\mathbb{Q}\setminus \{ 0 \} {}$ |                             |
| ${} M_{2}(\mathbb{R})$                                                        |                             |

### Definition 1.5: Order
Given a group ${} (G,\, *) {}$, the order of $G$ is the number of elements in the group, which is denoted as $|G| {}$.
## Powers of Group Elements
Let ${} G$ be a group, and let $g \in G$
### Notation:
Given ${} n \in \mathbb{N} {}$, write
$$
g^{n}:=\underbrace{ g g g \dots g }_{ n \text{ times} }
$$
and 
$$
g^{-n}:=\underbrace{ g^{-1}g^{-1}\dots g^{-1} }_{ n \text{ times} }
$$
Finally
$$
g^{0}:=e
$$
This is conveniently the same way we write powers in the real (complex) numbers
### Lemma 2.1
${} (g^{-1})^{n}=(g^{n})^{-1} {}$, for all ${} n \in \mathbb{N} {}$
#### Proof:
#todo In homework
### Proposition 2.2: Law of Exponents
Let $G$ be a group, ${} g \in G {}$, and $m,\, n \in\mathbb{Z}$. Then
1. ${} g^{m}g^{n}=g^{m+n} {}$
2. ${} ( g^{m} )^{n}=g^{mn} {}$
#### Proof:
1. 
If ${} m,\, n\geq 1 {}$, this is clear by definition
If ${} m,\, n\leq 1 {}$, this is also clear by definition
If ${} m=0 {}$, then
$$
g^{m}g^{n}=eg^{n}=g^{n}=g^{0+n}
$$
If ${} n=0$, then the proof is the same
We now only need to consider the case when one of ${} m,\, n {}$ is positive, and the other is negative. WLOG, assume ${} m<0 {}$ and $n>0$. We now have even more *sub*cases (holy shit)
Case 1: $m+n\geq 0 {}$
Then consider
$$
\begin{align}
 g^{\underbrace{ -m }_{ \geq 0 }}g^{\underbrace{ m+n }_{ \geq 0 }} & =g^{-m+m+n}   \\
 & =g^{n} \\
\text{So }g^{-m}g^{m+n} & =g^{n}
 \end{align}
$$
So we have
$$
\begin{align}
 g^{m}(g^{-m}g^{m+n})  & =g^{m}g^{n} \\
eg^{m+n} & =g^{m}g^{n} \\
g^{m+n} & =g^{m}g^{n}
 \end{align}
$$
As required
Case 2: ${} m+n<0 {}$
This proof well be almost exactly the same as the above. Now we have
$$
\begin{align}
 g^{\underbrace{ m+n }_{ <0 }}g^{\underbrace{ -n }_{ <0 }} & =g^{m+n-n}=g^{m}   \\
	(g^{m+n}g^{-n})g^{n} & =g^{m}g^{n} \\
 g^{m+n} & =g^{m}g^{n}
 \end{align}
$$
And the proof is exactly the same if $m>0 {}$ and $n<0$
2. 
#todo Homework on sheet $6$
#### Note:
If the operation on $G$ is addition, we write $ng {}$ instead of ${} g^{n}$.
### Definition 2.3: Order of Group elements
Let $G$ be a group with identity $e$. Let $g \in G$.
- If for all ${} n \in  \mathbb{N} {}$, ${} g^{n}\neq e$, then we say that $g$ has infinite order
- If $g$ does not have infinite order, then the order of $g$ is 
$$
\operatorname{ord}(g)=\min\{ n \in\mathbb{N}\mid g^{n}=e \}
$$
### Lemma 2.4
Let ${} g=(a_{1}\; a_{2}\; \dots\; a_{k})\in S_{n}$ be a $k {}$-cycle. Then ${} \operatorname{ord}(g)=k {}$
#### Proof:
Claim 1: $g^{k}=e$. We work slightly sloppily. Note that
$$
\begin{align}
 g(a_{1})  & =a_{2}  \\
g^{2}(a_{1}) & =a_{3} \\ \\
 & \vdots \\

g^{n}(a_{1}) & =a_{n+1} \\
\end{align}
$$
So we have
$$
\begin{align}
g^{k-1}(a_{1})=a_{k} \\
g^{k}(a_{1})=a_{1}
\end{align}
$$
For other elements, we can do this
$$
\begin{align}
 g^{k}(a_{2})  & =g^{k}(g(a_{1})) \\
 & =g^{k+1}(a_{1})=g(a_{1})=a_{2} 
 \end{align}
$$
In general, we have ${} g^{k}(a_{j})=a_{j} {}$
If ${} b\notin\{ a_{1},\,\dots,\,a_{k} \} {}$, then
$$
\begin{align}
g(b) & =b \\
g^{k}(b) & =b
\end{align}
$$
So ${} g^{k}=e {}$
Claim 2: if $1\leq l<k {}$, then $g^{l}\neq e$
$$