---
tags:
  - intro_algebra1
  - chapter
date: 2023-11-13
---
[[Directory]], [[Intro to Algebra 1|Subject Directory]]
### First some notation
Write $H\leq G$ means "$H$ is a subgroup of $G$". We also write $H<G$ if $H\leq G$ and $H\neq G$
Throughout the lecture, let ${} (G, *) {}$ be a group with identity element $e {}$.
# Subgroups
## Subgroup Testing
### Theorem 1.1: The (3 Step) Subgroup Test
Let ${} H\subseteq G {}$. Then $H\leq G {}$ iff these 3 conditions hold:
1. If ${} a,\, b \in H {}$, then $ab\in H {}$
2. $e \in H {}$
3. If ${} a \in H {}$, $a^{-1}\in H$
#### Proof:
First we prove ${} (\Leftarrow)$. Assume the 3 conditions hold. By 1, $*$ is a binary operation on $H$, by definition. We see that $*$ is associative on $G$. Therefore, since every element ${} a,\, b,\, c\in H$ is also ${} a,\, b,\, c \in G$, and so ${} a(bc)=(ab)c$, as $G$ is a group. Therefore, $*$ is associative on $H$.
By 2, we assert that $H$ contains an identity element.
Finally, by 3, we assert that for all elements ${} x \in H {}$, ${} x^{-1} \in H$, therefore, every element has an inverse in $H$. 
Therefore, $H\leq G {}$

Now we prove $(\Rightarrow )$. Assume we have $H\leq G$. Since $H$ is a subgroup, then $*$ must be a binary operation on $H$. Therefore, condition 1 holds. Since $H$ is a group, it contains an identity element, call it ${} e_{H} {}$. 
Since ${} e_{H} {}$ is an identity for $H$, we have
$$
e_{H}*e_{H}=e_{H}
$$But then, since $e$ is an identity for $G$, we have 
$$
e*e_{H}=e_{H}
$$Now we have
$$
e_{H}*e_{H}=e*e_{H}
$$
Therefore, by the cancellation law, we see that $e_{H}=e$, so we see that the second condition holds.
Finally, let ${} h \in H {}$. Since $H {}$ is a (sub)group, then ${} \exists k \in H$ such that $hk=e=kh$. We proved that this implies that ${} k=h^{-1}$. Therefore, the ${} 3^{\mathrm{rd}}$ condition holds.
#### Example:
Let $G$ be any group, and let 
$$
H=\{ e \}
$$Claim: $H\leq G$.
We check the 3 conditions:
1. ${} a,\, b \in H\Rightarrow a=b=e$, and ${} ee=e\in H {}$
2. ${} e \in H$ as ${} H=\{ e \} {}$
3. ${} a \in H\Rightarrow a=e, e^{-1}=e \in H {}$
Therefore, $H\leq G {}$. This is called the trivial subgroup
## Cyclic Subgroups
### Proposition 1.2 
Let ${} g \in G$. Then ${} \langle g \rangle  {}$ is a subgroup of $G {}$.
#### Proof:
We use the subgroup test
1. Let ${} x,\, y \in \langle g \rangle  {}$. Then, by definition, ${} \exists n,\, m \in \mathbb{Z} {}$ such that
$$
x=g^{n},\, \qquad y=g^{m}
$$
So
$$
xy=g^{n}g^{m}=g^{n+m}\in \langle g \rangle 
$$
As ${} n+m \in \mathbb{Z} {}$
2. ${} e=g^{0} {}$, ${} 0 \in \mathbb{Z} {}$, so ${} e \in \langle g \rangle  {}$
3. Let ${} x \in \langle g \rangle  {}$. Then ${} x=g^{n}$ for some ${} n \in \mathbb{Z}$. Now note that
$$
x^{-1}=x^{-n}\in \langle g \rangle 
$$ as ${} -n \in \mathbb{Z} {}$ too.
So by the subgroup test, $\langle g \rangle \leq G$, as required.
### Definition 1.3: Cyclic Subgroups
${} \langle g \rangle  {}$ is called the subgroup generated by $g$. A subgroup of the form ${} \langle g \rangle  {}$ is called a cyclic subgroup. 

#### Examples:
${} \{ e \}=\langle e \rangle  {}$ is a cyclic subgroup
We see that ${} \{ [0]_{6},\, [2]_{6},\, [4]_{6} \} {}$ is a cyclic subgroup of $$