---
tags:
  - intro_algebra1
  - chapter
date: 2023-11-30
---
[[Directory]], [[Intro to Algebra 1|Subject Directory]]
# 
## 
### Corollary 1.1:
Let $G$ be a group of order $n$ with identity $e$. Then ${} g^{n}=e {}$ for all ${} g \in G {}$.
#### Proof:
Let ${} g \in G {}$. By corollary from monday #todo , ${} |g| \mid n {}$. Let ${} d=|g| {}$. Then ${} n=dk {}$ for some ${} k \in \mathbb{Z}. {}$ Then $g^{n}=g^{dk}=( g^{d} )^{k}=e^{k}=e {}$.
### Theorem 1.2: Fermat's Little Theorem
Let ${} a \in \mathbb{Z} {}$ and let $p$ be a prime. Then 
1. ${} a^{p}\equiv a \:(\mathrm{mod}\  p)  {}$
2. If ${} p \nmid a {}$, then ${} a^{p-1}\equiv 1 \:(\mathrm{mod}\  p)  {}$
#### Proof:
2. 
We prove 2 first. Lets look at the group ${} G=\mathbb{Z}_{p}^{\times } {}$. First note that ${} |G|=p-1 {}$. Now we have, by ${} 1.1 {}$, for all ${} a \in G {}$, then ${} a^{p-1}=[1]_{p} {}$. A number ${} a \in \mathbb{Z} {}$ is an element of ${} G$ iff ${} p\nmid a {}$, so we have
$$
( [a]_{p} )^{p-1}=[1]_{p}
$$
Therefore, ${} a^{p-1}\equiv 1\:(\mathrm{mod}\  p)  {}$

1. 
Case 1:
${} p\nmid a {}$. Then ${} a^{p-1}\equiv 1\:(\mathrm{mod}\  p)  {}$, so ${} a^{p}\equiv a \:(\mathrm{mod}\  p)  {}$
Case 2:
${} p\mid a {}$. Then ${} a\equiv 0\:(\mathrm{mod}\  p)  {}$, so ${} a^{p}\equiv 0\equiv a\:(\mathrm{mod}\  p)  {}$

#### Side Note:
For general ${} n$, ${} |\mathbb{Z}_{n}^{\times }|=\varphi(n) {}$, where $\varphi {}$ is Euler's totient function.
So we get, in general, ${} \gcd(a,\, n)=1 {}$, then ${} a^{\varphi(n)}\equiv 1\:(\mathrm{mod}\  n)  {}$

#### Example:
Find the remainder when ${} 200^{600} {}$ is divided by by $7$.
$${} 200^{600}=(200^{100})^{6} {}$$
and
$$
7\nmid 200^{100}\Rightarrow (200^{100})^{6}\equiv 1 \:(\mathrm{mod}\  7) 
$$
# Ring Theory
## Introduction
### Definition 2.1: Rings
A *ring* is a set ${} R$ with *2* binary operations, $+$ and $*$, satisfying $3 {}$ properties
1. ${} (R, +) {}$ is a commutative group.
2. ${} * {}$ is associative and has an identity element, i.e. ${} (R, *) {}$ is a monoid.
3. Distributive property: given ${} r,\, s,\, t \in R {}$:
$$
r*(s+t)=r*s+r*t
$$
and
$$
(s+t)*r=s*r+t*r
$$
#### Example:
$\mathbb{Z}$ form a ring with addition and multiplication. 