---
tags:
  - chapter
  - intro_algebra1
date: 2023-10-16
---
[[Directory]], [[Intro to Algebra 1|Subject Directory]]
# Symmetric and Cyclic Groups
## Permutations
### Definition 1.1
A permutation of ${} S=\{ 1,\, 2,\,\dots,\,n \} {}$ is just a bijective function ${} f:S\to{} S$.

Write ${} S_{n} {}$ as the set of all permutations on ${} \{ 1,\, 2,\,\dots,\,n \} {}$.

Example:
${} S_{2}=\{ e,\, f \} {}$
There are 2 permutations:
${} e:\{ 1,\, 2 \}\to{} \{ 1,\, 2 \} {}${} , ${} 1\mapsto 1 {}$ and $2\mapsto 2 {}$
${} f:\{ 1,\, 2 \}\to{} \{ 1,\, 2 \} {}${} , $1\mapsto 2 {}$ and $2\mapsto 1 {}$

#### Notation:
We write ${} e\in S_{n} {}$ given by ${} e(x)=x\quad\forall x \in \{ 1,\, 2,\,\dots,\,n \} {}$

We have 2 main types of notation for ${} S_{n} {}$.
The ${} 1^{\mathrm{st}} {}$ notation: write ${} f \in  S_{n} {}$ as
$$
\begin{pmatrix}1&2&\dots&k\\ f(1) & f(2) &\dots& f(k) \end{pmatrix} 
$$
For example, for ${} n=4 {}$
$$
f=\begin{pmatrix}1&2&3&4\\ 2 & 4 & 3 & 1 \end{pmatrix} 
$$
THis means ${} f(1)=2,\, f(2)=4,\, f(3)=3,\, f(4)=1 {}$. Here, the bottom row is a reordering of ${} \{ 1,\,\dots,\,n \} {}$

The second notation is called cycle notation
Let ${} \{ a_{1},a_{2},\,\dots,\,a_{k} \}\subseteq \{ 1,\, 2,\,\dots,\,n \} {}$, and we have ${} a_{i}\neq a_{j}\quad\forall i\neq j {}$
We write
$$
(a_{1}\;a_{2}\;\dots\;a_{k})
$$
For the Function ${} f\in S_{n} {}$ defined by
$$
\begin{align}
f(a_{1}) & =a_{2} \\
f(a_{2}) & =a_{3} \\
 & \vdots \\
f(a_{k}) & =f(a_{1})
\end{align}
$$
and ${} f(x)=x {}$ for all ${} x\notin\{ a_{1},\,\dots,\,a_{k} \} {}$

#### Example:
let ${} f=(1\;5\;3)\in S_{5} {}$. Then 
$$
\begin{align}
f(1) & =5 \\
f(2) & =2 \\
f(3) & =1 \\
f(4) & =4 \\
f(5) & =3
\end{align}
$$
#### Note:
${} (a_{1}\;a_{2}\;\dots a_{k}\;) {}$ is called a $k {}$-cycle (or just cycle)

#### Note
A ${} 1 {}$-cycle is identical, i.e. ${} (a)=e {}$

### The Size of ${} S_{n} {}$
Fact: $S_{n}$ contains $n! {}$ elements, i.e. the number of bijective functions
Why? We have $n$ choices for ${} f(1)$, ${} n-1 {}$ choices for ${} f(2)$, and so on. Multiplying up, we get ${} \#S_{n}=n(n-1)\dots 2\cdot 1=n! {}$
### Composition
Take ${} f,\, g\in S_{n} {}$, then
$$
f\circ g:\{ 1,\, 2,\,\dots,\,n \}\to{} \{ 1,\, 2,\,\dots,\,n \}
$$
and ${} f\circ g {}$ is bijective. Therefore, $f\circ g\in S_{n}$, so $\circ {}$ is a binary operation on $S_{n} {}$

#### Notation:
instead of writing ${} f\circ g {}$, we write $fg {}$, and write ${} \underbrace{ f\circ f\circ \dots \circ f }_{ k \text{ times} } {}$ as $f^{k} {}$
If ${} f=(a_{1}\;\dots\;a_{k}) {}$ and ${} g=(b_{1}\;\dots\;b_{m}) {}$ are cycles, then write
$$
f\circ g=(a_{1}\;\dots\;a_{k})(b_{1}\;\dots\; b_{k})
$$

#### Example:
$f=(1\; 4\; 2)(1\; 3)\in S_{4}$
$$
\begin{align}
 f(1) & :1\to{(1\; 3)}3\to{(1\; 4\; 2)}3\qquad &  & \Rightarrow f(1)=3\\
 f(2) & :2\to{(1\; 3)}2\to{(1\; 4\; 2)}1  &  & \Rightarrow f(2)=1 \\
f(3) & :3\to{(1\; 3)}1\to{(1\; 4\; 2)}4  &  &  \Rightarrow f(3)=4 \\
 \end{align}
$$
Note that we don't even need to complete the process with ${} f(4) {}$, as its a bijection we immediately know that ${} f(4)=2 {}$, as its the only number that hasn't been used.

### Definition 1.2
Take 2 cycles ${} f=(a_{1}\; \dots\; a_{k})$ and ${} g=(b_{1}\; \dots\; b_{k})$ are called **disjoint** if
$$
\{ a_{1},\,\dots,\,a_{k} \}\cap \{ b_{1},\,\dots,\,b_{m} \}=\varnothing
$$

#### Example: 
In $S_{4}$ ${} (1\; 2) {}$ and ${} (3\; 4)$ are disjoint, but ${} (1\; 2) {}$ and ${} (1\; 4\; 2) {}$ are not disjoint

#### Fact:
Every ${} f\in S_{n} {}$ can be written as a composition (or product) of disjoint cycles
We will *not* prove this in this course

#### Example:
$f=\begin{pmatrix}1&2&3&4&5&6\\ 3 & 4 & 1 & 5 & 6 & 2 \end{pmatrix} {}$
Write ${} f {}$ as disjoint cycles:
${} f=(1\;3)(2\;4\;5\;6) {}$

The process is as follows:
We start with ${} 1$. We see that $1$ maps to $3$, so we list $3$ next. We then see that $3$ maps back to $1$, so we close the cycle. We then start with the next smallest number that has not been listed. We see that ${} 2\mapsto4$, ${} 4\mapsto 5 {}$, $5\mapsto 6$ and $6\mapsto 2$. As we have hit another loop, we close this cycle. As all numbers have been listed, we are now done

Another
$f=(1\; 4\; 2)(1\; 3)$. These are not disjoint. We work by the same process
${} f=(1\; 3\; 4\; 2)$. 

Another
${} f=(1\;3)(1\;2)(2\;4) {}$
then
$f=(1\;2\;4\;3)$

## Modular Arithmetic
### Congruences
Let ${} a,\, b\in \mathbb{Z} {}$ and ${} n \in  \mathbb{N}$. We say that ${} a {}$ is congruent to $b$ modulo $n$, if
$$
n\mid(a-b)
$$
Notation:
$$
a\equiv b\:(\mathrm{mod}\  2) 
$$
#### Examples:
take ${} n=10 {}$ and ${} a=3 {}$
then we have
$$
\begin{align}
3\equiv 13\equiv 23\equiv 33\equiv\dots\:(\mathrm{mod}\  10) 
\end{align}
$$
Because ${} 3-13=-10$ and ${} 10\mid-10 {}$ etc

and
$$
3\equiv-7\equiv-17\equiv-27\equiv\dots \:(\mathrm{mod}\  10) 
$$
Now take ${} n=2 {}$.
Then ${} m\equiv 0\:(\mathrm{mod}\  2)  {}$ iff $m$ is even
and 
${} m\equiv 1\:(\mathrm{mod}\  2)  {}$ iff ${} m {}$ is odd

### Proposition 2.1
Let ${} a,\, b \in  \mathbb{Z} {}$ and ${} n \in  \mathbb{N} {}$. The following are equivalent
1. ${} a\equiv b\:(\mathrm{mod}\  n)  {}$
2. ${} a=kn+b {}$ for some $k\in \mathbb{Z} {}$
3. ${} a$ and $b {}$ have the same remainder when dividing by ${} n {}$

#### Proof:
We look at ${} 1\Rightarrow 2 {}$. Assume that ${} a\equiv b\:(\mathrm{mod}\  n)  {}$  By definition of congruence ${} \:(\mathrm{mod}\  n)  {}$, 
$$
\begin{align}
 &n\mid(a-b)   \\
 & \Rightarrow a-b=nk
 \end{align}
$$
for some ${} k \in  \mathbb{Z} {}$
Therefore
$$
a=bk+b
$$
therefore, ${} 3 {}$

Next, ${} 2\Rightarrow 3 {}$. Assume $a=kn+b$ for some ${} k \in  \mathbb{Z} {}$. Use the division algorithm to write
$$
a=qn+r\qquad q,\, r \in  \mathbb{Z},\, 0\leq r<n
$$
Therefore
$$
\begin{align}
kn+b=qn+r \\
b=(q-k)n+r
\end{align}
$$
Therefore, ${} r$ is also the remainder when dividing $b$ by $n {}$

Finally, ${} 3\Rightarrow 1$. Assume $a$ and $b$ have the same remainder when dividing by $n {}$. 
Therefore, ${} \exists q_{1},\, q_{2}\in \mathbb{Z} {}$ and ${} r\in \mathbb{Z},\, 0\leq r<n {}$ such that
$$
\begin{align}
a & =q_{1}n+r \\
b & =q_{2}n+r \\
\Rightarrow a-b & =(q_{1}-q_{2})n \\
\Rightarrow n & \mid(a-b) \\
\Rightarrow a & \equiv b\:(\mathrm{mod}\  n) 
\end{align}
$$
### Proposition 2.2
Let $a,\, b,\, C\in  \mathbb{Z}$ and ${} n \in  \mathbb{N} {}$, then:
1. if ${} a\equiv b\:(\mathrm{mod}\  n)  {}$, then ${} b\equiv a \:(\mathrm{mod}\  n)  {}$
2. if ${} a\equiv b\:(\mathrm{mod}\  n) {}$ and ${} b\equiv c\:(\mathrm{mod}\  n)  {}$. Then ${} a\equiv c \:(\mathrm{mod}\  n)  {}$
3. ${} a\equiv a\:(\mathrm{mod}\  n) {}$
These are mostly homework questions

### Proposition 2.3
Let ${} a,\, b,\, c,\, d\in \mathbb{Z}$, and $n \in\mathbb{N} {}$. Assume $a\equiv b\:(\mathrm{mod}\  n)$ and ${} c\equiv d\:(\mathrm{mod}\  n) {}$
Then
1. ${} a+c\equiv b+d\:(\mathrm{mod}\  n)  {}$
2. ${} ac=bd\:(\mathrm{mod}\  n)  {}$

#### Proof:
1. 
${} a\equiv b\:(\mathrm{mod}\  n) \Rightarrow a=nk+b {}$ for some ${} k \in  \mathbb{Z} {}$
and
${} c\equiv d\:(\mathrm{mod}\  n) \Rightarrow c=nm+d {}$ for some ${} m \in \mathbb{Z} {}$

Then we have
${} a+c=(\underbrace{ k+m }_{ \in \mathbb{Z} })n+(b+d) {}$
Therefore, by the equivalence, 
$$
a+b\equiv b+d\:(\mathrm{mod}\  n) 
$$
2. 
Still have
${} a=nk+b {}$ and ${} c=nm+d {}$

then
$$
\begin{align}
ac & =(kn+b)(mn+d) \\
 & =kmn^{2}+(k+n)n+bd \\
 & =n(\underbrace{ kmn+k+m }_{ \in \mathbb{Z} })+bd \\
\Rightarrow ac & \equiv bd\:(\mathrm{mod}\  n) 
\end{align}
$$
### Definition 2.4
Given ${} a \in  \mathbb{Z}$, and $n \in\mathbb{N} {}$, let
$$
[a]_{n}=\{ b\in \mathbb{Z}\mid a\equiv b\:(\mathrm{mod}\  n)  \}
$$
and let
$$
\mathbb{Z}_{n}=\{ [a]_{n}\mid a\in \mathbb{Z} \}
$$
We say $[a]_{n}$ is called the congruence class of $a$ modulo $n$

#### Example:
${} [3]_{10}=\{ \dots,\, -17,\, -7,\, 3,\, 13,\, 23,\, \dots \}= {}$

By the proposition, 
$$
[a]_{n}=\{ nk+a\mid k\in \mathbb{Z} \}
$$
and
$$
\begin{align}
[0]_{n} & ={2k\mid k\in \mathbb{Z}} \\
[1]_{n} & =\{ 2k+1 \mid k \in  \mathbb{Z} \}
\end{align}
$$
etc.