---
tags:
  - chapter
  - calculus1
date: 2023-10-05
---
[[Directory]], [[Calculus 1|Subject Directory]]
# Graph Sketching
## Recap
### Key techniques
- First Principles
- Link to known example
- Axis Intercepts
- When is graph positive or negative
- Asymptotes
- Behaviour of function as $x\to{} \infty$ and $x\to{}-\infty$
- Discontinuities
- Turning points

Example: Sketch
$$
f:\mathbb{R}\to{} \mathbb{R}, f(x)=\begin{cases}
-&10& \qquad x\leq-2 \\
-&x& \qquad x \in (-2,\,  2) \\
&x& \qquad x\geq 2
\end{cases}
$$

![[Pasted image 20231005091909.png]]

Example: Sketch
$$
f:\mathbb{R}\setminus \{ 2 \}\to{} \mathbb{R}, \quad f(x)=\frac{1}{x-2}
$$
We can link to a known example:
![[Pasted image 20231005092356.png]]
Since we know what $\displaystyle \frac{1}{x}$ looks like

Example: Sketch
$$
\begin{align}
f & :\mathbb{R}\setminus \{ 2,\, 3 \}\to{} \mathbb{R} \\
f(x) & =\frac{x^{3}+1}{(x-3)(x+2)}
\end{align}
$$
This is called a rational function

First: Axis intercepts
$\displaystyle f(0)=-\frac{1}{6}$

If $f(x)=0$, then $x^{3}=-1$, then $x=-1$

Second: Asymptotes
Occur at $x=3,\,x=-2$
if $x>3$, then $x^{3}+1,\,(x-3),\,(x+2)>0$, so $f(x)>0$
if $-1<x<3$, then $x^{3}+1,\,(x+2)>0$, but $(x-3)<0$ so $f(x)<0$
if $-2<x<-1$, then $x^{3}+1,\,(x-3)<0$, but $(x+2)>0$, so $f(x)>0$
if $x<-2$, then $x^{3}+1,\,(x-3),\,(x+2)<0$, so $f(x)<0$

By Polynomial division, we can have
$$
\begin{align}
f(x) & =x+1+\frac{7x+7}{x^{2}-x-6} \\
 & =x+1+ \frac{7+\frac{7}{x}}{x-1-\frac{6}{x}}
\end{align}
$$
The last term gets very small as $x$ gets large, therefore, $f(x)$ is asymptotic to $x+1$ as $x$ gets very large.
So, we get this graph
![[Pasted image 20231005094513.png]]


# Exponents
## Recap of High School
### Definition 2.1
Let $n \in \mathbb{N}$ and $x \in \mathbb{R}$. Then define
$$
x^{n}=\underbrace{ x \cdot x\cdot x\cdot x{\cdot} {\dots} \cdot x }_{ n \text{ times} }
$$
### Interactions with multiplication and division
Given $n,\, m \in \mathbb{N}$
$$
\begin{align}
x^{n}x^{m} & =\underbrace{ (x\cdot{\dots}\,\cdot x) }_{ n \text{ times} } \cdot \underbrace{ (x\cdot{\dots}\,\cdot x) }_{ m \text{ times} } \\
 & =x^{m+n}
\end{align}
$$
$$
\begin{align}
\frac{x^{n}}{x^{m}} & =\frac{\underbrace{ (x\cdot{\dots}\,\cdot x) }_{ n \text{ times} }}{\underbrace{ (x\cdot{\dots}\,\cdot x) }_{ m \text{ times} }} \\
 & =x^{n-m}
\end{align}
$$

### Definition 2.2
(Informed by above)
Define for $m \in \mathbb{N}$
$$
x^{-m}:= \frac{1}{x^{m}}
$$

and $x^{0}:=1$

Exercise: Show with this definition that $\forall n, m \in \mathbb{Z}$
$$
x^{n}x^{m}=x^{n+m}
$$
