---
tags:
  - chapter
  - geotop1
date: 2024-10-14
---
[[Directory]], [[University/Undergraduate/Second Year/Geometric Topology 1/Geometric Topology 1|Subject Directory]]
[[1. Review of topology and intro to knots|ðŸž€ðŸž€]] [[University/Undergraduate/Second Year/Geometric Topology 1/Lectures/6. |â—€]] [[University/Undergraduate/Second Year/Geometric Topology 1/Lectures/8. |â–¶]] [[University/Undergraduate/Second Year/Geometric Topology 1/Lectures/22. |ðŸž‚ðŸž‚]]
(Correction from last lecture) #todo watch it
If ${} A,\, B, \in \mathbb{Z}^{c,\, c} {}$, then $A \sim B {}$ means that $PAQ=B {}$ where ${} \det  P=1=\det  Q {}$, and 
$$
\begin{pmatrix}1 & 0 \\ 0 & 12 \end{pmatrix} \sim \begin{pmatrix}3 & 0 \\ 0 & 4 \end{pmatrix} \not \sim \begin{pmatrix}2 & 0 \\ 0 & 6 \end{pmatrix} 
$$
as ${} 2,\, 6 {}$ are not coprime. 
# 
## Kauffman Bracket 
It's a Laurent polynomial in the variable ${} A$ that is generated by a link diagram, $D$, which is often written as
$$
\langle D \rangle =\framebox{D}=\operatorname{kb}(D)
$$
### Rules
Rules that determine the Kauffman bracket:
1. If $D=S_{1} {}$, then ${} \framebox{D}=1 {}$
2. If ${} D' = S_{1} \sqcup D {}$, then ${} \framebox{D'}=-(A^{2}+A^{-2})\framebox{D}=Z\framebox{D} {}$
3. Given a crossing in a diagram, then we represent the K.B. diagrammatically:
![[Pasted image 20241014162400.png]]
#### Example:
Let $F$ be a knot diagram, and let 
![[Pasted image 20241014162809.png]]
Now rule $3$ implies that
![[Pasted image 20241014163033.png]]
and rule $2$ implies that
![[Pasted image 20241014163252.png]]
Note that $D' {}$ is $D$ with a $-1 {}$ twist. We also get that
$$
(-A)^{3} \framebox{D'}=\framebox{D}
$$
and that, if ${} w=\operatorname{writhe}(D) {}$, then
$$
(-A)^{3-3w} \framebox{D'}=(-A)^{-3w} \framebox{D}=(-A)^{-3w'}\framebox{D'}
$$
where ${} w'=w-1 {}=w(D') {}$. It follows that 
$$
(-A)^{-3w(D)} \framebox{D}
$$
is invariant by R1 moves. We will show later that it is also invariant by R2 and R3 moves. This is essentially the Jones polynomial, once we substitute ${} t=A^{-4} {}$ (some people use $q {}$ instead of $t {}$). 
#### Example:
The Hopf link:
![[Pasted image 20241014163937.png]]
We compute the Kauffman Bracket of the Hopf link like so:![[Pasted image 20241014164223.png]]
Since the first term has positive writhe and the second has negative writhe, then we get that 
$$
\begin{align}
 &  =  A(-A^{3})+A^{-1}(-A^{-3}) \\
 & =-A^{4}-A^{-4}
 \end{align}
$$
Now the jones polynomial of the Hopf link, note that it depends on the orientation of the link. We orient like so:
![[Pasted image 20241014164629.png]]
And so 
$$
\begin{align}
 V(\text{right Hopf link}) & =(-A)^{-3w}(-A^{4}-A^{-4}) \\
 & =A^{-6}(-A^{4}-A^{-4}) \\
 & =-A^{-2}-A^{-10} \\
 & =-t^{1/2}-t^{5 /2}  
 \end{align}
$$
In general, if $L$ is a link diagram, then ${} V(L)(1)=(-2)^{\ell-1} {}$, where $\ell {}$ is the number of connected components of ${} L$.
### Proposition 1.1: 
The Kauffman bracket is invariant under R2 moves: Consider
![[Pasted image 20241014171334.png]]
### Proposition 1.2:
The Kauffman bracket is invariant under R3 moves: consider
![[Pasted image 20241014171849.png]]
Therefore, the Jones polynomial is invariant under R-moves
#### Example:
Consider the link
![[Pasted image 20241014172156.png]]
Now since the Jones polynomial is invariant under R-moves, then 
$$
V(L)=V(S^{1} \sqcup S^{1})=-A^{2}-A^{-2}=-t^{-1/2}-t^{1/2}
$$
## Skein Relation for the Jones Polynomial
### Proposition 1.3:
The Skein Relation concerns oriented links. We start with a section of a diagram, call the link ${} L_{+} {}$, since the writhe is positive: 
![[Pasted image 20241014172901.png|200]]
Since the orientation must be preserved, the there is only 1 way to split the crossing, call it ${} L_{0}: {}$ 
![[Pasted image 20241014173048.png|200]]
Otherwise, we reverse the link, and call it ${} L_{-} {}$, since the writhe is negative:
![[Pasted image 20241014173243.png|200]]
Now set ${} z=t^{1/2}-t^{-1/2} {}$. Then the Skein Relation says that
$$
t^{-1}V(L_{+})-tV(L_{-})=zV(L_{0})
$$
### Example:
We split the boxed link like so:
![[Pasted image 20241014174109.png]]

and therefore, 
$$
\begin{align}
 t^{-1}V(4_{1}) & =zV(L_{0})+t\cdot 1 \\
 & =(t^{1/2}-t^{-1/2})(-t^{-1/2}-t^{-5/2})+t   \\
 & =t^{2}+(t^{3/2}-t^{1/2})(-t^{1/2}-t^{-5/2}) \\
 & =t^{2}-t-t^{-1}+1+t^{-2} \\
 & =t^{-2}-t^{-1}+1-t+t^{2}
 \end{align}
$$
