---
tags:
  - chapter
  - numtheory1
date: 2024-11-08
---
[[Directory]], [[University/Undergraduate/Second Year/Introduction to Number Theory 1/Introduction to Number Theory 1|Subject Directory]]
[[University/Undergraduate/Second Year/Introduction to Number Theory 1/Lectures/1. Introduction|ðŸž€ðŸž€]] [[11. Primitive Roots in Prime Powers, and Quadratic Residues|â—€]] [[University/Undergraduate/Second Year/Introduction to Number Theory 1/Lectures/13. |â–¶]] [[University/Undergraduate/Second Year/Introduction to Number Theory 1/Lectures/22. |ðŸž‚ðŸž‚]]
# Quadratic Residues
### Question:
For which primes ${} p {}$ does ${} x^{2}+1\equiv 0 \:(\mathrm{mod}\  p)  {}$ have a solution in ${} \mathbb{Z}_{p} {}$. 
### Theorem 1.1:
We have ${} -1 {}$ as a QR iff ${} p\equiv 1\:(\mathrm{mod}\  4)  {}$.
#### Proof:
Let $g$ be a primitive root ${} \:(\mathrm{mod}\  p)  {}$, and let ${} y=g^{\frac{p-1}{2} } {}$. Assume that $p>2 {}$. Observe that ${} y^{2}=g^{p-1}\equiv 1\:(\mathrm{mod}\  p)  {}$, thanks to Fermat's little theorem. Therefore, ${} y\equiv 1 {}$ or ${} y\equiv -1 \:(\mathrm{mod}\  p)  {}$. Now we know that ${} g^{\frac{p-1}{2}  }\not\equiv 1\:(\mathrm{mod}\  p) {}$, since $g$ is a PR. Therefore, ${} g^{\frac{ p-1 }{ 2 }}\equiv -1 \:(\mathrm{mod}\  p)  {}$. 

Now consider ${} x^{2}\equiv -1 \:(\mathrm{mod}\  p)  {}$. Then $-1 {}$ is a QR iff ${} -1\equiv g^{i} \:(\mathrm{mod}\  p)  {}$ and $i$ is even. Since ${} i=\frac{ p-1 }{ 2 } {}$, and so $-1 {}$ is a QR iff ${} \frac{ p-1 }{ 2 } {}$ is even, and so ${} p=4k+1 {}$. 
## Euler's Criterion
### Theorem 1.2: Euler's Criterion
Let ${} b \in \mathbb{Z} {}$ and let $p>2 {}$ be an odd prime. with ${} \gcd(p,\, b)=1 {}$. Then each of the following hold:
1. $b$ is a QR modulo $p$ iff ${} b^{\frac{ p-1 }{ 2 }}\equiv 1\:(\mathrm{mod}\  p)  {}$
2. $b$ is a QNR modulo $p$ iff ${} b^{\frac{ p-1 }{ 2 }}\equiv -1\:(\mathrm{mod}\  p)  {}$
#### Proof:
Let $g$ be a PR modulo ${} p {}$, and write ${} b\equiv g^{i}\:(\mathrm{mod}\  p)  {}$. Consider ${} b^{\frac{ p-1 }{ 2 }}=(g^{i})^{\frac{ p-1 }{ 2 }}=\left(  g^{\frac{ p-1 }{ 2 }}  \right)^{i} {}$. Therefore
$$
b^{\frac{ p-1 }{ 2 }}\equiv (-1)^{i} \:(\mathrm{mod}\  p) 
$$
If $i$ is even, then ${} (-1)^{i}=1 {}$, and ${} -1 {}$ otherwise. Therefore, ${} b=g^{i} {}$ 