---
tags:
  - chapter
  - numtheory1
date: 2024-10-11
---
[[Directory]], [[University/Undergraduate/Second Year/Introduction to Number Theory 1/Introduction to Number Theory 1|Subject Directory]]
[[University/Undergraduate/Second Year/Introduction to Number Theory 1/Lectures/1. Introduction|ðŸž€ðŸž€]] [[5. Multiplicative Groups and Hensel's Lemma|â—€]] [[University/Undergraduate/Second Year/Introduction to Number Theory 1/Lectures/7. |â–¶]] [[University/Undergraduate/Second Year/Introduction to Number Theory 1/Lectures/22. |ðŸž‚ðŸž‚]]
# Hensel's Lemma
## Part 2
Recall that ${} f(x)=c_{n} x^{n}+\dots+c_{1}x+c_{0} {}$ with ${} c_{i} \in \mathbb{Z} {}$
### Problem: Solve
$$
f(x)\equiv 0 \:(\mathrm{mod}\  p^{r+1}) \qquad \text{in} \qquad \mathbb{Z}_{p^{r+1}}
$$
### Strategy:
Solve ${} f(x)\equiv 0 \:(\mathrm{mod}\  p^{r})  {}$ in ${} \mathbb{Z}_{p^{r}} {}$.
- For each solution $x$ to the above, find all ${} [y]_{p^{r+1}} {}$ with the following:
	- ${} y\equiv x \:(\mathrm{mod}\  p^{r})  {}$
	- ${} f(y)\equiv 0 \:(\mathrm{mod}\  p^{r+1})  {}$

### Goal:
Find all ${} t \:(\mathrm{mod}\  p)  {}$ with ${} f(x_{r}+tp^{r})\equiv 0 \:(\mathrm{mod}\  p^{r+1})  {}$, recalling that ${} f(x_{r})\equiv 0\:(\mathrm{mod}\  p^{r})  {}$.
### Informal Discussion
Observe that since ${} p^{r} \mid tp^{r} {}$, we have that ${} x_{r}+tp^{r} {}$ and ${} x_{r}$ are "close" ${} \:(\mathrm{mod}\  p^{r+1})  {}$, that is, "divisibility by powers of $p$". 

Now we use an idea from calculus. If we have some small ${} |h|< \varepsilon {}$ and $g:\mathbb{R}\to{}\mathbb{R} {}$ is a "nice" function, then we can have a Taylor expansion:
$$
\begin{align}
 g(x+h) & =g(x)+g'(x)h+g''(x) \frac{h^{2}}{2!}+\dots    \\
 & =\sum_{j=0}^{\infty} \frac{g^{(j)}(x)}{j!} h^{j}
 \end{align}
$$
### Lemma 1.1:
Let ${} t \in \mathbb{Z} {}$, ${} r \in \mathbb{Z}^{+} {}$. Then for ${} x \in \mathbb{Z} {}$, 
$$
f(x+tp^{r})\equiv f(x)+f'(x)tp^{r} \:(\mathrm{mod}\  p^{r+1}) 
$$
#### Proof:
Write ${} n=\deg f {}$. Apply Taylor's theorem (or the binomial theorem suffices). We then get that for ${} x,\, h \in \mathbb{R} {}$, 
$$
f(x+h)=\sum_{j=0}^{n} \frac{f^{(j)}(x)}{j!}h^{j}
$$
Note that
$$
\frac{f^{(j)}(x)}{j!}
$$
is a polynomial with integer coefficients. 

In the above take ${} h=p^{r}t {}$ to get 
$$
\begin{align}
 f(x+tp^{r}) & =f(x)+f'(x)p^{r}t+\frac{f''(x)}{2} (p^{r}t)^{2}+\dots+\frac{f^{(n)}(x)}{n!}(p^{r}t)^{n}   \\
 & \equiv f(x)+f'(x)p^{r}t \:(\mathrm{mod}\  p^{r+1}) 
 \end{align}
$$
### When Hensel's Lemma does *not* apply
If ${} f(x_{r})\equiv 0 \:(\mathrm{mod}\  p^{r})  {}$ and ${} f'(x_{r})\equiv \:(\mathrm{mod}\  p)  {}$. Then, by lemma 1.1:
$$
f(x_{r}+tp^{r})\equiv f(x_{r})+\cancelto{ 0 }{ f'(x_{r})tp^{r}C } \:(\mathrm{mod}\  p^{r+1}) 
$$
and so ${} f(x_{r}+tp^{r})\equiv f(x_{r}) \:(\mathrm{mod}\  p^{r+1})  {}$. Then each of the following hold:
1. If ${} p^{r+1} \mid f(x_{r}) {}$, then ${} f(x_{r}+tp^{r})\equiv 0 \:(\mathrm{mod}\  p^{r+1})  {}$ for each ${} t \:(\mathrm{mod}\  p)  {}$
2. If ${} p^{r+1} \nmid f(x_{r}) {}$, then there no solutions to the equations to ${} f(x)\equiv 0 \:(\mathrm{mod}\  p^{r+1})  {}$ with ${} x=x_{r} \:(\mathrm{mod}\  p^{r})  {}$ and ${} f(x_{r})\equiv 0 \:(\mathrm{mod}\  p^{r})  {}$.
#### Example:
Solve ${} x^{3}+1\equiv 0 \:(\mathrm{mod}\  9)  {}$. Note that ${} p=3 {}$ and ${} r=2 {}$. First, we solve ${} \:(\mathrm{mod}\  3)  {}$. The only solution is ${} x\equiv -1 \:(\mathrm{mod}\  3)  {}$, by trial and error (<3). 

Now we check if ${} f'(-1)\equiv^{?} 0 \:(\mathrm{mod}\  3)  {}$. In fact, ${} f'(x)=3x^{2} {}$, so ${} f'(-1)=3\equiv 0 \:(\mathrm{mod}\  3)  {}$, so Hensel's lemma does not apply. Now we check if ${} 9 \mid  f(-1) {}$. In particular, ${} f(-1)=0\equiv 0 \:(\mathrm{mod}\  9)  {}$. Then each ${} x=-1+3t {}$ for ${} t=0,\, 1,\, 2 {}$. Therefore, ${} x\equiv -1,\, 2,\, 5 \:(\mathrm{mod}\  9)  {}$ are the solutions to ${} x^{3}+1\equiv 0 \:(\mathrm{mod}\  9)  {}$.
#### Proof of Hensel's Lemma
Let ${} x_{r} \in \mathbb{Z} {}$ with ${} f(x_{r})\equiv 0\:(\mathrm{mod}\  p^{r})  {}$, and ${} f'(x_{r})\not\equiv \:(\mathrm{mod}\  p)  {}$. Suppose that ${} x_{r+1}\equiv x_{r} \:(\mathrm{mod}\  p^{r})  {}$, that is, ${} x_{r+1}=x_{r}+t\cdot p^{r} {}$ for some ${} t =0,\,\dots,\,p-1 {}$. We want to find a unique ${} t\:(\mathrm{mod}\  p) {}$ with ${} f(x_{r}+tp^{r})\equiv 0 \:(\mathrm{mod}\  p^{r+1})  {}$. 

In particular, note that, by lemma 1.1
$$
f(x_{r}+tp^{r})\equiv f(x_{r})+f'(x_{r})tp^{r} \:(\mathrm{mod}\  p^{r+1}) 
$$
Since ${} p^{r} \mid  f(x_{r}) {}$, cancel a factor of ${} p^{r}$ like so:
$$
0\equiv \frac{f(x_{r})}{p^{r}}+tf'(x_{r}) \:(\mathrm{mod}\  p) 
$$
Let ${} [u]_{p}=[f'(x_{r})]^{-1}_{p} {}$ to get 
$$
t\equiv -\frac{f(x_{r})}{p^{r}}u \:(\mathrm{mod}\  p) 
$$
