---
tags:
  - jacobson_lie_algebra
  - exercises
date: 2024-05-17
---
[[Directory]], [[Jacobson Lie Algebras|Subject Directory]]
[[Lie algebras - Nathan Jacobson.pdf#page=42|Exercise Sheet]]
1. 
Let $\mathfrak{A}$ and $\mathfrak{B}$ be associative algebras. Let $\theta:\mathfrak{A}\to{}\mathfrak{B} {}$ be a homomorphism. Now given ${} x,\, y \in \mathfrak{A} {}$, we have that
$$
\theta([x,\, y])=\theta(xy-yx)=\theta(x)\theta(y)-\theta(y)\theta(x)=[\theta(x),\, \theta(y)]
$$
and so ${} \theta:\mathfrak{A}_{L}\to{}\mathfrak{B}_{L} {}$ is a Lie homomorphism.

Now let ${} \theta:\mathfrak{A}\to{}\mathfrak{B} {}$ is a antihomomorphism. We see that, given ${} x,\, y \in \mathfrak{A} {}$, we have
$$
-\theta([x,\, y])=-\theta(xy-yx)=-\theta(y)\theta(x)+\theta(x)\theta(y)=[\theta(x),\, \theta(y)]
$$

Now let ${} \theta:\mathfrak{A}\to{} \mathfrak{A} {}$ be an antihomomorphism. Let 
$$
\mathfrak{S}(\mathfrak{A},\, \theta) =\{ a \in \mathfrak{A} |\theta(a)=-a \}
$$
Now let ${} x,\, y \in \mathfrak{S}(\mathfrak{A},\, \theta) {}$. Now
$$
\begin{align}
 \theta([x,\, y]) & =\theta(xy-yx) \\
	 & =\theta(y)\theta(x)-\theta(x)\theta(y) \\
	 & =(-y)(-x)-(-x)(-y) \\
 & = yx-xy \\
 & =-(xy-yx) \\
 & =-[x,\, y]  
 \end{align}
$$
and so ${} [x,\, y] \in  \mathfrak{S} (\mathfrak{A},\, \theta) {}$. Furthermore, 
$$
\theta(x+y)=\theta(x)+\theta(y)=-x-y=-(x+y)
$$
and so ${} x+y \in  \mathfrak{S}(\mathfrak{A},\, \theta) {}$. Therefore, ${} \mathfrak{S}(\mathfrak{A},\, \theta) {}$ is a subalgebra of $\mathfrak{A}_{L}$.

Now let $D:\mathfrak{A}\to{}\mathfrak{A} {}$. Now given ${} x,\, y \in \mathfrak{A} {}$, we have
$$
\begin{align}
 D([x,\, y]) & =D(xy-yx) \\
 & =D(x)y+xD(y)-D(y)x-yD(x) \\
 & =(D(x)y-yD(x))+(xD(y)-D(y)x) \\
  & =[D(x),\, y]+[x,\, D(y)]
 \end{align}
$$
and so $D$ is a derivation of $\mathfrak{A}_{L}$ too. 
2. 
Let ${} S \subseteq  \mathfrak{L} {}$. Let
$$
\mathfrak{C}(S)=\{ c \in \mathfrak{L} \mid \forall s \in S:[s,\, c]=0 \}
$$
be the centraliser of ${} S {}$. Let ${} x,\, y \in \mathfrak{C}(S) {}$. Now if ${} s \in S {}$, then
$$
\begin{align}
 [[x,\, y],\, s] & =-([[s,\, x],\, y]+[[y,\, s],\, x])   \\
 & =-([0,\, y]+[0,\, x]) \\
 & =0
 \end{align}
$$
so ${} [x,\, y] \in \mathfrak{C}(S) {}$. Furthermore, we have
$$
[x+y,\, s]=[x,\, s]+[y,\, s]=0+0=0
$$
so ${} x+y \in \mathfrak{C}(S) {}$. Therefore, $\mathfrak{C}(S)$ is a subalgebra of $\mathfrak{L}$. 

Now let $\mathfrak{B}$ be a vector subspace of $\mathfrak{L}$, and set
$$
\mathfrak{N}(\mathfrak{B})=\{ l \in \mathfrak{L} \mid\forall  b \in \mathfrak{B}:[b,\, l]\in \mathfrak{B} \}
$$
be the normaliser of $\mathfrak{B}$. Now let ${} x,\, y \in \mathfrak{N}(\mathfrak{B}) {}$. If ${} b \in \mathfrak{B} {}$, we have
$$
\begin{align}
[[x,\, y],\, b]=[y,\, [b,\, x]]+ [x,\, [y,\, b]]
\end{align}
$$
since ${} x,\, y \in \mathfrak{N}(\mathfrak{B}) {}$, we have that 
$$
\begin{align}
c=[b,\, x] \in \mathfrak{B} \\
d=[y,\, b] \in \mathfrak{B}
\end{align}
$$
Therefore, ${} [y,\, c] \in \mathfrak{B} {}$ and ${} [x,\, d] \in \mathfrak{B} {}$, so since $\mathfrak{B} {}$ is a subspace, 
$$
[[x,\, y],\, b] \in \mathfrak{B}
$$
Furthermore, 
$$
\begin{align}
[x+y,\, b] & =[x,\, b]+[y,\, b]
\end{align}
$$
since ${} [x,\, b],\, [y,\, b] \in \mathfrak{B} {}$ and ${} \mathfrak{B} {}$ is a vector subspace, we see that
$$
[x+y,\, b] \in \mathfrak{B}
$$
Therefore, ${} [x,\, y] \in \mathfrak{N}(\mathfrak{B}) {}$ and ${} x+y \in \mathfrak{N}(\mathfrak{B}) {}$.
3. 
Let $\mathfrak{A}$ be a non-associative algebra, and let ${} D:\mathfrak{A}\to{}\mathfrak{A} {}$ be a derivation. Let
$$
\mathfrak{C}=\{ z \in \mathfrak{A}\mid D(z)=0 \}
$$
First, let ${} x,\, y \in \mathfrak{C} {}$. Now
$$
D(x+y)=D(x)+D(y)=0+0=0
$$
so ${} x+y \in \mathfrak{C} {}$. Furthermore, 
$$
\begin{align}
D(xy)=D(x)y+xD(y)=0y+x 0=0+0=0
\end{align}
$$
and so ${} xy \in \mathfrak{C} {}$, and ${} \mathfrak{C} {}$ is a subalgebra

Now let 
$$
\mathfrak{D}=\{ z \in \mathfrak{A} \mid\exists  i \in \mathbb{N}:D^{i}(z)=0 \}
$$
First, let ${} x,\, y \in \mathfrak{D} {}$. Therefore, we have some ${} i,\, j \in \mathbb{N} {}$ with ${} D^{i}(x)=0 {}$ and ${} D^{j}(y)=0 {}$. Now if ${} k=\max(i,\, j) {}$
$$
D^{k}(x+y)=D^{k}(x)+D^{k}(y)=0+0=0
$$
and
$$
\begin{align}
 D^{i+j}(xy) & =\sum_{n=0}^{i+j} \binom{i+j}{n} D^{n}(x)D^{i+j-n}(y)  \\
 & = \sum_{n=0}^{i} \binom{i+j}{n} D^{n}(x)D^{i+j-n}(y)+\sum_{m=i+1}^{i+j} \binom{i+j}{m} D^{m}(x)D^{i+j-m}(y) 
 \end{align}
$$
and so since ${} 0\leq n\leq i {}$, ${} i+j-n\geq j {}$, and ${} D^{i+j-n}(y)=0 {}$, and since ${} i+1\leq m\leq i+j {}$, then $m\geq i$, and ${} D^{m}(x)=0 {}$. Therefore, 
$$
D^{i+j}(xy)=0
$$
and so ${} x+y,\, xy \in \mathfrak{D} {}$, and $\mathfrak{D}$ is a subalgebra.
4. 
Let ${} D:\mathfrak{L}\to{}\mathfrak{L} {}$ be a derivation in $\mathfrak{L}$ such that for all ${} x \in \mathfrak{L} {}$, 
$$
D(\ad x)=(\ad x) D
$$
is the inner derivation associated with ${} x$. Let ${} x \in \mathfrak{L} {}$. Now if ${} y \in \mathfrak{L} {}$, then
$$
\begin{align}
 [x, Dy]  & =(\ad x)(D(y)) \\
	 & =D((\ad x)(y)) \\
 & =D[x,\,  y]  \\
 & =[Dx,\,  y]+[x,\,  Dy] \\ 
\Rightarrow [Dx,\, y] & =0
 \end{align}
$$
Therefore, ${} Dx \in \mathfrak{C}(\mathfrak{L}) {}$, and so ${} \im D \subseteq \mathfrak{C}(\mathfrak{L}) {}$. 
5. 
Let $\mathfrak{L}$ be a three dimensional simple lie algebra over a field of characteristic which is not 2. Then there exists a basis ${} \{ e,\, f,\, h \} {}$ such that
$$
[e,\, h]=2e,\, \qquad [f,\, h]=-2f,\, \qquad [e,\, f]=h
$$
Now let ${} D$ be a derivation in $\mathfrak{L} {}$. Set
$$
\begin{align}
 De & = ae+bf+ch  \\
Df & =xe+yf+zh
 \end{align}
$$
Now see that
$$
\begin{align}
 Dh  =D[e,\, f] & =[De,\, f]+[e,\, Df]  \\
 & = [ae+bf+ch,\, f]+[e,\, xe+yf+zh] \\
 & =ah+2cf+yh+2ze \\
 & =2ze+2cf+(a+y)h
 \end{align}
$$
Now note that
$$
\begin{align}
 De & =\frac{1}{2}D[e,\, h] \\
	 & =\frac{1}{2}\left( [De,\, h]+ [e,\, Dh]\right) \\
 & =\frac{1}{2}([ae+b f+ch,\, h]+[e,\, 2ze+2cf+(a+y)h]) \\
 & =\frac{1}{2} (2ae-2b f+2ch+2(a+y)e) \\
ae+b f+ch & =(2a+y)e-bf+c h
 \end{align}
$$
Now we have ${} a=2a+y {}$, so ${} a=-y {}$, and ${} -b=b {}$, so ${} 2b=0 {}$, and since ${} \Char  \Phi\neq 0 {}$, then ${} b=0 {}$. Finally, $c$ is free. We may do a similar operation with $Df {}$, and find that again ${} x=0 {}$, ${} y=-a {}$, and $z$ is free. Now we have
$$
\begin{align}
 De  & =ae+ch \\
Df & =-af+zh \\
Dh & =2ze+2cf 
 \end{align}
$$
If we set ${} v=ze-cf-\frac{1}{2}ah {}$, we see that
$$
\begin{align}
 [v,\, e] & =ae+ch   \\
 [v,\, f] & =-af+zh \\
[v,\, h] & =2ze+2cf
 \end{align}
$$
and so $$
D=\ad v
$$
and every derivation is inner. Also, the centre is trivially $0$, as the centre is an ideal, and $\mathfrak{L}$ is non-abelian and simple. Therefore, $\mathfrak{L}$ is complete.
6. 
Let $\mathfrak{L}$ be a 4-dimensional nilpotent Lie algebra. Let $k\leq 4$ be the nilpotence degree of $\mathfrak{L}$.
7. skip
8. 
Let $\mathfrak{L} {}$ be a lie algebra. We proceed by induction. First note that if ${} \mathfrak{B} {}$ is subinvariant of degree ${} 1$, then ${} \mathfrak{B} \subseteq  \mathfrak{L} {}$ is an ideal, and ${} [\mathfrak{L},\, \mathfrak{B}] \subseteq \mathfrak{B} {}$ by definition. Now 