---
tags:
  - exercises
  - dnf_algebra
date: 2023-10-19
---
[[Directory]], [[D&F Abstract Algebra|Subject Directory]], 
[[1. Introduction to Groups#Exercises 1.1|Relevant Notes]]
[[Abstract Algebra - David S. Dummit, Richard M. Foote.pdf#page=35|Exercises in Textbook]]
1. 
a) ${} -$ on $\mathbb{Z}$ is not associative, as ${} (1-1)-1=-1\neq 1=1-(1-1)= {}$
b) $*$ on $\mathbb{R}$, with $a*b=a+b+ab {}$ is associative, as
$$
\begin{align}
a*(b*c) & =a*(b+c+bc) \\
 & =a+b+c+ab+ac+bc+abc \\
 & =(a+b+ab)*c \\
 & =(a*b)*c
\end{align}
$$
c) $*$ is associative, as $+$ is associative
d) Let $(a_{1},\, a_{2}),\, (b_{1},\, b_{2}),\, (c_{1},\, c_{2})\in \mathbb{Z}\times \mathbb{Z}$. Now we have
$$
\begin{align}
((a_{1},\, a_{2})*(b_{1},\, b_{2}))*(c_{1},\, c_{2}) & =(a_{1}b_{2}+a_{2}b_{1},\, a_{2}b_{2})*(c_{1},\, c_{2}) \\
 & =(a_{1}b_{2}c_{2}+a_{2}b_{1}c_{2}+a_{2}b_{2}c_{1},\, a_{2}b_{2}c_{2}) \\
 & =(a_{1},\, a_{2})*(b_{1}c_{2}+b_{2}c_{1},\, b_{2}c_{2}) \\
 & =(a_{1},\, a_{2})*((b_{1},\, b_{2})*(c_{1},\, c_{2}))
\end{align}
$$
Therefore, $*$ is associative
e) $*$ is not associative. Consider 
$$
\begin{align}
\frac{2}{\left( \frac{1}{3} \right)}=6\neq \frac{2}{3}=\frac{\left( \frac{2}{1} \right)}{3}
\end{align}
$$
2. We give these with minimal proofs
a) No. ${} 3-5\neq 5-3$
b) yes, as $+$ and $\cdot$ are commutative
c) yes, as ${} + {}$ is associative
d) yes, as ${} +$ and $\cdot {}$ are commutative
e) no. ${} 3 / 5\neq 5/3 {}$

3. Let ${} \conj{a},\, \conj{b},\, \conj{c}\in \mathbb{Z}/n\mathbb{Z} {}$. Now we have
$$
\begin{align}
\conj{a}+(\conj{b}+\conj{c}) & =\conj{a}+\conj{b+c} \\
	 & =\conj{a+b+c} \\
 & =\conj{a+b}+\conj{c} \\
 & =(\conj{a}+\conj{b})+\conj{c}
\end{align}
$$
Therefore, addition is associative over ${} \mathbb{Z} /n\mathbb{Z} {}$
4. Let ${} \conj{a},\, \conj{b},\, \conj{c}\in \mathbb{Z} /n\mathbb{Z} {}$. Now we have
$$
\begin{align}
 \conj{a}(\conj{b} \conj{c})  & =\conj{a}\; \conj{bc} \\
 & =\conj{abc} \\
	 & =\conj{ab}\;\conj{c} \\
	 & =(\conj{a}\conj{b})\conj{c} 
 \end{align}
$$
Therefore, multiplication over ${} \mathbb{Z}/n\mathbb{Z} {}$ is associative

5. The element ${} \conj{0}\in \mathbb{Z} /n\mathbb{Z}$ does not have an inverse. Note that $\conj{0}\cdot \conj{a}=\conj{0a}=\conj{0}\neq \conj{1}$, unless of course ${} n=1 {}$. Therefore, ${} \mathbb{Z} /n\mathbb{Z} {}$ is not a group over multiplication

6. skip

7. Let $G=\{ x \in \mathbb{R}\mid 0\leq x<1 \}$, and $a*b=a+b-\floor*{a+b} {}$. This is well defined, because ${} {}\floor*{x} {}$ is well defined, and it is a binary operation on $G {}$ by the definition of floor. Now let ${} a,\, b,\, c \in G$. We show that $* {}$ is associative. 
$$
\begin{align}
a*(b*c) & =a*(b+c-\floor*{b+c} ) \\
 &=a+b+c-\floor*{b+c} -\floor*{a+b+c-\floor*{b+c} } 
\end{align}
$$
Since ${} \floor*{b+c}  {}$ is an integer, then we may move it outside of the outer floor. Therefore, we have
$$
\begin{align}
a*(b*c) & =a+b+c-\floor*{b+c} -\floor*{a+b+c-\floor*{b+c} }  \\
 & =a+b+c-\floor*{a+b+c}  \\
 &= a+b+c-\floor*{a+b} -\floor*{a+b+c-\floor*{a+b} }  \\
 & =(a+b-\floor*{a+b} )*c \\
 & =(a*b)*c
\end{align}
$$
Therefore, $* {}$ is associative. We now show the existence of an identity. ${} 0 \in G {}$. Observe that
$$
a*0=0*a=a+0-\floor*{a+0}=a-\floor*{a} =a 
$$
${} \floor*{a} =0 {}$, as $0\leq a<1$. Now given ${} x \in G {}$, we show the existence of an inverse. Observe that
$$
x*(1-x)=x+1-x-\floor*{x+1-x}=1-\floor*{1}=0  
$$
and
$$
(1-x)*x=1-x+x-\floor*{1-x+x} =1-\floor*{1} =0
$$
Therefore, ${} 1-x {}$ is the inverse of $x$, so for all ${} x \in  G {}$, there exists an inverse. Finally, we show that $G$ is commutative. Let ${} a,\, b \in  G {}$. 
$$
a*b=a+b-\floor*{a+b} =b+a-\floor*{b+a}=b*a
$$
Therefore, ${} (G, *) {}$ is a abelian group.

8. skip
9. 
a) Let $x=a_{1}+b_{1}\sqrt{2}\in G {}$ , ${} y=a_{2}+b_{2}\sqrt{2}\in G {}$ , $z=a_{3}+b_{3}\sqrt{2}\in G {}$. First we show associativity
$$
\begin{align}
 x+(y+z) & =x+  \left( a_{2}+b_{2}\sqrt{2}+a_{3}+b_{3}\sqrt{2} \right) \\
 & =a_{1}+a_{2}+a_{3}+(b_{1}+b_{2}+b_{3})\sqrt{2} \\
 & =\left( a_{1}+b_{1}\sqrt{2}+a_{2}+b_{2}\sqrt{2} \right)+z \\
 & =(x+y)+z
 \end{align}
$$
Now note that ${} 0=0+0\sqrt{2}\in G {}$, and ${} 0+x=x+0=x$. Also note that ${} -x=-a_{1}-b_{1}\sqrt{2}\in G, {}$ and ${} x+(-x)=a_{1}-a_{2}+(b_{1}-b_{2})\sqrt{2}=0$. Therefore, $G$ is a group under addition

b) Let ${} x=a_{1}+b_{1}\sqrt{2},\, y=a_{2}+b_{2}\sqrt{2}\ ,\, z=a_{3}+b_{3}\sqrt{2}\in G\setminus \{ 0 \} {}$. First we show associativity. Since ${} x,\, y,\, z {}$ are just real numbers, then we have associativity of multiplication from the real numbers. Likewise, note that ${} 1=1+0\sqrt{2}\in G {}$, and ${} 1x=x1=x {}$. Lastly, given ${} x=a+b\sqrt{2}\in G {}$, we have
$$
\begin{align}
\left( a+b\sqrt{2} \right)\left( \frac{a}{a^{2}-2b^{2}}-\frac{ b }{ a^{2}-2b^{2} }\sqrt{2} \right) & =\frac{\left( a+b\sqrt{2} \right)\left( a-b\sqrt{2} \right)}{a^{2}-2b^{2}} \\
 & =\frac{a^{2}-2b^{2}}{a^{2}-2b^{2}} \\
 & =1
\end{align}
$$
Since ${} a/(a^{2}-2b^{2})\in \mathbb{Q} {}$ and ${} b /(a^{2}-2b^{2})\in \mathbb{Q} {}$, then we have $\displaystyle{}  \frac{a}{a^{2}-2b^{2}}-\frac{ b }{ a^{2}-2b^{2} }\sqrt{2}\in G$, and so $x$ has an inverse

10. skip
11. We list the elements of ${} \mathbb{Z} /12\mathbb{Z} {}$ without their overbar for convenience. 
- ${} |0|=1 {}$
- ${} |1|=12$
- ${} |2|=6 {}$
- ${} |3|=4$
- $|4|=6$
- ${} |5|=12 {}$
- ${} |6|=2 {}$
- $|7|=12$
- ${} |8|=6$
- ${} |9|=4 {}$
- ${} |10|=6$
- ${} |11|=12 {}$

12. Same as above
- ${} |1|=1$
- $|-1|=2$
- ${} |5|=2 {}$
- $|7|=2$
- $|-7|=2$
- ${} |13|=1 {}$

13. Same as above
- ${} |1|=36 {}$
- ${} |2|=18 {}$
- $|6|=6$
- ${} |9|=12 {}$
- ${} |10|=18 {}$
- ${} |12|=3 {}$
- ${} |-1|=36 {}$
- ${} |-10|=18 {}$
- ${} |-18|=2 {}$

14. Same as above
- ${} |1|=1 {}$
- ${} |-1|=2 {}$
- $|5|=6$
- ${} |13|=3 {}$
- ${} |-13|=6 {}$
- ${} |17|=2 {}$

15. We work by induction. First note that $( a_{1} )^{-1}=a_{1}^{-1}$, and ${} (a_{1}a_{2})^{-1}=a_{2}^{-1}a_{1}^{-1} {}$
Now suppose that we have ${} (a_{1}a_{2}\dots a_{n-1})^{-1}=a_{n-1}^{-1}a_{n-2}^{-1}\dots a_{1}^{-1}$. Observe that 
$$
\begin{align}
(a_{1}a_{2}\dots a_{n})^{-1} & =a_{n}^{-1}(a_{1}a_{2}\dots a_{n-1})^{-1} \\
 & =a_{n}^{-1}a_{n-1}^{-1}\dots a_{1}^{-1}
\end{align}
$$
Therefore, by the induction principle, we have that for all ${} n \in  \mathbb{N} {}$, 
$$
(a_{1}a_{2}\dots a_{n})^{-1}=a_{n}^{-1}a_{n-1}^{-1}\dots a_{1}^{-1}
$$

16. skip
17. If ${} |x|=n {}$, then we have $x^{n}=1$. Multiplying by $x^{-1} {}$ on the right (or left), we get ${} x^{n-1}=x^{-1} {}$ as required
18. skip

19. let ${} x \in  G {}$ and ${} a,\, b \in  \mathbb{Z}_{+}$.
a) ${} x^{a+b}=\underbrace{ xx\dots x }_{ a+b \text{ times} }=\underbrace{ x\dots x }_{ a \text{ times} }\underbrace{ x\dots x }_{ b \text{ times} }=x^{a}x^{b} {}$
${} ( x^{a} )^{b}=\underbrace{ x^{a}x^{a}\dots x^{a} }_{ b \text{ times} }=x^{\underbrace{ a+a+\dots+a }_{ b \text{ times} }}=x^{ab}$
b) Note that ${} x^{a}x^{-a}=\underbrace{ x x\dots x }_{ a \text{ times} }\underbrace{ x^{-1}x^{-1}\dots x^{-1} }_{ a\text{ times} }=\underbrace{ x x\dots x }_{ a-1 \text{ times} }\underbrace{ x^{-1}x^{-1}\dots x^{-1} }_{ a-1\text{ times} }=\dots=xx^{-1}=1 {}$. Therefore, ${} ( x^{a} )^{-1}=x^{-a} {}$

c) let ${} a,\, b\in \mathbb{Z} {}$. We now have several cases:
If ${} a=b=0$, then we have
${} x^{a}x^{b}=1\cdot 1=x^{0+0}=x^{a+b} {}$
if ${} a=0 {}$, then we have
$$
x^{a}x^{b}=1x^{b}=x^{b}=x^{0+b}=x^{a+b}
$$
if ${} b=0 {}$, then we have
$$
x^{a}x^{b}=x^{a}1=x^{a}=x^{a+0}=x^{a+b}
$$
If ${} a,\, b>0 {}$, then we have
${} x^{a}x^{b}=x^{a+b}  {}$ as proved above

If ${} a>0$, $b<0$, then ${} -b>0 {}$, so we have
$$
x^{a}x^{b}=x^{a}(x^{-b})^{-1}=x^{a-(-b)}=x^{a+b}
$$
If $a<0$, $b>0$, then ${} -a>0 {}$, so we have
$$
x^{a}x^{b}=( x^{-a} )^{-1}x^{b}=x^{b-(-a)}=x^{a+b}
$$
If ${} a,\, b<0$, then $-a>0$, ${} -b>0 {}$, so we have
$$
x^{a}x^{b}=( x^{-a} )^{-1}(x^{-b})^{-1}=( x^{-b}x^{-a} )^{-1}=(x^{-(a+b)})^{-1}=x^{a+b}
$$
Therefore, for all ${} a,\,  b\in  \mathbb{Z} {}$, we have
$$
x^{a}x^{b}=x^{a+b}
$$
20. Let $x \in  G$, and ${} |x|=n {}$. Then we have ${} x^{n}=1 {}$, and ${} x^{n}x^{-n}=x^{0}=1 {}$, so ${} 1 x^{-n}=1=( x^{-1} )^{n}$. Therefore, $x^{-1} {}$ has at least the order of ${} x$. Now note that ${} (x^{-1})^{-1}=x {}$, so we have that ${} ( x^{-1} )^{-1}=x {}$ has at least the order of ${} x$. Therefore, ${} |x|=|x^{-1}| {}$ 

21. Because ${} G {}$ is finite, we have that ${} x^{n}=1 {}$, so $x^{n+1}=x$. $n$ is odd, so $n+1$ is even, therefore, there exists a number $k$ such that $n+1=2k$. Therefore, we have ${} x=x^{n+1}=x^{2k}=(x^{2})^{k} {}$

22. Let ${} x,\, g \in  G {}$. Let ${} n=|x| {}$, with finite order. We have
$$
\begin{align}
 (g^{-1}xg)^{n} & =\underbrace{ g^{-1}xg g^{-1}xg\dots g^{-1}xg }_{ n\text{ times} }   \\
 & =g^{-1} \underbrace{ x x\dots x }_{ n \text{ times} }\, g \\
 & =g^{-1}x^{n}g \\
 & =g^{-1} g \\
 & =1
 \end{align}
$$
Therefore, the order of ${} g^{-1}xg {}$ is at most ${} n$. Now suppose that ${} |g^{-1}xg|<n$. Let ${} k=|g^{-1}xg| {}$. Now we have
$$
\begin{align}
1 & =(g^{-1}xg)^{k} \\
 & =g^{-1}x^{k}g
\end{align}
$$
By above argument. So we have
$$
\begin{align}
g^{-1}x^{k}g & =1 \\
x^{k}g & =g \\
 x^{k}& =1
\end{align}
$$
But since $k<n {}$, then ${} x^{k}\neq 1$. Therefore, ${} |x|=|g^{-1}xg| {}$. 
We also have the case when the order of $x {}$ is infinite. Suppose for some ${} n {}$, we have that
$$
g^{-1}x^{n}g=1
$$
Then we would have
$$
x^{n}g=g
$$
and 
$$
x^{n}=1
$$
But this is impossible as $x {}$ has infinite order. Therefore, ${} g^{-1}xg {}$ also has infinite order

Now let ${} a,\, b\in G {}$. Let $|ab|=n {}$ have finite order. Now we have
$$
\begin{align}
( ba )^{n} & =\underbrace{ baba\dots baba }_{ n \text{ times} } \\
 & =b(\underbrace{ abab\dots abab }_{ n-1 \text{ times} })a \\
 & =b(( ab )^{-1})a \\
 & =b(b^{-1}a^{-1})a \\
 & =1
\end{align}
$$
So ${} |ba|\leq |ab| {}$. However, note that this is symmetric, and by the same argument, we can set ${} b=a {}$ and ${} a=b$, and get that ${} |ab|\leq|ba| {}$. Therefore, ${} |ab|=|ba| {}$
We also have the case that $ab {}$ has infinite order. Suppose that for some $n$, we have
$$
(ba)^{n}=1
$$
Then we would have
$$
\begin{align}
b(ab)^{n-1}a & =1 \\
( ab )^{n-1} & =(ab)^{-1} \\
(ab)^{n} & =1
\end{align}
$$
Which is impossible, as $ab {}$ has infinite order. Therefore, $ba {}$ also has infinite order, so ${} |ab|=|ba| {}$

23. Let ${} x \in  G$ have finite order. Let ${} |x|=n {}$, and suppose that ${} n=st {}$. Then
$$
\begin{align}
x^{n} & =1 \\
x^{st} & =1 \\
( x^{s} )^{t} & =1 \\
\end{align}
$$
So the order of ${} x^{s} {}$ is at most $t$. Now suppose that ${} |x^{s}|=k\leq t {}$. Then we have
$$
\begin{align}
( x^{s} )^{k} & =1 \\
x^{sk} & =1
\end{align}
$$
Since $k\leq t$, the $sk\leq n {}$. But $n$ is the smallest $n$ such that $x^{n}$. Therefore, ${} sk=n=st$. Therefore, ${} k=t$. Therefore, ${} |x^{s}|=t {}$, as required

24. skip

25. Suppose that for all $x \in G$, we have ${} x^{2}=1 {}$. Take ${} x,\, y\in G {}$. We have
$$
\begin{align}
xyxy=1
\end{align}
$$
So $(xy)^{-1}=xy {}$, and ${} (xy)^{-1}=y^{-1}x^{-1}=yx {}$, so ${} xy=yx {}$. Therefore, $G$ is abelian

26. Let ${} H\subseteq G {}$ such that ${} a,\, b\in H {}$ implies ${} ab\in H {}$, and ${} a^{-1}\in H {}$. We first prove associativity: 
- Let ${} a,\, b,\, c \in  H {}$. Therefore, ${} a,\, b,\, c\in G$. Therefore, ${} a(bc)=(ab)c$. But ${} a(bc)\in H {}$ as it is closed, so for all ${} a,\, b,\, c\in H {}$, then ${} a(bc)=(ab)c {}$. Therefore, $*$ is associative over $H$.
- Next, identity. Given an element $x \in H$, we have ${} x^{-1}\in H {}$, as well, by hypothesis. Therefore, we also have $xx^{-1}=x^{-1}x=1\in H$, so ${} 1 \in  H {}$. 
- Note that if ${} x \in H {}$, then ${} x^{-1}\in H {}$, by hypothesis

Therefore, we have associativity, identity, and inverses in $H$. Therefore, $H$ is a group over $*$

27. skip 
28. Given ${} (A, \otimes ) {}$, ${} (B, \oplus )$ are groups. Then we have $A\times B {}$ as their direct product. 
a)  We prove associativity. Let ${} (a_{1}, a_{2}),\, (b_{1},\, b_{2}),\, (c_{1},\, c_{2})\in A\times B {}$. Then we have
$$
\begin{align}
(a_{1},\, a_{2})((b_{1},\, b_{2})(c_{1},\, c_{2})) & =(a_{1},\, a_{2})(b_{1}c_{1},\, b_{2}c_{2}) \\
 & =(a_{1}b_{1}c_{1},\, a_{2}b_{2}c2) \\
 & =(a_{1}b_{1},\, a_{2}b_{2})(c_{1},\, c_{2}) \\
 & =((a_{1},\, a_{2})(b_{1},\, b_{2}))(c_{1},\, c_{2})
\end{align}
$$
Therefore, multiplication is associative

b) Let ${} (a,\, b) \in A\times B {}$. Then we have
$$
\begin{align}
(a,\, b)(1,\, 1) & =(a1,\, b1)=(a,\, b)
\end{align}
$$
and 
$$
(1,\, 1)(a,\, b)=(1a,\, 1b)=(a,\, b)
$$
Therefore, ${} (1,\, 1)$ is an identity

c) Let ${} (a,\, b)\in A\times B$. Then we have
$$
(a^{-1},\, b^{-1})(a,\, b)=(a^{-1}a,\, b^{-1}b)=(1,\, 1)
$$
and 
$$
(a,\, b)(a^{-1},\, b^{-1})=(aa^{-1},\, b b^{-1})=(1,\, 1)
$$
Therefore, ${} (a,\, b)^{-1}=(a^{-1},\, b^{-1})$.
29. Skip
30.  Let ${} a \in A {}$ and ${} b \in B {}$. Observe that
$$
(a,\, 1)(1,\, b)=(a,\, b)=(1,\, b)(a,\, 1)
$$
Let ${} n=|a| {}$, and ${} m=|b| {}$. Observe that, for some ${} k\geq 1 {}$, 
$$
(a,\, b)^{k}=(a^{k},\, b^{k})
$$
For ${} (a,\, b)^{k}=(1,\, 1) {}$, then we must have ${} a^{k}=1 {}$ and ${} b^{k}=1 {}$. Therefore, 