---
tags:
  - dnf_algebra
  - exercises
date: 2023-11-10
---
[[Directory]], [[D&F Abstract Algebra|Subject Directory]]
[[Abstract Algebra - David S. Dummit, Richard M. Foote.pdf#page=46|Exercise Sheet]]
1. 
$\sigma=(1\;3\;5)(2\;4)$
${} \tau=(1\;5)(2\;3) {}$
${} \sigma^{2}=(1\; 3\; 5)(2\; 4)(1\; 3\; 5)(2\; 4)=(1\; 3\; 5)(1\; 3\; 5)(2\; 4)(2\;4)=(1\;5\;3) {}$
${} \sigma \tau=(1\;3\;5)(2\;4)(1\;5)(2\;3)=(2\;5\;3\;4) {}$
${} \tau \sigma=(1\;5)(2\;3)(1\;3\;5)(2\;4)=(1\;2\;4\;3) {}$
${} \tau^{2}\sigma=(1\;5)(2\;3)(1\;2\;4\;3)=(1\;3\;5)(2\;4) {}$, so $\tau^{2}=()$
2. skip
3. double skip
4. 
a) ${} S_{3}:|S_{3}|=6 {}$
${} |()|=1 {}$
${} |(1\;2)|=2 {}$
${} |(2\;3)|=2$
${} |(1\;3)|=2 {}$
${} |(1\;2\;3)|=3 {}$
$|(1\;3\;2)|=3$
b) ${} S_{4}:|S_{4}|=24 {}$
${} |()|=1 {}$
${} |(1\;2)|=2 {}$
${} |(1\;3)|=2 {}$
${} |(1\;4)|=2 {}$
${} |(2\;3)|=2 {}$
${} |(2\;4)|=2 {}$
$|(3\;4)|=2$
$|(1\;2)(3\;4)|=2$
$|(1\;3)(2\;4)|=2 {}$
$|(1\;4)(2\;3)|=2$
${} |(1\;2\;3)|=3 {}$
$|(1\;3\;2)|=3$
${} |(1\;2\;4)|=3 {}$
${} |(1\;4\;2)|=3 {}$
${} |(1\;3\;4)|=3 {}$
$|(1\;4\;3)|=3$
${} |(2\;3\;4)|=3 {}$
${} |(2\;4\;3)|=3 {}$
${} |(1\;2\;3\;4)|=4 {}$
$|(1\;2\;4\;3)|=4$
$|(1\;3\;2\;4)|=4 {}$
${} |(1\;3\;4\;2)|=4 {}$
${} |(1\;4\;2\;3)|=4 {}$
$|(1\;4\;3\;2)|=4$

5. $$
|(1\;12\;8\;10\;4)(2\;13)(5\;11\;7)(6\;9)|=\lcm(5,\, 2,\, 3,\, 2)=5\times 2\times 3=30
$$
6. skip
7. skip
8. skip
9. skip due to q11
10. 
Let ${} \sigma=(a_{1}\;a_{2}\;\dots\;a_{m})$, and let ${} f:\mathbb{N}\to{}\{ 1,\,\dots,\,m \} {}$ such that ${} f(n) {}$ is the smallest positive integer $k$ such that $k\equiv n\:(\mathrm{mod}\  m)$. Now we work by induction. Note that, given ${} k \in  \{ 1,\,\dots,\,m \} {}$, if ${} k\neq m {}$, then ${} f(k+1)=k+1 {}$, so ${} \sigma(a_{k})=a_{k+1}=a_{f(k+1)}$. However, if ${} k=m$, then ${} f(k+1)=1 {}$, and $\sigma(a_{k})=a_{0}=a_{f(k+1) }$. Therefore, ${} \sigma(a_{k})=a_{f(k+1) }$. Now suppose that ${} \sigma^{i}(a_{k})=a_{f(k+i)}$ for all ${} k \in  \{ 1,\,\dots,\,m \}$. Now we have 
$$
\begin{align}
\sigma^{i+1}(a_{k}) & =\sigma(\sigma^{i}(a_{k})) \\
 & =\sigma(a_{f(k+i)}) \\
 & =a_{f(f(k+i)+1)}
\end{align}
$$
We must have ${} f(k+i)=k+i-am {}$ for some ${} a \in \mathbb{N} {}$, by definition. Therefore, we have ${} f(f(k+i)+1)=f(k+i+1-am)=f(k+i+1)$, by the properties of modulo classes.
Now we have
$$
\sigma^{i+1}(a_{k})=a_{f(k+i+1)}
$$
So by induction, for all ${} i \in \mathbb{N} {}$, we have ${} \sigma^{i}(a_{k})=a_{f(k+i)} {}$ as required
11. 
Let ${} \sigma=(1\;2\;\dots\;m) {}$. We deduced above that, given ${} i,\, k \in  \mathbb{N} {}$, then ${} \sigma^{i}(a_{k})=a_{f(k+i)} {}$. In order for $\tau {}$ to be a ${} k$ cycle, we must have ${} \tau^{j}(a_{k})=a_{k}\Rightarrow m\mid j {}$. Therefore, if we set ${} \tau=\sigma^{i} {}$ with ${} i \in  \{ 1,\,\dots,\,m \} {}$, we see that we must have ${} \sigma^{ij}(a_{k})=a_{k}\Rightarrow m\mid j {}$. We have ${} \sigma^{ij}(a_{k})=a_{f(k+ij)}=a_{k} {}$, so we must have ${} f(k+ij)=f(k)$. Therefore, ${} m\mid ij$. If $i$ is relatively prime to $m {}$, then it follows immediately that $m\mid j {}$, so ${} \sigma^{i} {}$ must be a $m$-cycle. Otherwise, we may have $j=m /\gcd(i,\, m)$, so $m\nmid j {}$, but we still have ${} m \mid ij$, but this does not imply that ${} m \mid j {}$ ${} \sigma^{i}$ is not a $k$-cycle, as required
12. 
a) We have $$
(1\;3\;5\;7\;9\;2\;4\;6\;8\;10)^{5}=(1\;2)(3\;4)(5\;6)(7\;8)(9\;10)
$$
b) ${} |(1\;2)(3\;4\;5)|=6$, so $|\sigma|=6k {}$. We see that an element of a $k$-cycle is fixed by a 