---
tags:
  - dnf_algebra
  - exercises
date: 2023-11-20
---
[[Directory]], [[D&F Abstract Algebra]]
[[Abstract Algebra - David S. Dummit, Richard M. Foote.pdf#page=58|Exercise Sheet]]
1. skip
2. skip
3. skip
4. a)
Let ${} G {}$ be a group acting on a set $A$. Let ${} a \in A {}$. The kernel of the action is 
$$
K=\{ g \in G\mid \forall b \in A:gb=b  \}
$$
It is clear that this is both associative and a subset of $G {}$. Next, if ${} g,\, h \in K$, then ${} (gh)a=g(ha)=ga=a {}$, so $gh \in K {}$. Now by definition, $1 \in K$. Finally, if ${} g \in K {}$, then ${} ga=a$. Therefore, ${} a=1a=(gg^{-1})a=g(g^{-1}a) {}$. Since ${} g {}$ acts bijectively, then if ${} g(g^{-1}a)=a {}$, then ${} g^{-1}a=a {}$. Therefore, ${} g^{-1} \in K {}$, and $K\leq G {}$.

b) 
The stabiliser of this action w.r.t ${} a {}$ is
$$
S=\{ g \in G\mid ga=a \}
$$
It is clear that this is both associative and a subset of ${} G$. Next, if ${} g,\, h \in S {}$, then ${} (gh)a=g(ha)=ga=a {}$, so ${} gh \in S {}$. Now, by definition, ${} 1a=a {}$, so ${} 1 \in S {}$. Finally, if ${} g \in S {}$, then ${} ga=a {}$. Therefore, ${} a=1a=(g g^{-1})a=g(g^{-1}a) {}$. Since $g$ acts bijectively, then if ${} g(g^{-1}a)=a {}$, then ${} g^{-1}a=a {}$. Therefore, ${} g^{-1} \in S {}$ and $S\leq G {}$
5. skip
6. skip
7. skip
8. 
a)
Let ${} \sigma \in S_{A} {}$. Then, $\sigma: A\to{}A$ is a bijection. Therefore, there exists some $\sigma^{-1}$ such that ${} \sigma ^{-1}\circ \sigma=\sigma \circ \sigma ^{-1}=1 {}$