---
tags:
  - dnf_algebra
  - exercises
date: 2023-11-22
---
[[Directory]], [[D&F Abstract Algebra|Subject Directory]]
[[Abstract Algebra - David S. Dummit, Richard M. Foote.pdf#page=66|Exercise Sheet]]
1. skip
2. 
Informally, the centralizer is the set of elements that commute with the subset; if the subset is the centre, then all elements commute with it. 

Formally, we have
$$
C_{G}(Z(G))=\{ g \in G\mid \forall a \in Z(G):gag^{-1}=a \}
$$
Since ${} a \in Z(G)$, then ${} gag^{-1}=g g^{-1}a=a {}$. Therefore, 
$$
C_{G}(Z(G))=\{ g \in G\mid\forall a \in Z(G):a=a \}=G
$$
Since ${} G\supseteq Z_{G}(Z(A))\supseteq C_{G}(Z(A)) {}$, then $Z_{G}(Z(G))=G$.
3. 
Let $A,\, B \subseteq G$ with ${} A \subseteq B {}$. Let $x \in  C_{G}(B) {}$. Then, ${} \forall a \in B:xax^{-1}=a {}$. Since ${} A\subseteq B$, then ${} \forall a \in A:xax^{-1}=a {}$. Therefore, $x \in C_{G}(A)$, so ${} C_{G}(B)\subseteq C_{G}(A) {}$. Since all the group axioms definitely hold in ${} C_{G}(B) {}$, then $C_{G}(B)\leq C_{G}(A)$.
4. 
$S_{3}$:
$C_{S_{3}}(1)=S_{3}$
${} C_{S_{3}}((1\;2))=\{ 1,\, (1\;2)\} {}$
${} C_{S_{3}}((2\;3))=\{ 1,\,  (2\;3) \} {}$
${} C_{S_{3}}((1\;3))=\{ 1,\,  (1\;3) \} {}$
${} C_{S_{3}}((1\;2\;3))=\{ 1,\,  (1\;2\;3),\,  (1\;3\;2) \} {}$
${} C_{S_{3}}((1\;3\;2))=\{ 1,\, (1\;3\;2),\, (1\;2\;3) \}$

$D_{8} {}$:
${} C_{D_{8}}(1)=D_{8} {}$
${} C_{D_{8}}(r)=\{ 1,\, r,\, r^{2},\, r^{3} \} {}$
$C_{D_{8}}(r^{2})=D_{8}$
${} C_{D_{8}}(r^{3})=\{ 1,\, r,\, r^{2},\, r^{3} \} {}$
$C_{D_{8}}(s)=\{ 1,\, s,\, r^{2}, sr^{2} \}$
${} C_{D_{8}}(sr)=\{ 1,\, sr,\, r^{2},\, sr^{3} \} {}$
${} C_{D_{8}}(sr^{2})=\{ 1, sr^{2},\, r^{2},\, s \} {}$
${} C_{D_{8}}(sr^{3})=\{ 1,\, sr^{3},\, r^{2},\, sr \} {}$

$Q_{8}$:
${} C_{Q_{8}}(1)=Q_{8} {}$
${} C_{Q_{8}}(-1)=Q_{8} {}$
${} C_{Q_{8}}(i)=\{ 1,\, -1,\, i,\, -i \} {}$
${} C_{Q_{8}}(-i)=\{ 1,\, -1,\, i,\, -i \}$
${} C_{Q_{8}}(j)=\{ 1,\, -1,\, j,\, -j \} {}$
${} C_{Q_{8}}(-j)=\{ 1,\, -1,\, j,\, -j \} {}$
$C_{Q_{8}}(k)=\{ 1,\, -1,\, k,\, -k \}$
${} C_{Q_{8}}(-k)=\{ 1,\, -1,\, k,\, -k \} {}$
5. skip
6. a)
Let $H\leq G {}$, and let ${} x \in H {}$. Note that ${} xHx^{-1}=\{ xhx^{-1}\mid h \in H \}$. Since ${} x \in G$, and ${} \sigma_{x}(h)=xhx^{-1} {}$ is a bijection, then ${} xhx^{-1} \in H {}$, so ${} xHx^{-1}=H {}$. Therefore, $H= \{ x \in H\mid x Hx^{-1}=H\}\subseteq \{ x \in G\mid xHx^{-1}=H \}=N_{G}(H)$. Since $H$ is a group, then $H\leq N_{G}(H)$. 

For a counterexample, consider any set $H$ that does not contain $1$. Then $H$ cannot be a subgroup of *anything*
b) skip 
7. skip
8. 
Let ${} G=S_{n} {}$, and let $i \in \{ 1,\, 2,\,\dots,\,n \}$, and let ${} G_{i}=\{ \sigma \in G\mid\sigma(i)=i \} {}$. Then $G$ is the group acting on ${} S=\{ 1,\, 2,\,\dots,\,n \} {}$, and ${} G_{i} {}$ is the stabiliser of some element ${} i\in {} S {}$. Therefore $G_{i}\leq G$.

The stabilizers of the elements of $S$ form a partition of $G$. Since there is nothing special about any element of $S$, then the stabilisers must be of equal size. Therefore, we must partition $G$ into $n$ partitions. Since $G$ has order $n!$, then the order of each stabiliser must be $(n-1)!$.
9. 
Let $H\leq G$, and let ${} A\subseteq G {}$ with $A\neq \varnothing$. Let ${} N_{H}(A)=\{ h \in H\mid hAh^{-1}=A \} {}$. 
Let ${} x \in N_{H}(A) {}$. Then $xAx^{-1}=A$. Since ${} x \in H {}$, then ${} x \in G {}$. Therefore, $x \in N_{G}(A)$. Therefore, ${} x \in H \cap N_{G}(A) {}$. Conversely, let ${} x \in H \cap N_{H}(A)$. Then $xAx^{-1}=A$, and ${} x \in H {}$. Therefore, ${} x \in N_{H}(A)$. Therefore, ${} N_{H}(A)=N_{G}(A)\cap H {}$.

Since the intersection of any 2 subgroups is a subgroup, then ${} N_{H}(A)=H \cap N_{G}(A) \leq G {}$. Therefore, as ${} N_{H}(A)\subseteq H$, and it has group structure, then $N_{H}(A)\leq H {}$.
10. 
First we prove a useful lemma:
##### Lemma:
$$
C_{G}(A)=\bigcap_{a\in A} C_{G}(a) 
$$
###### Proof:
Let ${} x \in C_{G}(A) {}$. Then ${} \forall a \in A:xax^{-1}=a {}$. Therefore, given ${} a \in A {}$, then ${} xax^{-1}=a {}$, so ${} x \in C_{G}(a) {}$. Therefore, ${} x \in \bigcap_{a\in A} C_{G}(a) {}$. 

Conversely, let ${} x \in  \bigcap_{a\in A} C_{G}(a) {}$. Then we see that ${} \forall a \in A: xax^{-1}=a {}$. Therefore, by definition, $a \in C_{G}(A) {}$.

Now note that if ${} |H|=2 {}$, then there is a single non-identity element; call it $a {}$. Suppose that ${} x \in N_{G}(H) {}$. Then for $a {}$, we have 2 cases: ${} xax^{-1}=1 {}$ and ${} xax^{-1}=a$. If $xax^{-1}=1 {}$, then ${} xa=x\Rightarrow a=1 {}$, which is a contradiction. Therefore, ${} xax^{-1}=a {}$. For $1 {}$, note that ${} x1x^{-1}=x x^{-1}=1 {}$. Therefore, ${} x \in C_{G}(H) {}$. Since we already know that ${} C_{G}(H)\subseteq N_{G}(H) {}$, then ${} C_{G}(H)=N_{G}(H) {}$.

Now we see that ${} a \in Z(G)$ iff ${} C_{G}(a)=G$. First suppose that ${} a \in Z(G) {}$. Then ${} \forall x \in G:xax^{-1}=x x^{-1}a=a {}$, so $\forall x \in G:x \in C_{G}(a)$, so ${} C_{G}(a)=G$. Conversely, suppose that ${} C_{G}(a)=G$. Then ${} \forall x \in G:xax^{-1}=a$. Therefore, ${} a \in Z(G) {}$. 
Therefore, by the lemma, given a subset ${} A\subseteq Z(G) {}$, then 
$$
C_{G}(A)=\bigcap_{a\in A} C_{G}(a)=\bigcap_{a\in A} G=G
$$
and conversely, if $C_{G}(A)=G {}$, then
$$
C_{G}(A)=\bigcap_{a\in A} C_{G}(a)=G
$$but ${} C_{G}(a)\subseteq G {}$, so ${} \forall a \in A:C_{G}(a)=G$. Therefore, ${} C_{G}(A)=G$ iff $A\subseteq Z(G)$

Since $C_{G}(A)\leq N_{G}(A)\leq G {}$, then if $C_{G}(A)=G {}$, then $N_{G}(A)=G$. Since that happens iff ${} A\subseteq Z(G)$, then if ${} A\subseteq Z(G)$, then $N_{G}(A)=G {}$. Conversely, if ${} H\leq G {}$ with ${} |H|=2 {}$, then ${} N_{G}(H)=C_{G}(H)=G$. Therefore, $H\subseteq Z(G)$
11. 
Let $A\subseteq G$. Now suppose ${} x \in Z(G)=C_{G}(G)\leq C_{G}(A) {}$, as $A \subseteq G {}$. We showed that ${} C_{G}(A)\leq N_{G}(A)$, so $Z(G)=N_{G}(A) {}$.
12. a)
Let ${} p(x_{1},\, x_{2},\, x_{3},\, x_{4})=12x_{1}^{5}x_{2}^{7}x_{4}-18x_{2}^{3}x_{3}+11x_{1}^{6}x_{2}x_{3}^{3}x_{4}^{24} {}$. Then 
$$
\begin{align}
(\sigma\cdot p)(x_{1},\, x_{2},\, x_{3},\, x_{4}) &=12x_{2}^{5}x_{3}^{7}x_{1}-18x_{2}^{3}x_{4}+11x_{2}^{6}x_{3}x_{4}^{3}x_{1}^{24} \\
\tau\cdot (\sigma\cdot p)(x_{1},\, x_{2},\, x_{3},\, x_{4}) & =12x_{3}^{5}x_{1}^{7}x_{2}-18x_{3}^{3}x_{4}+11x_{3}^{6}x_{1}^{3}x_{4}^{3}x_{2}^{24} \\
\sigma\tau=(1\;2\;3\;4)(1\;2\;3) & =(1\;3\;2\;4) \\
((\sigma\tau)\cdot p)(x_{1},\, x_{2},\, x_{3},\, x_{4}) & =12x_{3}^{5}x_{4}^{7}x_{1}-18x_{4}^{3}x_{2}+11x_{3}^{6}x_{4}x_{2}^{3}x_{1}^{24}
\end{align}
$$
b) skip
c)
${} G_{x_{4}}=\{ 1,\, (1\;2),\, (1\;3),\, (2\;3),\, (1\;2\;3),\, (1\;3\;2) \}=S_{3}\cong S_{3} {}$
d)
${} G_{x_{1}+x_{2}}=\{ 1,\, (3\;4),\, (1\;2), (1\;2)(3\;4) \}\cong V_{4}\cong D_{\displaystyle\cancelto{4}{2} \ } {}${}  
e)
${} G_{x_{1} x_{2}+x_{3} x_{4}}=\{ 1,\, (1\;2),\, (3\;4),\, (1\;3)(2\;4),\, (1\;4)(2\;3),\, (1\;3\;2\;4),\, (1\;2)(3\;4),\, (1\;4\;2\;3) \}$
Let $\theta:G_{x_{1} x_{2}+x_{3} x_{4}}\to{}D_{8}$, mapping ${} (1\;2)\mapsto s {}$ and $(1\;3\;2\;4)\mapsto r$. These elements generate the stabilizer, by inspection. Note that ${} |(1\;3\;2\;4)|=4 {}$, ${} |(1\;2)|=2 {}$, and ${} (1\;4\;2\;3)(1\;2)=(1\;3)(2\;4)=(1\;2)(1\;3\;2\;4)$. Therefore, all the same relations that hold in ${} D_{8}$ hold in the stabilizer, so $G_{x_{1} x_{2}+x_{3} x_{4}}\cong D_{8}$
f)
$$
G_{(x_{1}+x_{2})(x_{3}+x_{4})}=\{ 1,\, (1\;2),\, (3\;4),\, (1\;3)(2\;4),\, (1\;4)(2\;3),\, (1\;3\;2\;4),\, (1\;2)(3\;4),\, (1\;4\;2\;3) \}
$$
13. skip are you kidding me
14. skip
