---
tags:
  - dynamical_systems1
  - chapter
date: 2024-01-19
---
[[Directory]], [[Intro to Dynamical Systems 1|Subject Directory]]
[[2. Homogenous and First Order ODEs|Last]] ;; [[4. Peano's and Picard's Theorems|Next]]
# ODEs
## Linear ODES
### General form
We have ${} f,\, g,\, x {}$ as functions of $t$. A linear ODE is of the form
$$
\frac{dx}{dt} -fx=g
$$
If we multiply by a function ${} \mu=\mu(t) {}$, we get
$$
\mu \frac{dx}{dt} -\mu fx=\mu g
$$
Now note that 
$$
\frac{d(\mu x)}{dt} =\mu \frac{dx}{dt}  + x \frac{d\mu}{dt}
$$
So we can add $0$  on our original equation like so
$$
\mu \frac{dx}{dt} +x \frac{d\mu}{dt} - x \frac{d\mu}{dt}-\mu fx=\mu g
$$
and we get
$$
\frac{d(\mu x)}{dt}-x\left( \frac{d\mu}{dt}-\mu f \right)=\mu g
$$
We can pick $\mu$ (as will be shown later) such that
$$
\frac{d\mu}{dt}+\mu f=0
$$
and so we simply get
$$
\frac{d(\mu x)}{dt}=\mu g
$$
This is an *explicit* equation, as $\mu g$ only depends on $t$. Therefore
$$
\begin{align}
 \mu x & =\int \mu g \ud t   \\
 & =\Gamma(t)+C \\
x & =\frac{\Gamma+C}{\mu}
 \end{align} 
$$
Now we find $\mu$. Recall that we pick $\mu$ such that
$$
\frac{d\mu}{dt}+\mu f=0
$$
so
$$
\begin{align}
 \frac{d\mu}{dt} & =-\mu f \\
\frac{1}{\mu} \frac{d\mu}{dt} & =-f  \\
\int \frac{1}{\mu} \ud \mu & =-\int f \ud t   \\
\ln |\mu|+C & =-\int f(t) \ud t 
 \end{align}
$$
so
$$
\mu(t)=\exp\left( -\int f(t) \ud t  +C\right)
$$
(don't ask me where the absolute values went). We generally pick $C$ to be $0$, as we just need *a* $\mu$ that satisfies the equation, and ${} C=0 {}$ is (usually) simpler
#### Example:
$$
t(t+1) \frac{dx}{dt} -(t+2)x=t^{3}(2x-3)
$$
We *bring it to the linear form*, that is, 
$$
\frac{dx}{dt} -\frac{t+2}{t(t+1)}x=\frac{t^{3}(2t-3)}{t(t+1)}=\frac{t^{2}(2t-3)}{t+1}
$$
Note that
$$
f(t)=\frac{ t+2 }{ t(t+1) }\qquad g(t)=\frac{ t^{2}(2t-3) }{ t+1 }
$$
We now find $\mu$. We have
$$
\begin{align}
 \mu(t) & =\exp\left( -\int \frac{ t+2 }{ t(t+1) } \ud t  \right)  \\
 & = \exp\left( -\left( \int \frac{2(t+1)}{t(t+1)}dt-\int  \frac{t}{t(t+1)} \ud t  \right) \right) \\
 & =\exp\left( -\left( \int \frac{2}{t} \ud t -\int \frac{1}{t+1} \ud t  \right) \right) \\
 & =\exp(-(2\ln(t)-\ln(t+1))) \\
 & =\exp(\ln(t+1)+\ln(t^{-2})) \\
 & =\exp\left( \ln\left( \frac{ t+1 }{ t^{2} } \right) \right) \\
 & =\frac{ t+1 }{ t^{2} }
 \end{align}
$$
Finally, we find $x {}$. Recall that
$$
\begin{align}
 x(t) & =\frac{1}{\mu(t)} \int \mu(t)g(t) \ud t  \\ \\
 & =\frac{t^{2}}{t+1} \int \frac{t+1}{t^{2}} \cdot  \frac{t^{2}(2t-3)}{t+1}  \ud t  \\
 & = \frac{t^{2}}{t+1} \int 2t-3 \ud t \\
 & =\frac{t^{2}}{t+2}(t^{2}-3t+C)
 \end{align}
$$
### Another Method
This method isn't very good in it's application to first order linear ODEs, but it generalises better to higher order ODEs.

If we write the map ${} L(x)=\frac{dx}{dt} -fx {}$, so the equation is 
$$
L(x)=g(t)
$$
If ${} g(t)=0 {}$, then 
$$
L(x)=0
$$
is a *homogenous linear* ODE. These are separable, so relatively easy to solve, that is
$$
\begin{align}
\frac{dx}{dt} -fx & =0 \\
\frac{dx}{dt}  & =fx \\
\ln |x| & =\int f(t) \ud t \\
x & =\exp\left( \int f(t) \ud t  \right) \tag{1}
\end{align}
$$
Now if we can find a *particular solution* of
$$
L(x)=g(t)
$$
then we can construct a general solution using ${} (1) {}$. Particular solutions can be found by *guessing* often. Now we can find the general soltuion simply by combining the *complementary function*, ${} x_{\mathrm{cf}}(t) {}$ that is, the solution to the homogenous equation, and a particular solution, ${} x_{\mathrm{pf}}(t) {}$ like so 
$$
x(t)=x_{\mathrm{cf}}(t)+x_{\mathrm{pf}}(t)
$$
#### Example:
$$
\frac{dx}{dt} =-8x+4t+\frac{1}{2}
$$
we see that
$$
f(t)=-8 \qquad \qquad g(t)=4t+\frac{1}{2}
$$
First we solve the homogenous version, we see that
$$
\begin{align}
\frac{dx}{dt} +8x & =0 \\
\ln |x| & =-8t+C \\
x_{\mathrm{cf}}(t) & =Ae^{-8t}
\end{align}
$$
Now to find a particular solution, observe that $t/2 {}$ is a particular solution. Therefore, the general solution is
$$
x(t)=x_{\mathrm{cf}}(t)+x_{\mathrm{pf}}(t)=Ae^{-8t}+\frac{t}{2}
$$
# Summary of Types of ODEs
## Explicit
Are of the form
$$
\frac{dy}{dx} =f(x)
$$
#### Solution:
$$
y=\int f(x) \ud x 
$$
## Separable
Are of the form
$$
\frac{dy}{dx} =f(x)g(y)
$$
#### Solution:
$$
\int \frac{1}{g(y)} \ud y =\int f(x) \ud x 
$$
## Homogeneous
Homo(genius)
Are of the form
$$
\frac{dy}{dx} =f\left( \frac{y}{x} \right)
$$
or
$$
\frac{dy}{dx}=f(x,\, y)
$$
where ${} f(\lambda x,\, \lambda y)=f(x,\, y) {}$ for all ${} \lambda \in \mathbb{R},\, \lambda\neq 0 {}$.
#### Solution:
Set ${} v=\frac{y}{x} {}$ and substitute:
$$
x \frac{dv}{dx} +v=f(v)
$$
we get
$$
\frac{dv}{dx} =\frac{ f(v)-v }{ x }\quad\Rightarrow \quad \int \frac{1}{f(v)-v} \ud v=\int \frac{1}{x} \ud x  
$$
and then we may solve using elementary methods for ${} x {}$
## Linear
Are of the form 
$$
\frac{dy}{dx} =f(x)y+g(x)
$$
#### Solution:
find
$$
\mu(x)=\exp\left( -\int f(x) \ud x  \right)
$$
and we see that
$$
y(x)=\frac{1}{\mu(x)}\int \mu (x)g(x) \ud x 
$$
# Initial Value Problems
## Problem Statement
### General Forms
For first order ODEs, we found
$$
x(t)=h(t,\, C)
$$
where ${} x(t)$ satisfies the ODE iff ${} x(t)=h(t,\, C) {}$ for some ${} C \in \mathbb{R} {}$. Given some pair ${} (t_{0},\, x_{0}) {}$, we want to find $C$ such that
$$
h(t_{0},\, C)=x(t_{0})=x_{0}
$$
#### Example:
$$
\frac{dx}{dt} =\frac{ 2t+1 }{ 3x^{2}+e^{x} }\qquad \qquad x(t_{0})=x_{0}
$$
This is separable, so
$$
\int 3x^{2}+e^{x} \ud x =\int 2t+1 \ud t
$$
and we get
$$
x^{2}+e^{x}=t^{2}+t+C
$$
We can't really solve this for ${} x(t)$. If we plug in the initial condition, then we get
$$
C=x_{0}^{3}+e^{x_{0}}-t_{0} ^{2}- t_{0}
$$
and so we still get a unique $C$. Therefore, we get a unique $C$ for all ${} (x_{0},\, t_{0}) {}$ (if it exists).
#### Example:
$$
\frac{dx}{dt} =\frac{x}{t},\, \qquad \qquad x(t_{0})=x_{0}
$$
we get that
$$
x(t)=Ct
$$
Now substituting the initial value, we get
$$
x_{0}=Ct_{0}
$$
Now if ${} t_{0} {}$ is non-zero, then 
$$
C=\frac{x_{0}}{t_{0}}
$$
If $t_{0}$ is zero, then we can split into 2 cases. First, if ${} x_{0}=0 {}$, then we don't have a unique $C {}$; in fact, it is true for all ${} C \in \mathbb{R} {}$.

Secondly, if ${} x_{0}\neq 0$. Now ${} 0C=x_{0}\neq 0 {}$, so this is not satisfied for *any* ${} C \in \mathbb{R} {}$.
## Existance and Uniqueness of Solutions
### Theorem 2.1: Peano's Theorem
If we have
$$
\frac{dx}{dt} =f(x,\, t),\, \qquad \qquad x(t_{0})=x_{0}
$$
If we can find a value ${} \delta>0 {}$ such that for
$$
A=\{ (t,\, x)\mid |t-t_{0}|< \delta,\, |x - x_{0}| < \delta \}
$$
the function $f:A\to{}\mathbb{R} {}$ is continuous then there is an interval
$$
[t_{0}-\delta,\, t_{0}+\delta]
$$


