---
tags:
  - chapter
  - real_anal1
date: 2024-11-15
completed: true
---
[[Directory]], [[University/Undergraduate/Second Year/Real Analysis 1/Real Analysis 1|Subject Directory]]
[[University/Undergraduate/Second Year/Real Analysis 1/Lectures/1. Introduction|ðŸž€ðŸž€]] [[13. Integral Identities and Inequalities|â—€]] [[15. Improper Integrals|â–¶]] [[University/Undergraduate/Second Year/Real Analysis 1/Lectures/22. |ðŸž‚ðŸž‚]]
# Integration
## Fundamental Theorem of Calculus
### Theorem 1.1: FTC Part 1
Let ${} f \in \mathcal{R}[a,\, b] {}$. For ${} x \in [a,\, b] {}$, put
$$
F(x)=\int_{a}^{x} f(t) \ud t 
$$
Then $F$ is continuous on ${} [a,\, b] {}$. Now if $f$ is continuous at ${} x_{0} \in (a,\, b) {}$, then ${} F$ is differentiable at $x_{0} {}$, and
$$
F'(x_{0})=f(x_{0})
$$
$F$ is called the primitive or antiderivative of $f$. 
#### Proof:
First we show that $F$ is continuous on ${} [a,\, b] {}$. Since ${} f \in \mathcal{R}[a,\, b] {}$, then $f$ is bounded. Therefore, it has an upper bound $M$ such that 
$$
|f(t)|\leq M,\, t \in [a,\, b]
$$
Let ${} x_{1},\, x_{2} \in [a,\, b] {}$. WLOG suppose that ${} x_{1} \leq x_{2} {}$. Then 
$$
\begin{align}
 |F(x_{1})-F(x_{2})| &  = \left|  \int_{a}^{x_{1}} f(t) \ud x -\int_{a}^{x_{2}} f(t) \ud x  \right|    \\
 & =\left|  \int_{x_{1}}^{x_{2}} f(x) \ud x  \right|  \\
 & \leq  (x_{2}-x_{1}) \sup _{t \in [x_{1},\, x_{2}]} |f(t)| \\
 & \leq  (x_{2}-x_{1})M
 \end{align}

$$
and therefore $F$ is Lipschitz continuous, and therefore continuous. 

Now suppose that $f$ is continuous at $x_{0}$. Then given some $\varepsilon>0 {}$, there exists some $\delta>0 {}$ such that ${} |f(s)-f(x_{0})|<\varepsilon {}$ if ${} |s-x_{0}|<\delta {}$. 

Now consider the right derivative of ${} F$. Let ${} t \in (x_{0},\, x_{0}+\delta) {}$. Then 
$$
\begin{align}
\left| \frac{ F(t)-F(x_{0}) }{ t-x_{0} } -f(x_{0})\right| &  =\left| \frac{1}{t-x_{0}}\int_{a}^{t} f(s) \ud s -\frac{1}{t-x_{0}} \int_{a}^{x_{0}} f(s) \ud s -f(x_{0})\right|  \\
 & =\left| \frac{1}{t-x_{0}} \int_{x_{0}}^{t} f(s) \ud s -f(x_{0}) \right|  \\
& =\left| \frac{1}{t-x_{0}} \int_{x_{0}}^{t} f(s) \ud s -\frac{1}{t-x_{0}}\int_{x_{0}}^{t} f(x_{0}) \ud s  \right|  \\
 & =\left| \frac{1}{t-x_{0}} \int_{x_{0}}^{t}( f(s)-f(x_{0})) \ud s  \right|  \\
 & \leq \left|\frac{1}{t-x_{0}}(t-x_{0}) \sup _{s \in [x_{0},\, t] }|f(s)-f(x_{0})|\right| \\
 & <\varepsilon
\end{align}
$$
and so
$$
\lim_{t\tto x_{0}^{+}} \frac{ F(t)-F(x_{0}) }{ t-x_{0} } =f(x_{0})
$$
and likewise for the left derivative. Therefore, $F$ is differentiable at $x_{0}$, and 
$$
F'(x_{0})=f(x_{0})
$$
### Theorem 1.2: FTC Part 2
Let ${} f \in C[a,\, b] {}$ with ${} f \in C^{1}(a,\, b) {}$, and ${} f' \in \mathcal{R}[a,\, b] {}$. Then for all ${} x \in [a,\, b] {}$, 
$$
f(x)=f(a)+\int_{a}^{x} f'(s) \ud s 
$$
#### Proof:
Let ${} G(x)=f(a)-f(x)+\int_{a}^{x} f'(x) \ud s  {}$. We want to show that ${} G(x)=0 {}$. By the FTC part 1, we have that
$$
G'(x)=f'(x)+f'(x)=0
$$
Therefore, ${} G=c {}$ some constant. Then 
$$
\begin{align}
G(a)=f(a)-f(a)+\int_{a}^{a} f'(s) \ud s =0
\end{align}
$$
and so ${} G(x)=0 {}$ for all ${} x \in [a,\, b] {}$.
### Theorem 1.3: Integration by Parts
Let ${} f,\, g \in C[a,\, b] {}$ with ${} f',\, g' \in C[a,\, b] {}$. Then
$$
\int_{a}^{b} f'(x)g(x) \ud x =f(b)g(b)-f(a)g(a)-\int_{a}^{b} f(x)g'(x) \ud x 
$$
### Theorem 1.4: Change of Variable
Let ${} \varphi \in C[a,\, b] {}$ and ${} \varphi' \in C[a,\, b] {}$ with ${} \varphi(a)=A {}$, and ${} \varphi(b)=B {}$, and let ${} f \in C[A,\, B] {}$. Then
$$
\int_{A}^{B}f(y)  \ud y= \int_{a}^{b} f(\varphi(x))\varphi'(x) \ud x  
$$