---
tags:
  - chapter
  - real_anal1
date: 2024-10-18
---
[[Directory]], [[University/Undergraduate/Second Year/Real Analysis 1/Real Analysis 1|Subject Directory]]
[[University/Undergraduate/Second Year/Real Analysis 1/Lectures/1. Introduction|ðŸž€ðŸž€]] [[7. Lipschitz Continuity|â—€]] [[9. Derivative Tests and Convexity|â–¶]] [[University/Undergraduate/Second Year/Real Analysis 1/Lectures/22. |ðŸž‚ðŸž‚]]
# Iterated Differentiation
## Mean Value Theorem Corollaries
### Corollary 1.1:
If ${} f'(x)=0 {}$ for all ${} x \in (a,\, b) {}$, then $f$ is constant.
#### Proof:
Given ${} x \in (a,\, b) {}$, we know that there exists some ${} c \in (a,\, x) {}$ such that ${} 0=f'(c)=f(x)=\frac{f(x)-f(a)}{x-a}  {}$, and so ${} f(x)=f(a) {}$. Therefore, $f$ is constant. 
### Corollary 1.2:
If ${} f'(x)>0 {}$ for all ${} x \in (a,\, b) {}$, then $f$ is strictly increasing on ${} [a,\, b] {}$. 
#### Proof:
Given ${} x<y \in [a,\, b] {}$, by MVT there exists some ${} c \in (x,\, y) {}$ such that 
$$
f'(c)=\frac{ f(y)-f(x) }{ y-x }>0
$$
since ${} y-x>0 {}$, then ${} f(y)-f(x)>0 {}$, and ${} f(y)>f(x) {}$
## Taylor's Formula
### Definition 1.3: ${} n {}$-times Differentiable
We say that ${} f$ is $n$-times differentiable, if
$$
\begin{align}
f^{(0)} & =f  &  & \text{ is differentiable} \\
f^{(1)} & =f'  &  & \text{ is differentiable} \\
 & \vdots \\
f^{(n-1)} & =(f^{(n-2)})'  &  & \text{ is differentiable}
\end{align}
$$
and say that $f$ is $n$-times continuously differentiable if it is $n$-times differentiable and ${} f^{(n)} {}$ is continuous.

We write ${} f \in C^{n}(a,\, b) {}$ if $f$ is $n$-times continuously differentiable on ${} (a,\, b) {}$.
### Theorem 1.4: Taylor's Formula
Suppose that ${} f \in C^{n}(a,\, b) {}$, and ${} x_{0} \in (a,\, b) {}$. Then for all ${} x \in (a,b) {}$, there exists some ${} c {}$ between $x$ and $x_{0}$ such that 
$$
f(x)=\underbrace{ \sum_{k=0}^{n-1} \frac{f^{(k)}(x_{0})}{k!}(x-x_{0})^{k} }_{ \substack{\text{ Taylor Polynomial}\\ \text{ of order }n-1 \text{ at }x_{0}}  }+\underbrace{ \frac{f^{(n)}(c)}{n!}(x-x_{0})^{n} }_{ \substack{O\left((x-x_{0})^{n}\right)\\\text{ as }x\tto x_{0}}  }
$$
#### Remarks:
When ${} n=1 {}$, then this is just MVT. 

If ${} f^{(n)}(x)=0 {}$ for all ${} x \in (a,\, b) {}$, then $f$ is a polynomial of order ${} (n-1) {}$. 
#### Proof:
Suppose ${} x_{0}=0 {}$ (WLOG, since we can always change the variables). Fix some $x\neq x_{0}$ in ${} (a,\, b) {}$. We claim that there exists some $c$ between $x_{0}$ and $x {}$ such that
$$
f(x)=\sum_{k=0}^{n-1} \frac{f^{k}(0)}{k!} x^{k}+\frac{f^{(n)}(c)}{n!}x^{n} 
$$
Define ${} P(t)=\sum_{k=0}^{n-1} \frac{f^{(k)}(0)}{k!}t^{k} {}$. Define ${} M \in \mathbb{R} {}$ so that ${} f(x)=P(x)+\frac{M}{n!}x^{n} {}$. We claim that ${} M=f^{(n)}(c) {}$ for some $c$ between $x$ and $x_{0}$.

Let ${} g(t)=f(t)-P(t)-\frac{M}{n!}t^{n} {}$. Then 
$$
\begin{align}
g^{(n)}(t) & =f^{(n)}(t)-P^{(n)}(t)-m \\
 & =f^{(n)}(t)-M
\end{align}
$$
Then the claim is proven if there exists some $c$ such that ${} g^{(n)}(c)=0 {}$. Note:
$$
\begin{align}
g(0) & =f(0)-P(0)=f(0)-f(0)=0 \\
 g'(0) & =f'(0)-P'(0)=f'(0)-f'(0)=0 \\
 & \vdots  \\
g^{(n-1)}(0) & =f^{n-1}(0)-P^{(n-1)}(0)=0
\end{align}
$$
By the definition of $M$, ${} g(x)=f(x)-\left( P(x)+\frac{M}{n!}x^{n} \right)=0 {}$. Then we may use Rolle's Theorem to show that ${} g'(c_{1})=0 {}$ for some $c_{1}$ between $0$ and $x {}$. We may continue by induction by using Rolle's to show that ${} g^{(k)}(c_{k})=0 {}$ for some ${} c_{k} {}$ between $0$ and ${} c_{k-1} {}$, till we obtain a ${} c_{n} {}$ such that
$$
g^{(n)}(c_{n})=0
$$
for some ${} c_{n} {}$ between $0$ and $x$. Therefore, the claim is proven. 
### Corollary 1.5:
For ${} x_{0} \in (a,\, b) {}$, ${} \delta>0 {}$, and ${} x \in [x_{0}-\delta,\, x_{0}+\delta] {}$, we have
$$
\left| f(x)=\sum_{k=0}^{n-1} \frac{f^{(k)}(x_{0})}{k!}(x-x_{0})^{k} \right| \leq \frac{1}{n!} \left(\sup _{t \in [x_{0}-\delta,\, x_{0}+\delta]}f^{(n)}(t)\right)|x-x_{0}|^{n}
$$