---
tags:
  - chapter
  - seq_and_series1
date: 2023-10-10
---
[[Directory]], [[Sequences and Series 1|Subject Directory]] 
# Proofs
## Propositions and Implication
### The Deductive Method
We have $P(x)$ to be true. The general structure of a proof is to show that this implies another statement $Q(x)$ is true. Often, this cannot be done directly, and we must have in-between statements, so we have a chain of propositions, each leading from the last, as so:
$$
\begin{align}
P(x) & \Rightarrow P_{1}(x) \\
P_{1}(x) & \Rightarrow P_{2}(x) \\
P_{2}(x) & \Rightarrow P_{3}(x) \\
& \ \ \,\vdots \\
P_{n}(x) & \Rightarrow Q(x)
\end{align}
$$

### Proving Equality of Sets
Say we have 2 sets $A$ and $B$. How can we prove that $A=B$?

To do this, we must show that $x \in A\Rightarrow x \in B$, and $x \in B \Rightarrow x \in A$.
(Note that this is equivalent to $x \in A \iff x \in B$)

#### Example:
$A=\{ n \in \mathbb{N} \mid n=2k, k \in \mathbb{N} \}$
$B=\{ n \in \mathbb{N} \mid n=3k, k \in \mathbb{N} \}$
$C=\{ n \in \mathbb{N} \mid n=6k, k \in \mathbb{N} \}$

We want to show that $C=A\cap B$
Proof:
1. $x \in C\Rightarrow x \in A \cap B$
	$$
\begin{align}
x \in C & \Rightarrow\exists m \in \mathbb{N}: x=6m \\
 & \Rightarrow\exists m \in \mathbb{N}: x=2(3m)=3(2m) \\
 & \Rightarrow x \in A \wedge x \in B \\
 & \Rightarrow x \in A \cap B
\end{align}
$$
2. $x \in A \cap B \Rightarrow x \in C$
$$
\begin{align}
x \in A \cap B  & \Rightarrow x \in A \wedge x \in B \\
 & \Rightarrow(\exists m \in \mathbb{N}: x=2m) \wedge (\exists n \in \mathbb{N}: x=3n) \\
 & \Rightarrow \exists m,\, n \in \mathbb{N}: x=2m=3n \\
 & \Rightarrow \exists k \in \mathbb{N}: n=2k \wedge x=3n \\
 & \Rightarrow \exists  k \in \mathbb{N} : x=3n=3(2k)=6k \\
 & \Rightarrow x \in C
\end{align}
$$
Therefore, $C=A\cap B$.

### Theorem 1.1: Distributivity of $\cap$ and $\cup$
For any sets $A, B, C$, we have 
1. $A\cup(B\cap C)=(A\cup B)\cap(A\cup C)$
2. $A\cap(B\cup C)=(A\cap B)\cup(A\cap C)$

#### Proof:
1. $A\cup(B\cap C)=(A\cup B)\cap(A\cup C)$
Take $x \in A\cup(B\cap C)$. This implies that $x \in A \vee x \in (B \cap C)$
Case 1:
$$
\begin{align}
 x \in A  & \Rightarrow x \in A\cup B \wedge x \in A \cup C   \\
 & \Rightarrow x \in (A\cup B)\cap (A\cup C)
 \end{align}
$$
Case 2:
$$
\begin{align}
x \in B \cap C  & \Rightarrow x \in B \cap x \in C \\
 & \Rightarrow x \in A \cup B \cap x \in A \cup C \\
 & \Rightarrow x \in (A \cup B) \cap (A \cup B)
\end{align}
$$
Now take $x \in (A \cup B) \cap (A \cup C)$.
Case 1:
$$
x \in A\cap(A \cup B) \cap (A \cup C)\Rightarrow  A\cup(B \cap C)
$$
Case 2:
$$
\begin{align}
 x \in ((A \cup B)\cap (A \cup C))\setminus A & \Rightarrow  x \in (A \cup B)\setminus A \wedge x \in (A \cup C) \setminus A \\
 & \Rightarrow x \in B \wedge x \in C \\
 & \Rightarrow x \in B \cap C \\
 & \Rightarrow x \in A \cup(B \cap C)
 \end{align} 
$$
2. $A\cap(B\cup C)=(A\cap B)\cup(A\cap C)$
This is left as an exercise to the reader

## Proof by Induction
### A Strategy
Want to prove $P(n)$ for all $n \in \mathbb{N}$

Induction tells us that its enough to show that 
1. $P(1)$ is true
2. $\forall k\in\mathbb{N}, P(k)=\to{}p\Rightarrow P(k+1)=\to{}p$

#### Example:
$P(n)=\left( \sum_{k=1}^{n}k=\frac{1}{2}n(n+1) \right)$

## Proof by Contradiction
### A strategy
Want to prove $P(x)$. Consider $\neg P(x)$. so
$$
\begin{align}
\neg P(x)\Rightarrow Q(x) \\
\neg Q(x)\Rightarrow P(x)
\end{align}
$$
We start by building an implication from $\neg P(x)$ to a false statement $Q(x)$. This then gives us $P(x)$ true.

### Theorem 1.2: The irrationality of $\sqrt{2}$
#### Proof:
We work by contradiction. Assume that there exist $p, q \in \mathbb{N}$ with $\gcd(p,\,q)=1$ such that 
$$
\sqrt{2}=\frac{p}{q}
$$
Now we have 
$$
\begin{align}
 q\sqrt{2}=p & \Rightarrow 2q^{2}=p^{2}   \\
 & \Rightarrow \exists k \in \mathbb{N}, p=2k \wedge 2q^{2}=p^{2} \\
 & \Rightarrow \exists k \in \mathbb{N}, 2q^{2}=(2k)^{2}=4k^{2} \\
 & \Rightarrow \exists k \in \mathbb{N}, q^{2}=2k^{2}
 \end{align}
$$
Therefore, both $p$ and $q$ are even, so $\gcd(p,\,q)=2$, which is a contradiction. So there cannot exist 2 $p, q$ with $\gcd(p,\,q)=1$ such that $\sqrt{2}=p/q$. Therefore, $\sqrt{2}$ is irrational
## Proof by Counter Example
### A strategy
This is fairly simple: It only takes 1 exception to disprove a for all statement.

#### Example:
$p(n)=n^{2}+n+41$ is prime for all $n\geq 0$
Counter example:
$p(40)=41^{2}$ is a counterexample

## Further examples
### Example 1:
$$
\bigcup_{n=1}^{\infty} (-n,n)=\mathbb{R}
$$
#### Proof:
1. $$
\begin{align}
x \in \bigcup_{n=1}^{\infty}(-n,n) & \Rightarrow \exists n \in \mathbb{N}: x \in (-n, n) \\
 & \Rightarrow x \in \mathbb{R}
\end{align}
$$
2. Take $x \in \mathbb{R}$
Case 1: $x\geq 0$
Take $n=\ceil*{x}+1$. Therefore, $x \in (-n,\, n)$

Case 2: $x<0$
Take $n=\floor*{x}-1$. Therefore, $x \in (-n,\,n)$

Therefore, $x \in \mathbb{R}\Rightarrow x \in \bigcup_{n=1}^{\infty}(-n,\,n)$

### Example 2:
$$
\bigcap_{n=1}^{\infty} \left( -\frac{1}{n},\, \frac{1}{n} \right)=\{ 0 \}
$$
1. $x \in \{ 0 \}$
$$
\begin{align}
 x \in \{ 0 \}&\Rightarrow x=0  \\
 & \Rightarrow  \forall n \in \mathbb{N}: x \in \left( -\frac{1}{n},\, \frac{1}{n} \right)  \\
 & \Rightarrow x \in \bigcap_{n=1}^{\infty} \left( -\frac{1}{n},\, \frac{1}{n} \right)
 \end{align}
$$
2. $x \in \bigcap_{n=1}^{\infty}(-1/n, 1/n)$
We argue by contradiction. Assume
$$
\begin{align}
x \in \bigcap_{n=1}^{\infty} \left(-\frac{1}{n},\,  \frac{1}{n} \right)\setminus \{ 0 \}
\end{align}
$$
Case 1: $x>0$
$$
\begin{align}
&x>0 \wedge \forall n \in \mathbb{N}:x \in\left( -\frac{1}{n},\, \frac{1}{n} \right) \\
 & \Rightarrow  x>0 \wedge \forall n \in \mathbb{N}:x<\frac{1}{n} \\
 & \Rightarrow x>0 \wedge \forall n \in \mathbb{N}: n<\frac{1}{x}
\end{align}
$$
This is a contradiction, so $x\not>0$

Case 2: $x<0$
$$
\begin{align}
&\quad x<0 \wedge \forall n \in \mathbb{N}: x \in \left( -\frac{1}{n}, \frac{1}{n} \right) \\
&\Rightarrow x<0 \wedge \forall  n \in \mathbb{N}: -\frac{1}{n}<x \\
 & \Rightarrow x<0 \wedge \forall n \in \mathbb{N}: -\frac{1}{x}>n
\end{align}
$$

This is a contradiction, so $x\not<0$ 
Therefore, $x=0$
Therefore, 
$$
\bigcap_{n=1}^{\infty} \left( -\frac{1}{n},\, \frac{1}{n} \right)=\{ 0 \}
$$
